<rdf:RDF
    xmlns:rdf="http://www.w3.org/1999/02/22-rdf-syntax-ns#"
    xmlns:dc-term="http://purl.org/dc/terms/"
    xmlns:dc="http://purl.org/dc/elements/1.1/"
    xmlns:ptop="http://www.ontotext.com/proton/protontop#"
    xmlns:owl="http://www.w3.org/2002/07/owl#"
    xmlns:pext="http://www.ontotext.com/proton/protonext#"
    xmlns:rdfs="http://www.w3.org/2000/01/rdf-schema#"
    xmlns:xsd="http://www.w3.org/2001/XMLSchema#">
  <owl:Ontology rdf:about="http://www.ontotext.com/proton/protonext">
    <owl:versionInfo>3.0</owl:versionInfo>
    <owl:imports rdf:resource="http://www.ontotext.com/proton/protontop"/>
    <dc:rights>Proton ontology is available under the Creative Commons Attribution 3.0 Unported license; see http://creativecommons.org/licenses/by/3.0/. In a nutshell, you are free to copy, distribute and transmit the work; to remix/adapt the work (e.g. to import the ontology and create specializations of its elements), as long as you attribute the work in the manner specified by the author or licensor (but not in any way that suggests that they endorse you or your use of the work). Proper Attribution: Simply include the statement This work is based on Proton ontology, developed by Ontotext and link back to http://www.ontotext.com/proton-ontology</dc:rights>
    <dc:creator>Ontotext (Ivan Terziev, Atanas Kiryakov, Kiril Simov, Dimitar Manov, Mariana Damova, Svetoslav Petrov) </dc:creator>
    <rdfs:label>Proton Ontology</rdfs:label>
    <dc:subject>Upper-level ontology with extensions to handle Linked Open Data (LOD)</dc:subject>
    <dc:title>Proton</dc:title>
    <rdfs:comment>PROTON (Proto Ontology), Extension module</rdfs:comment>
  </owl:Ontology>
  <owl:Class rdf:about="http://www.ontotext.com/proton/protonext#WaterReach">
    <rdfs:subClassOf>
      <owl:Class rdf:about="http://www.ontotext.com/proton/protonext#WaterRegion"/>
    </rdfs:subClassOf>
    <rdfs:label xml:lang="en">Reach</rdfs:label>
    <rdfs:comment xml:lang="en">A straight section of a navigable stream or channel between two bends. NIMA GNS designator H.RCH.</rdfs:comment>
  </owl:Class>
  <owl:Class rdf:about="http://www.ontotext.com/proton/protonext#Machine">
    <rdfs:subClassOf rdf:resource="http://www.ontotext.com/proton/protontop#ProductModel"/>
    <rdfs:label xml:lang="en">Device</rdfs:label>
    <rdfs:label xml:lang="en">Machine</rdfs:label>
    <rdfs:comment xml:lang="en">Any produced device with particular purpose that uses energy to perform some activity. The device has parts that perform or assist in performing any type of work. (Wikipedia)</rdfs:comment>
  </owl:Class>
  <owl:Class rdf:about="http://www.ontotext.com/proton/protonext#VideoGame">
    <rdfs:subClassOf>
      <owl:Class rdf:about="http://www.ontotext.com/proton/protonext#Software"/>
    </rdfs:subClassOf>
    <rdfs:label xml:lang="en">Video Game</rdfs:label>
    <rdfs:comment xml:lang="en">Any electronic game that involves interaction with a user interface to generate visual feedback on a video device. (Wikipedia)</rdfs:comment>
  </owl:Class>
  <owl:Class rdf:about="http://www.ontotext.com/proton/protonext#TournamentOccurrence">
    <rdfs:subClassOf>
      <owl:Class rdf:about="http://www.ontotext.com/proton/protonext#SportEvent"/>
    </rdfs:subClassOf>
    <rdfs:label xml:lang="en">Tournament</rdfs:label>
    <rdfs:comment xml:lang="en">A Tournament held at a particular time</rdfs:comment>
  </owl:Class>
  <owl:Class rdf:about="http://www.ontotext.com/proton/protonext#Reserve">
    <rdfs:subClassOf>
      <owl:Class rdf:about="http://www.ontotext.com/proton/protonext#Facility"/>
    </rdfs:subClassOf>
    <rdfs:label xml:lang="en">Reserve</rdfs:label>
    <rdfs:comment xml:lang="en">(ADL FT) Areas set aside for the preservation of fauna, flora, and their natural habitats. [Macmillan Encyc., 2001] We use this category for agricultural reserves; for conservation areas; for demonstration areas; for environmental areas; for forest reserves; for game management areas; for hunting reserves; for management areas (reserves); for natural areas; for nature reserves; for palm tree reserves; for preserves; for primitive areas; for protected areas; for reservations (nature sites); for road less areas; for sanctuaries (wildlife); for wildlife areas; for wildlife refuges; and for wildlife reserves. NIMA GNS designators RES, RESA, RESF, RESH, RESN, RESP, RESV, RESW.</rdfs:comment>
  </owl:Class>
  <owl:Class rdf:about="http://www.ontotext.com/proton/protonext#SoccerClub">
    <rdfs:subClassOf>
      <owl:Class rdf:about="http://www.ontotext.com/proton/protonext#SportClub"/>
    </rdfs:subClassOf>
    <rdfs:label xml:lang="en">Soccer Club</rdfs:label>
    <rdfs:comment xml:lang="en">A soccer (football) team</rdfs:comment>
    <rdfs:comment xml:lang="en">A sport club that organizes the playing of soccer.</rdfs:comment>
  </owl:Class>
  <owl:Class rdf:about="http://www.ontotext.com/proton/protonext#ReferenceLocation">
    <rdfs:subClassOf>
      <owl:Class rdf:about="http://www.ontotext.com/proton/protonext#Facility"/>
    </rdfs:subClassOf>
    <rdfs:label xml:lang="en">Reference Location</rdfs:label>
    <rdfs:comment xml:lang="en">(ADL FT) We use this category for astronomical stations; for beacons; for bench marks; for boundaries; for boundary markers; for buoys; for control points; for geodectic stations; for geographic centers; for landmarks (reference locations); for light houses; for light stations; for lighthouses; for markers; for milestones; for plaques; for poles (sphere); for triangulation stations; and for walls. NIMNA GNS designators LTHSE, BP, TRIG.</rdfs:comment>
  </owl:Class>
  <owl:Class rdf:about="http://www.ontotext.com/proton/protonext#Project">
    <rdfs:subClassOf rdf:resource="http://www.ontotext.com/proton/protontop#Event"/>
    <rdfs:label xml:lang="en">Project</rdfs:label>
    <rdfs:comment xml:lang="en">A project is carefully planned event to achieve a particular aim. Based on Wikipedia.</rdfs:comment>
  </owl:Class>
  <owl:Class rdf:about="http://www.ontotext.com/proton/protonext#PostalAddress">
    <rdfs:subClassOf>
      <owl:Class rdf:about="http://www.ontotext.com/proton/protonext#Address"/>
    </rdfs:subClassOf>
    <rdfs:label xml:lang="en">Postal Address</rdfs:label>
    <rdfs:comment xml:lang="en">An address of a geographical place - usually a building. A postal address consists, usually, of a country name, zip code, city/village name, street name and number, a person name.</rdfs:comment>
  </owl:Class>
  <owl:Class rdf:about="http://www.ontotext.com/proton/protonext#SpeedwayLeague">
    <rdfs:subClassOf>
      <owl:Class rdf:about="http://www.ontotext.com/proton/protonext#SportsLeague"/>
    </rdfs:subClassOf>
    <rdfs:label xml:lang="en">Speedway League</rdfs:label>
    <rdfs:comment xml:lang="en">Any Speedway league</rdfs:comment>
  </owl:Class>
  <owl:Class rdf:about="http://www.ontotext.com/proton/protonext#BodyPart">
    <rdfs:subClassOf rdf:resource="http://www.ontotext.com/proton/protontop#Object"/>
    <rdfs:label xml:lang="en">Body Part</rdfs:label>
    <rdfs:comment xml:lang="en">Any part of the body of any living entity</rdfs:comment>
  </owl:Class>
  <owl:Class rdf:about="http://www.ontotext.com/proton/protonext#Library">
    <rdfs:subClassOf>
      <owl:Class rdf:about="http://www.ontotext.com/proton/protonext#ResourceCollection"/>
    </rdfs:subClassOf>
    <rdfs:label xml:lang="en">Library</rdfs:label>
    <rdfs:comment xml:lang="en">A collection of books, journals, audio and video materials, etc.</rdfs:comment>
  </owl:Class>
  <owl:Class rdf:about="http://www.ontotext.com/proton/protonext#LivingObject">
    <rdfs:subClassOf rdf:resource="http://www.ontotext.com/proton/protontop#Object"/>
    <rdfs:label xml:lang="en">Living Object</rdfs:label>
    <rdfs:comment xml:lang="en">Living object is any organism which is living, e.g. breathing and regular lifecycle.</rdfs:comment>
  </owl:Class>
  <owl:Class rdf:about="http://www.ontotext.com/proton/protonext#Territory">
    <rdfs:subClassOf>
      <owl:Class rdf:about="http://www.ontotext.com/proton/protonext#LandRegion"/>
    </rdfs:subClassOf>
    <rdfs:label xml:lang="en">Territory</rdfs:label>
    <rdfs:comment xml:lang="en">Territory a region of land which can be a part of contry that is non-sovereign or a geographic region determined by some charateristics. (Wikipedia) (http://www.eionet.europa.eu/gemet/concept?ns=1&amp;cp=8401. NIMA GNS designator A.TERR.</rdfs:comment>
  </owl:Class>
  <owl:Class rdf:about="http://www.ontotext.com/proton/protonext#Market">
    <rdfs:subClassOf>
      <owl:Class rdf:about="http://www.ontotext.com/proton/protonext#BusinessAbstraction"/>
    </rdfs:subClassOf>
    <rdfs:label xml:lang="en">Market</rdfs:label>
    <rdfs:comment xml:lang="en">In contrast to IndustrySector, the market is determined by the customers instead of the business or the manifacturers. The market can be defined in terms of types of goods/services, geographic region, price levels and typical customer behaviours. Corresponding to the third sense in WordNet 1.7.1 "the customers for a particular product or service".</rdfs:comment>
  </owl:Class>
  <owl:Class rdf:about="http://www.ontotext.com/proton/protonext#Week">
    <rdfs:subClassOf rdf:resource="http://www.ontotext.com/proton/protontop#TimeInterval"/>
    <rdfs:label xml:lang="en">Week</rdfs:label>
    <rdfs:comment xml:lang="en">A specific week of a specific year (say the 41st of 2001)</rdfs:comment>
  </owl:Class>
  <owl:Class rdf:about="http://www.ontotext.com/proton/protonext#Camp">
    <rdfs:subClassOf>
      <owl:Class rdf:about="http://www.ontotext.com/proton/protonext#RecreationalFacility"/>
    </rdfs:subClassOf>
    <rdfs:label xml:lang="en">Camp</rdfs:label>
    <rdfs:comment xml:lang="en">(ADL FT) Designated areas on which primitive structure(s) are erected for temporary shelter or where recreational vehicles are temporarily parked. [USGS Circ 1048] We use this category for campgrounds; for camping sites; for logging camps; for oil camps; for refugee camps; for RV parks; and for trailer parks (recreational). NIMA GNS designators CMP, CMPL, CMPLA, CMPO, CMPQ, CMPRF.</rdfs:comment>
  </owl:Class>
  <owl:Class rdf:about="http://www.ontotext.com/proton/protonext#PopulatedPlaceName">
    <rdfs:subClassOf rdf:resource="http://www.ontotext.com/proton/protontop#ContactInformation"/>
    <rdfs:label xml:lang="en">City Name</rdfs:label>
    <rdfs:label xml:lang="en">Country Name</rdfs:label>
    <rdfs:label xml:lang="en">Name of a Populated Place</rdfs:label>
    <rdfs:label xml:lang="en">Town Name</rdfs:label>
    <rdfs:label xml:lang="en">Village Name</rdfs:label>
    <rdfs:comment xml:lang="en">Part of a postal address denoting the name of a village, town, city, country, etc.</rdfs:comment>
  </owl:Class>
  <owl:Class rdf:about="http://www.ontotext.com/proton/protonext#SeaSound">
    <rdfs:subClassOf>
      <owl:Class rdf:about="http://www.ontotext.com/proton/protonext#WaterRegion"/>
    </rdfs:subClassOf>
    <rdfs:label xml:lang="en">Sound</rdfs:label>
    <rdfs:comment xml:lang="en">A long arm of the sea forming a channel between the mainland and an island or islands; or connecting two larger bodies of water. NIMA GNS designator H.SD.</rdfs:comment>
  </owl:Class>
  <owl:Class rdf:about="http://www.ontotext.com/proton/protonext#Award">
    <rdfs:subClassOf rdf:resource="http://www.ontotext.com/proton/protontop#Abstract"/>
    <rdfs:label xml:lang="en">Award</rdfs:label>
    <rdfs:comment xml:lang="en">Any award. An award is something given to a person or a group of people to recognize excellence in a certain field; a certificate of excellence, for example trophies, titles, medals, badges, etc.</rdfs:comment>
  </owl:Class>
  <owl:Class rdf:about="http://www.ontotext.com/proton/protonext#ReligiousOrganization">
    <rdfs:subClassOf rdf:resource="http://www.ontotext.com/proton/protontop#Organization"/>
    <rdfs:label xml:lang="en">Religious Organization</rdfs:label>
    <rdfs:comment xml:lang="en">Organization which offers ideas and opinions about life. Just joking.</rdfs:comment>
  </owl:Class>
  <owl:Class rdf:about="http://www.ontotext.com/proton/protonext#Plateau">
    <rdfs:subClassOf>
      <owl:Class rdf:about="http://www.ontotext.com/proton/protonext#LandRegion"/>
    </rdfs:subClassOf>
    <rdfs:label xml:lang="en">Plateau</rdfs:label>
    <rdfs:comment xml:lang="en">(ADL FT) Comparatively flat areas of great extent and elevation; specif. extensive land regions considerably above the adjacent country or above sea level; commonly limited on at least one side by an abrupt descent, have flat or nearly smooth surfaces but are often dissected by deep valleys and surmounted by high hills or mountains, and have a large part of their total surface at or near the summit level. We use this category for table mountains; and for tablelands. The ADL type Mesas, collapsed here. NIMA GNS designators PLAT, PLTX, PLTU, MESA, MESU, TMSU, TMST.</rdfs:comment>
  </owl:Class>
  <owl:Class rdf:about="http://www.ontotext.com/proton/protonext#NonGeographicLocation">
    <rdfs:subClassOf rdf:resource="http://www.ontotext.com/proton/protontop#Location"/>
    <rdfs:label xml:lang="en">Non-Geographic Location</rdfs:label>
    <rdfs:comment xml:lang="en">A non-geographic region in some 3D space. The Longitude and Latitude properties for such objects could be void.</rdfs:comment>
  </owl:Class>
  <owl:Class rdf:about="http://www.ontotext.com/proton/protonext#MountainPass">
    <rdfs:subClassOf>
      <owl:Class rdf:about="http://www.ontotext.com/proton/protonext#LandRegion"/>
    </rdfs:subClassOf>
    <rdfs:label xml:lang="en">Mountain Pass</rdfs:label>
    <rdfs:comment xml:lang="en">Any mountain pass. NIMA GNS designators - no direct equivalents</rdfs:comment>
  </owl:Class>
  <owl:Class rdf:about="http://www.ontotext.com/proton/protonext#Non-ProfitOrganisation">
    <rdfs:subClassOf rdf:resource="http://www.ontotext.com/proton/protontop#Organization"/>
    <rdfs:label xml:lang="en">Non-Orofit Organisation</rdfs:label>
    <rdfs:comment xml:lang="en">Any Non-Profit Organization, an organization that does not distribute its surplus funds to owners or shareholders, but instead uses them to help pursue its goals. (Wikipedia)</rdfs:comment>
  </owl:Class>
  <owl:Class rdf:about="http://www.ontotext.com/proton/protonext#GeographicLocation">
    <rdfs:subClassOf rdf:resource="http://www.ontotext.com/proton/protontop#Location"/>
    <rdfs:label xml:lang="en">Geographic Region</rdfs:label>
    <rdfs:comment xml:lang="en">Any Geographic Region with lattitude and longitude coordinates</rdfs:comment>
  </owl:Class>
  <owl:Class rdf:about="http://www.ontotext.com/proton/protonext#Settlement">
    <rdfs:subClassOf>
      <owl:Class rdf:about="http://www.ontotext.com/proton/protonext#PopulatedPlace"/>
    </rdfs:subClassOf>
    <rdfs:label xml:lang="en">Settlement</rdfs:label>
    <rdfs:comment xml:lang="en">Describes a populated place with organisation, like city, village, town</rdfs:comment>
  </owl:Class>
  <owl:Class rdf:about="http://www.ontotext.com/proton/protonext#Tournament">
    <rdfs:subClassOf>
      <owl:Class rdf:about="http://www.ontotext.com/proton/protonext#RecurringEvent"/>
    </rdfs:subClassOf>
    <rdfs:label xml:lang="en">Tournament</rdfs:label>
    <rdfs:comment xml:lang="en">A Tournament which is held regularly at particular time intervals, every year, every week, etc.</rdfs:comment>
  </owl:Class>
  <owl:Class rdf:about="http://www.ontotext.com/proton/protonext#BaseballLeague">
    <rdfs:subClassOf>
      <owl:Class rdf:about="http://www.ontotext.com/proton/protonext#SportsLeague"/>
    </rdfs:subClassOf>
    <rdfs:label xml:lang="en">Baseball League</rdfs:label>
    <rdfs:comment xml:lang="en">Any Baseball league</rdfs:comment>
  </owl:Class>
  <owl:Class rdf:about="http://www.ontotext.com/proton/protonext#Hotel">
    <rdfs:subClassOf>
      <owl:Class rdf:about="http://www.ontotext.com/proton/protonext#Building"/>
    </rdfs:subClassOf>
    <rdfs:label xml:lang="en">Hotel</rdfs:label>
    <rdfs:comment xml:lang="en">A hotel is an establishment that provides paid lodging on a short-term basis. Wikipedia</rdfs:comment>
  </owl:Class>
  <owl:Class rdf:about="http://www.ontotext.com/proton/protonext#Vein">
    <rdfs:subClassOf rdf:resource="http://www.ontotext.com/proton/protonext#BodyPart"/>
    <rdfs:label xml:lang="en">Vein</rdfs:label>
    <rdfs:comment xml:lang="en">Vein is a general concept gathering all veins of a body.</rdfs:comment>
  </owl:Class>
  <owl:Class rdf:about="http://www.ontotext.com/proton/protonext#CarModel">
    <rdfs:subClassOf rdf:resource="http://www.ontotext.com/proton/protontop#ProductModel"/>
    <rdfs:label xml:lang="en">Car Model</rdfs:label>
    <rdfs:comment xml:lang="en">A concrete model of a car which determines the main features of any car of this model. For example, Ford-T or BMW Z3.</rdfs:comment>
  </owl:Class>
  <owl:Class rdf:about="http://www.ontotext.com/proton/protonext#Newspaper">
    <rdfs:subClassOf>
      <owl:Class rdf:about="http://www.ontotext.com/proton/protonext#PeriodicalPublication"/>
    </rdfs:subClassOf>
    <rdfs:label xml:lang="en">Newspaper</rdfs:label>
    <rdfs:comment xml:lang="en">A newspaper abstracted from its organizational and ownership aspects as well as from a specific issue or paper body.</rdfs:comment>
  </owl:Class>
  <owl:Class rdf:about="http://www.ontotext.com/proton/protonext#Ramp">
    <rdfs:subClassOf>
      <owl:Class rdf:about="http://www.ontotext.com/proton/protonext#LandRegion"/>
    </rdfs:subClassOf>
    <rdfs:label xml:lang="en">Ramp</rdfs:label>
    <rdfs:comment xml:lang="en">A gentle slope connecting areas of different elevations</rdfs:comment>
  </owl:Class>
  <owl:Class rdf:about="http://www.ontotext.com/proton/protonext#InsuranceCompany">
    <rdfs:subClassOf>
      <owl:Class rdf:about="http://www.ontotext.com/proton/protonext#Company"/>
    </rdfs:subClassOf>
    <rdfs:label xml:lang="en">Insurance Company</rdfs:label>
    <rdfs:comment xml:lang="en">A company providing insurance services agains different dangerous or risky events.</rdfs:comment>
  </owl:Class>
  <owl:Class rdf:about="http://www.ontotext.com/proton/protonext#CanadianFootballTeam">
    <rdfs:subClassOf>
      <owl:Class rdf:about="http://www.ontotext.com/proton/protonext#Team"/>
    </rdfs:subClassOf>
    <rdfs:label xml:lang="en">Canadian Football Team</rdfs:label>
    <rdfs:comment xml:lang="en">Any Canadian Football Team</rdfs:comment>
  </owl:Class>
  <owl:Class rdf:about="http://www.ontotext.com/proton/protonext#ChemicalSubstance">
    <rdfs:subClassOf rdf:resource="http://www.ontotext.com/proton/protontop#Object"/>
    <rdfs:label xml:lang="en">Chemical substance</rdfs:label>
    <rdfs:comment xml:lang="en">Any substance or element that has chemical nature.</rdfs:comment>
  </owl:Class>
  <owl:Class rdf:about="http://www.ontotext.com/proton/protonext#Magazine">
    <rdfs:subClassOf>
      <owl:Class rdf:about="http://www.ontotext.com/proton/protonext#PeriodicalPublication"/>
    </rdfs:subClassOf>
    <rdfs:label xml:lang="en">Magazine</rdfs:label>
    <rdfs:comment xml:lang="en">A periodic paperback publication; "it takes several years before a magazine starts to break even or make money"), WordNet 1.7.1. This includes also journals and digests. The specific issues typically contain a number of different articles.</rdfs:comment>
  </owl:Class>
  <owl:Class rdf:about="http://www.ontotext.com/proton/protonext#Accident">
    <rdfs:subClassOf rdf:resource="http://www.ontotext.com/proton/protontop#Event"/>
    <rdfs:label xml:lang="en">Accident</rdfs:label>
  </owl:Class>
  <owl:Class rdf:about="http://www.ontotext.com/proton/protonext#Bacteria">
    <rdfs:subClassOf rdf:resource="http://www.ontotext.com/proton/protonext#LivingObject"/>
    <rdfs:label xml:lang="en">Bacteria</rdfs:label>
    <rdfs:comment xml:lang="en">Bacteria is a single-celled, prokaryote microorganisms, typically a few micrometres in length (Wikipedia)</rdfs:comment>
  </owl:Class>
  <owl:Class rdf:about="http://www.ontotext.com/proton/protonext#WaterCurrent">
    <rdfs:subClassOf>
      <owl:Class rdf:about="http://www.ontotext.com/proton/protonext#WaterRegion"/>
    </rdfs:subClassOf>
    <rdfs:label xml:lang="en">Current</rdfs:label>
    <rdfs:comment xml:lang="en">A net transport of ocean water along a definable path. http://www.eionet.europa.eu/gemet/concept/5792 NIMA GNS designator H.CRNT.</rdfs:comment>
  </owl:Class>
  <owl:Class rdf:about="http://www.ontotext.com/proton/protonext#ProgrammingLanguage">
    <rdfs:subClassOf rdf:resource="http://www.ontotext.com/proton/protontop#Abstract"/>
    <rdfs:label xml:lang="en">Programming language</rdfs:label>
    <rdfs:comment xml:lang="en">A formal language for encoding of computer programs.</rdfs:comment>
  </owl:Class>
  <owl:Class rdf:about="http://www.ontotext.com/proton/protonext#Bank">
    <rdfs:subClassOf>
      <owl:Class rdf:about="http://www.ontotext.com/proton/protonext#Building"/>
    </rdfs:subClassOf>
    <rdfs:subClassOf>
      <owl:Class rdf:about="http://www.ontotext.com/proton/protonext#Company"/>
    </rdfs:subClassOf>
    <rdfs:label xml:lang="en">Bank</rdfs:label>
    <rdfs:comment xml:lang="en">A business establishment in which money is kept for saving or commercial purposes or is invested, supplied for loans, or exchanged.</rdfs:comment>
    <rdfs:comment xml:lang="en">A company providing financial services like credits, deposits, etc.</rdfs:comment>
  </owl:Class>
  <owl:Class rdf:about="http://www.ontotext.com/proton/protonext#AcademicJournal">
    <rdfs:subClassOf rdf:resource="http://www.ontotext.com/proton/protonext#Magazine"/>
    <rdfs:label xml:lang="en">Academic journal</rdfs:label>
    <rdfs:comment xml:lang="en">A journal publishing scientific articles</rdfs:comment>
  </owl:Class>
  <owl:Class rdf:about="http://www.ontotext.com/proton/protonext#Announcement">
    <rdfs:subClassOf>
      <owl:Class rdf:about="http://www.ontotext.com/proton/protonext#PublishedMaterial"/>
    </rdfs:subClassOf>
    <rdfs:label xml:lang="en">Announcement</rdfs:label>
    <rdfs:comment xml:lang="en">A formal public statement; "the government made an announcement about the changes in the drug war" ; "a declaration of independence".) WordNet 1.7.1</rdfs:comment>
  </owl:Class>
  <owl:Class rdf:about="http://www.ontotext.com/proton/protonext#Bridge">
    <rdfs:subClassOf>
      <owl:Class rdf:about="http://www.ontotext.com/proton/protonext#TransportFacility"/>
    </rdfs:subClassOf>
    <rdfs:label xml:lang="en">Bridge</rdfs:label>
    <rdfs:comment xml:lang="en">(ADL FT) Structures erected over a depression or obstacle to carry traffic. [USGS Circ 1048] We use this category for covered bridges; for drawbridges; for overpasses; for trestles; and for viaducts. NIMA GNS designator BDG, BDGQ.</rdfs:comment>
  </owl:Class>
  <owl:Class rdf:about="http://www.ontotext.com/proton/protonext#IssueOfPeriodical">
    <rdfs:subClassOf>
      <owl:Class rdf:about="http://www.ontotext.com/proton/protonext#PublishedMaterial"/>
    </rdfs:subClassOf>
    <rdfs:label xml:lang="en">Issue of Periodical</rdfs:label>
    <rdfs:comment xml:lang="en">A specific issue, number, and/or volume of periodical publication such as magazine.</rdfs:comment>
  </owl:Class>
  <owl:Class rdf:about="http://www.ontotext.com/proton/protonext#Whirlpool">
    <rdfs:subClassOf>
      <owl:Class rdf:about="http://www.ontotext.com/proton/protonext#WaterRegion"/>
    </rdfs:subClassOf>
    <rdfs:label xml:lang="en">Whirlpool</rdfs:label>
    <rdfs:comment xml:lang="en">A turbulent, rotating movement of water in a stream. NIMA GNS designator H.WHRL.</rdfs:comment>
  </owl:Class>
  <owl:Class rdf:about="http://www.ontotext.com/proton/protonext#Gulf">
    <rdfs:subClassOf>
      <owl:Class rdf:about="http://www.ontotext.com/proton/protonext#Bay"/>
    </rdfs:subClassOf>
    <rdfs:label xml:lang="en">Gulf</rdfs:label>
    <rdfs:comment xml:lang="en">(ADL FT) Largest of various forms of inlets of the sea; usually larger, more enclosed, and more deeply indented than bays. NIMA GNS designator GULF.</rdfs:comment>
  </owl:Class>
  <owl:Class rdf:about="http://www.ontotext.com/proton/protonext#PowerStation">
    <rdfs:subClassOf>
      <owl:Class rdf:about="http://www.ontotext.com/proton/protonext#Facility"/>
    </rdfs:subClassOf>
    <rdfs:label xml:lang="en">Power station</rdfs:label>
    <rdfs:comment xml:lang="en">Any power station</rdfs:comment>
  </owl:Class>
  <owl:Class rdf:about="http://www.ontotext.com/proton/protonext#TheatrePerformance">
    <rdfs:subClassOf>
      <owl:Class rdf:about="http://www.ontotext.com/proton/protonext#ArtPerformance"/>
    </rdfs:subClassOf>
    <rdfs:label xml:lang="en">Theatre Performance</rdfs:label>
    <rdfs:comment xml:lang="en">An art performance following a stage play.</rdfs:comment>
  </owl:Class>
  <owl:Class rdf:about="http://www.ontotext.com/proton/protonext#SportOrganization">
    <rdfs:subClassOf rdf:resource="http://www.ontotext.com/proton/protontop#Organization"/>
    <rdfs:label xml:lang="en">Sport Organization</rdfs:label>
    <rdfs:comment xml:lang="en">An organization (local, national or international) which main activity is related to one or more sports. Those could be clubs, as well, as all the sorts of federations.</rdfs:comment>
  </owl:Class>
  <owl:Class rdf:about="http://www.ontotext.com/proton/protonext#Dataset">
    <rdfs:subClassOf rdf:resource="http://www.ontotext.com/proton/protontop#InformationResource"/>
    <rdfs:label xml:lang="en">Dataset</rdfs:label>
    <rdfs:comment xml:lang="en">A dataset is information encoded in a defined structure (for example, lists, tables, and databases), intended to be useful for direct machine processing (DCMI Type.) Somehow structured and interrelated body of information, data, or knowledge. This includes databases, knowledge bases, catalogues, registries, specific lists, etc. All tangible aspects (like media or host) are irrelevant for this class - it only considers the abstract information. What can be considered as a single document is outside the scope of this class, although it can be comprehensive in terms of size and structure.</rdfs:comment>
  </owl:Class>
  <owl:Class rdf:about="http://www.ontotext.com/proton/protonext#StockExchangeIndex">
    <rdfs:subClassOf>
      <owl:Class rdf:about="http://www.ontotext.com/proton/protonext#BusinessAbstraction"/>
    </rdfs:subClassOf>
    <rdfs:label xml:lang="en">Stock Exchange Index</rdfs:label>
    <rdfs:comment xml:lang="en">A stock exchange/market index is a method of measuring a section of the stock market. (Wikipedia)</rdfs:comment>
  </owl:Class>
  <owl:Class rdf:about="http://www.ontotext.com/proton/protonext#MineSite">
    <rdfs:subClassOf>
      <owl:Class rdf:about="http://www.ontotext.com/proton/protonext#Facility"/>
    </rdfs:subClassOf>
    <rdfs:label xml:lang="en">Mine Site</rdfs:label>
    <rdfs:comment xml:lang="en">(ADL FT) Places or areas from which commercial minerals are or were removed by excavation from the Earth. [Adapted from USGS Feature Class Definitions &lt;http://mapping.usgs.gov/www/ti/GNIS/gnis_users_guide_appendixc.html&gt;] We use this category for adits (mine sites); for chrome mines; for coal mines; for collieries; for copper mines; for diatomite mines; for gold mines; for gravel pits; for iron mines; for lead mines; for mine entrances; for mine shafts; for mines; for mining areas; for mining camps; for nickel mines; for open pit mines; for placer mines; for quarries; for salt mines; for strip mines; and for tin mines. NIMA GNS designators MN, MNA, MNAU, MNC, MNCR, MNDT, MNCU, MNFE, MNN, MNNI, MNPB, MNPL. MNQ, MNSN.</rdfs:comment>
  </owl:Class>
  <owl:Class rdf:about="http://www.ontotext.com/proton/protonext#Spacecraft">
    <rdfs:subClassOf>
      <owl:Class rdf:about="http://www.ontotext.com/proton/protonext#Vehicle"/>
    </rdfs:subClassOf>
    <rdfs:label xml:lang="en">Spacecraft</rdfs:label>
    <rdfs:comment xml:lang="en">[WN1.7] Space vehicle - a craft capable of traveling in outer space; technically a satellite around the sun.</rdfs:comment>
  </owl:Class>
  <owl:Class rdf:about="http://www.ontotext.com/proton/protonext#SportsLeague">
    <rdfs:subClassOf rdf:resource="http://www.ontotext.com/proton/protonext#SportOrganization"/>
    <rdfs:label xml:lang="en">Sports League</rdfs:label>
    <rdfs:comment xml:lang="en">Any sports league, a group of sports teams or individual athletes that compete against each other in a specific sport. (Wikipedia)</rdfs:comment>
  </owl:Class>
  <owl:Class rdf:about="http://www.ontotext.com/proton/protonext#FishingArea">
    <rdfs:subClassOf>
      <owl:Class rdf:about="http://www.ontotext.com/proton/protonext#WaterRegion"/>
    </rdfs:subClassOf>
    <rdfs:label xml:lang="en">Fishing Area</rdfs:label>
    <rdfs:comment xml:lang="en">A bank or area where fishermen go to catch fish. NIMA GNS designator H.FISH.</rdfs:comment>
  </owl:Class>
  <owl:Class rdf:about="http://www.ontotext.com/proton/protonext#Waterfalls">
    <rdfs:subClassOf>
      <owl:Class rdf:about="http://www.ontotext.com/proton/protonext#LandRegion"/>
    </rdfs:subClassOf>
    <rdfs:label xml:lang="en">Waterfalls</rdfs:label>
    <rdfs:comment xml:lang="en">(ADL FT) Perpendicular or very steep falls of water in the course of a stream. ... We use this category for cascades; for cataracts; and for falls. NIMA GNS designator FLLS, FLLSX</rdfs:comment>
  </owl:Class>
  <owl:Class rdf:about="http://www.ontotext.com/proton/protonext#Car">
    <rdfs:subClassOf>
      <owl:Class rdf:about="http://www.ontotext.com/proton/protonext#Vehicle"/>
    </rdfs:subClassOf>
    <rdfs:label xml:lang="en">Car</rdfs:label>
    <rdfs:comment xml:lang="en">Any automoabile car.</rdfs:comment>
  </owl:Class>
  <owl:Class rdf:about="http://www.ontotext.com/proton/protonext#Facility">
    <rdfs:subClassOf rdf:resource="http://www.ontotext.com/proton/protontop#Location"/>
    <rdfs:label xml:lang="en">Facility</rdfs:label>
    <rdfs:comment xml:lang="en">(ADL FT: Manmade Features, no def) Any regions and locations determined artificially, as a result of human activity. Many of the ADL sub-classes are omitted. NIMA GNS - no direct equivalent, although many sub-types are defined as classes (S, R) and designators.</rdfs:comment>
  </owl:Class>
  <owl:Class rdf:about="http://www.ontotext.com/proton/protonext#Mention">
    <rdfs:subClassOf rdf:resource="http://www.ontotext.com/proton/protontop#InformationResource"/>
    <rdfs:label>Section</rdfs:label>
    <rdfs:comment xml:lang="en">An area of a document that can be considered a mention of something.</rdfs:comment>
  </owl:Class>
  <owl:Class rdf:about="http://www.ontotext.com/proton/protonext#Monument">
    <rdfs:subClassOf rdf:resource="http://www.ontotext.com/proton/protonext#Facility"/>
    <rdfs:label xml:lang="en">Monument</rdfs:label>
    <rdfs:comment xml:lang="en">(ADL FT) Structures erected as memorials. [Adapted from American Heritage Dic. of the English Language, 4th ed.] We use this category for cairns; for landmarks (monuments); for memorials; for national monuments; for pyramids; for shrines; for statues; and for tombs. NIMA GNS designators MNMT, PYR, PYRS, CARN.</rdfs:comment>
  </owl:Class>
  <owl:Class rdf:about="http://www.ontotext.com/proton/protonext#RegionMention">
    <rdfs:subClassOf rdf:resource="http://www.ontotext.com/proton/protonext#Mention"/>
    <rdfs:label>Region Mention</rdfs:label>
  </owl:Class>
  <owl:Class rdf:about="http://www.ontotext.com/proton/protonext#Genre">
    <rdfs:subClassOf rdf:resource="http://www.ontotext.com/proton/protontop#Abstract"/>
    <rdfs:label xml:lang="en">Genre</rdfs:label>
    <rdfs:comment xml:lang="en">Any Genre. Denotes any category of literature as well as various other forms of art or culture, e.g., music, based on some loose set of stylistic criteria. Genres are formed by conventions that change over time as new genres are invented and the use of old ones are discontinued. (Wikipedia)</rdfs:comment>
  </owl:Class>
  <owl:Class rdf:about="http://www.ontotext.com/proton/protonext#LawFirm">
    <rdfs:subClassOf>
      <owl:Class rdf:about="http://www.ontotext.com/proton/protonext#Company"/>
    </rdfs:subClassOf>
    <rdfs:label xml:lang="en">Law firm</rdfs:label>
    <rdfs:comment xml:lang="en">A law firm is a business entity formed by one or more lawyers to engage in the practice of law. The primary service provided by a law firm is to advise clients (individuals or corporations) about their legal rights and responsibilities, and to represent their clients in civil or criminal cases, business transactions, and other matters in which legal advice and other assistance are sought. DBPedia</rdfs:comment>
  </owl:Class>
  <owl:Class rdf:about="http://www.ontotext.com/proton/protonext#Coast">
    <rdfs:subClassOf>
      <owl:Class rdf:about="http://www.ontotext.com/proton/protonext#LandRegion"/>
    </rdfs:subClassOf>
    <rdfs:label xml:lang="en">Coast</rdfs:label>
    <rdfs:comment xml:lang="en">(ADL FT: Coastal Zones) Strips of land (of indefinite width) that extend from the low-tide line inland to the first major change in landform features. [Adapted from Glossary of Geology, 4th ed.] We use this category for coastal plains; for coasts; for intertidal zones; for offshore areas; for shorelines; and for shores. NIMA GNS designators CST, SHOR.</rdfs:comment>
  </owl:Class>
  <owl:Class rdf:about="http://www.ontotext.com/proton/protonext#RecurringEvent">
    <rdfs:subClassOf rdf:resource="http://www.ontotext.com/proton/protontop#Happening"/>
    <rdfs:label xml:lang="en">Recurring Event</rdfs:label>
    <rdfs:comment xml:lang="en">Recurring sequence of events, such as Olympic Games, etc..</rdfs:comment>
  </owl:Class>
  <owl:Class rdf:about="http://www.ontotext.com/proton/protonext#RadioStation">
    <rdfs:subClassOf>
      <owl:Class rdf:about="http://www.ontotext.com/proton/protonext#MediaBrand"/>
    </rdfs:subClassOf>
    <rdfs:label xml:lang="en">Radio Station</rdfs:label>
    <rdfs:comment xml:lang="en">A brand of a radio station.</rdfs:comment>
  </owl:Class>
  <owl:Class rdf:about="http://www.ontotext.com/proton/protonext#SoftballLeague">
    <rdfs:subClassOf rdf:resource="http://www.ontotext.com/proton/protonext#SportsLeague"/>
    <rdfs:label xml:lang="en">Softball League</rdfs:label>
    <rdfs:comment xml:lang="en">Any Softball league</rdfs:comment>
  </owl:Class>
  <owl:Class rdf:about="http://www.ontotext.com/proton/protonext#PeriodicalPublication">
    <rdfs:subClassOf>
      <owl:Class rdf:about="http://www.ontotext.com/proton/protonext#MediaBrand"/>
    </rdfs:subClassOf>
    <rdfs:label xml:lang="en">Periodical Publication</rdfs:label>
    <rdfs:comment xml:lang="en">A periodical publication, disregarding its specific issues, numbers, volumes, etc.</rdfs:comment>
  </owl:Class>
  <owl:Class rdf:about="http://www.ontotext.com/proton/protonext#GovernmentBuilding">
    <rdfs:subClassOf>
      <owl:Class rdf:about="http://www.ontotext.com/proton/protonext#Building"/>
    </rdfs:subClassOf>
    <rdfs:label xml:lang="en">Government Building</rdfs:label>
    <rdfs:comment xml:lang="en">A government building, a building which serves the government, or where government officials work.</rdfs:comment>
  </owl:Class>
  <owl:Class rdf:about="http://www.ontotext.com/proton/protonext#FictionalCharacter">
    <rdfs:subClassOf rdf:resource="http://www.ontotext.com/proton/protontop#Person"/>
    <rdfs:label xml:lang="en">Fictional Character</rdfs:label>
    <rdfs:comment xml:lang="en">The characters in fictional artwork like movies, books, etc</rdfs:comment>
  </owl:Class>
  <owl:Class rdf:about="http://www.ontotext.com/proton/protonext#Capital">
    <rdfs:subClassOf>
      <owl:Class rdf:about="http://www.ontotext.com/proton/protonext#City"/>
    </rdfs:subClassOf>
    <rdfs:label xml:lang="en">Capital</rdfs:label>
    <rdfs:comment xml:lang="en">(ADL FT) Towns or cities that are the official seats of government in a political entity, such as a state or nation. [American Heritage Dic. of the English Language, 4th ed.] We use this category for county seats; for national capitals; and for state capitals. NIMA GNS designators PPLC, PPLA</rdfs:comment>
  </owl:Class>
  <owl:Class rdf:about="http://www.ontotext.com/proton/protonext#SeaTrough">
    <rdfs:subClassOf>
      <owl:Class rdf:about="http://www.ontotext.com/proton/protonext#LandRegion"/>
    </rdfs:subClassOf>
    <rdfs:label xml:lang="en">Trough</rdfs:label>
    <rdfs:comment xml:lang="en">A long depression of the sea floor characteristically flat bottomed and steep sided, and normally shallower than a trench</rdfs:comment>
  </owl:Class>
  <owl:Class rdf:about="http://www.ontotext.com/proton/protonext#Stream">
    <rdfs:subClassOf>
      <owl:Class rdf:about="http://www.ontotext.com/proton/protonext#WaterRegion"/>
    </rdfs:subClassOf>
    <rdfs:label xml:lang="en">Stream</rdfs:label>
    <rdfs:comment xml:lang="en">(ADL FT) Linear bodies of water flowing on the Earth's surface. We use this category for anabranches; for brooks; for burns (hydrographic); for confluences; for creeks; for distributaries; for dry stream beds; for forks (physiographic features); for intermittent streams; for lost rivers; for meanders; for stream bends; for stream mouths; for tidal creeks; for tributaries; and for watercourses. NIMA GNS designators STM, STMA, STMB, STMC, STMD, STMH, STMI, STMIX, STMM, STMQ, STMS, STMSB, STMX</rdfs:comment>
  </owl:Class>
  <owl:Class rdf:about="http://www.ontotext.com/proton/protonext#UrbanDistrict">
    <rdfs:subClassOf>
      <owl:Class rdf:about="http://www.ontotext.com/proton/protonext#PoliticalRegion"/>
    </rdfs:subClassOf>
    <rdfs:subClassOf>
      <owl:Class rdf:about="http://www.ontotext.com/proton/protonext#PopulatedPlace"/>
    </rdfs:subClassOf>
    <rdfs:label xml:lang="en">Urban District</rdfs:label>
    <rdfs:comment xml:lang="en">(ADL FT: Countries, 3rd order divisions) Minor civil units. [USGS Circ 1048] We use this category for barrios; for precincts; for third-order administrative divisions; and for townships. NIMA GNS designator ADM3.</rdfs:comment>
  </owl:Class>
  <owl:Class rdf:about="http://www.ontotext.com/proton/protonext#RailroadFacility">
    <rdfs:subClassOf>
      <owl:Class rdf:about="http://www.ontotext.com/proton/protonext#TransportFacility"/>
    </rdfs:subClassOf>
    <rdfs:label xml:lang="en">Railroad Facility</rdfs:label>
    <rdfs:comment xml:lang="en">(ADL FT: Railroad Features) We use this category for metro rail stations; for railroad junctions; for railroad sidings; for railroad spurs; for railroad stations; for railroad stops; for railroad switches; for railroad yards; for railways; for subway stations; for switches (railroad); and for tramways. NIMA GNS designator RJCT, RR, RRQ, RSD, RSGNL, RSTN, RSTNQ, RSTP, RSTPQ, RYD.</rdfs:comment>
  </owl:Class>
  <owl:Class rdf:about="http://www.ontotext.com/proton/protonext#FestivalOccurrence">
    <rdfs:subClassOf rdf:resource="http://www.ontotext.com/proton/protontop#Event"/>
    <rdfs:label xml:lang="en">Festival Held at a Particular Time</rdfs:label>
    <rdfs:comment xml:lang="en">An occurrence of a Festival or holiday, Sofia Film Festival 2011, Christmas of 2010 or St. Valentine's Day of 2011.</rdfs:comment>
  </owl:Class>
  <owl:Class rdf:about="http://www.ontotext.com/proton/protonext#BroadcastNetwork">
    <rdfs:subClassOf>
      <owl:Class rdf:about="http://www.ontotext.com/proton/protonext#Broadcaster"/>
    </rdfs:subClassOf>
    <rdfs:label xml:lang="en">Broadcast network</rdfs:label>
    <rdfs:comment xml:lang="en">A broadcast network is an organization, such as a corporation or other voluntary association, that provides live television or recorded content, such as movies, newscasts, sports, Public affairs programming, and other television programs for broadcast over a group of radio stations or television stations. Wikipedia</rdfs:comment>
  </owl:Class>
  <owl:Class rdf:about="http://www.ontotext.com/proton/protonext#NaturalPhenomenon">
    <rdfs:subClassOf rdf:resource="http://www.ontotext.com/proton/protontop#Abstract"/>
    <rdfs:label xml:lang="en">Natural Phenomenon</rdfs:label>
    <rdfs:comment xml:lang="en">Such as particular disease, the Gulfstream and other similar natural abstractions. The particular events or objects which could instantiate an abstract natural phenomena (i.e. specific sickness event caused by a disease) are not instances of this class.</rdfs:comment>
  </owl:Class>
  <owl:Class rdf:about="http://www.ontotext.com/proton/protonext#Profile">
    <rdfs:subClassOf rdf:resource="http://www.ontotext.com/proton/protontop#InformationResource"/>
    <rdfs:label>Profile</rdfs:label>
  </owl:Class>
  <owl:Class rdf:about="http://www.ontotext.com/proton/protonext#Mammal">
    <rdfs:subClassOf>
      <owl:Class rdf:about="http://www.ontotext.com/proton/protonext#Animal"/>
    </rdfs:subClassOf>
    <rdfs:label xml:lang="en">Mammal</rdfs:label>
    <rdfs:comment xml:lang="en">Mammals are members of a class of air-breathing vertebrate animals characterized by the possession of hair, three middle ear bones, and mammary glands functional in mothers with young. Most mammals also possess sweat glands and specialized teeth, and the largest group of mammals, the placentals, have a placenta which feeds the offspring during gestation. (Wikipedia)</rdfs:comment>
  </owl:Class>
  <owl:Class rdf:about="http://www.ontotext.com/proton/protonext#Sport">
    <rdfs:subClassOf>
      <owl:Class rdf:about="http://www.ontotext.com/proton/protonext#SocialAbstraction"/>
    </rdfs:subClassOf>
    <rdfs:label xml:lang="en">Sport</rdfs:label>
    <rdfs:comment xml:lang="en">A specific type of sport game</rdfs:comment>
  </owl:Class>
  <owl:Class rdf:about="http://www.ontotext.com/proton/protonext#OfficialPosition">
    <rdfs:subClassOf rdf:resource="http://www.ontotext.com/proton/protontop#JobPosition"/>
    <rdfs:label xml:lang="en">Official Position</rdfs:label>
    <rdfs:comment xml:lang="en">A job position having a representative function with respect to an organization. Usually this is a position within a governmental organization.</rdfs:comment>
  </owl:Class>
  <owl:Class rdf:about="http://www.ontotext.com/proton/protonext#Man">
    <rdfs:subClassOf>
      <owl:Class rdf:about="http://www.ontotext.com/proton/protonext#Human"/>
    </rdfs:subClassOf>
    <rdfs:subClassOf rdf:resource="http://www.ontotext.com/proton/protontop#Person"/>
    <rdfs:label xml:lang="en">Man</rdfs:label>
    <rdfs:comment xml:lang="en">A male human.</rdfs:comment>
  </owl:Class>
  <owl:Class rdf:about="http://www.ontotext.com/proton/protonext#Possession">
    <rdfs:subClassOf>
      <owl:Class rdf:about="http://www.ontotext.com/proton/protonext#BusinessAbstraction"/>
    </rdfs:subClassOf>
    <rdfs:label xml:lang="en">Possessions</rdfs:label>
    <rdfs:comment xml:lang="en">Any property, e.g. possessions, the situation of owning an object.</rdfs:comment>
  </owl:Class>
  <owl:Class rdf:about="http://www.ontotext.com/proton/protonext#Rapids">
    <rdfs:subClassOf>
      <owl:Class rdf:about="http://www.ontotext.com/proton/protonext#WaterRegion"/>
    </rdfs:subClassOf>
    <rdfs:label xml:lang="en">Rapids</rdfs:label>
    <rdfs:comment xml:lang="en">A turbulent section of a stream associated with a steep, irregular stream bed. NIMA GNS designator H.RPDS.</rdfs:comment>
  </owl:Class>
  <owl:Class rdf:about="http://www.ontotext.com/proton/protonext#Plant">
    <rdfs:subClassOf rdf:resource="http://www.ontotext.com/proton/protonext#LivingObject"/>
    <rdfs:label xml:lang="en">Plant</rdfs:label>
    <rdfs:comment xml:lang="en">Plants are living organisms. They include familiar organisms such as trees, flowers, herbs, bushes, grasses, vines, ferns, mosses, and green algae. (Wikipedia)</rdfs:comment>
  </owl:Class>
  <owl:Class rdf:about="http://www.ontotext.com/proton/protonext#PerformanceSite">
    <rdfs:subClassOf>
      <owl:Class rdf:about="http://www.ontotext.com/proton/protonext#Building"/>
    </rdfs:subClassOf>
    <rdfs:subClassOf>
      <owl:Class rdf:about="http://www.ontotext.com/proton/protonext#RecreationalFacility"/>
    </rdfs:subClassOf>
    <rdfs:label xml:lang="en">Performance Site</rdfs:label>
    <rdfs:comment xml:lang="en">Buildings where cultural events are presented before an audience. We use this category for amphitheaters; for amphitheatres; for auditoriums; for bowls (performance); for coliseums; for concert halls; for opera houses; for playhouses; for recital halls; for stages (performance); for symphony halls; for theaters; and for theatres. NIMA GNS designator AMTH.</rdfs:comment>
  </owl:Class>
  <owl:Class rdf:about="http://www.ontotext.com/proton/protonext#Glacier">
    <rdfs:subClassOf>
      <owl:Class rdf:about="http://www.ontotext.com/proton/protonext#LandRegion"/>
    </rdfs:subClassOf>
    <rdfs:label xml:lang="en">Glacier</rdfs:label>
    <rdfs:comment xml:lang="en">A mass of ice, usually at high latitudes or high elevations, with sufficient thickness to flow away from the source area in lobes, tongues, or masses</rdfs:comment>
  </owl:Class>
  <owl:Class rdf:about="http://www.ontotext.com/proton/protonext#Game">
    <rdfs:subClassOf>
      <owl:Class rdf:about="http://www.ontotext.com/proton/protonext#Activity"/>
    </rdfs:subClassOf>
    <rdfs:label xml:lang="en">Game</rdfs:label>
    <rdfs:comment xml:lang="en">Game. Activity involving participants usually divided in teams, which obeys particualr rules, and has often a winner.</rdfs:comment>
  </owl:Class>
  <owl:Class rdf:about="http://www.ontotext.com/proton/protonext#Animal">
    <rdfs:subClassOf rdf:resource="http://www.ontotext.com/proton/protonext#LivingObject"/>
    <rdfs:label xml:lang="en">Animal</rdfs:label>
    <rdfs:comment xml:lang="en">Animals are a major group of multicellular, eukaryotic organisms. Their body plan eventually becomes fixed as they develop. Most animals are motile. (Wikipedia)</rdfs:comment>
  </owl:Class>
  <owl:Class rdf:about="http://www.ontotext.com/proton/protonext#Muscle">
    <rdfs:subClassOf rdf:resource="http://www.ontotext.com/proton/protonext#BodyPart"/>
    <rdfs:label xml:lang="en">Muscle</rdfs:label>
    <rdfs:comment xml:lang="en">Any muscle of a body.</rdfs:comment>
  </owl:Class>
  <owl:Class rdf:about="http://www.ontotext.com/proton/protonext#College">
    <rdfs:subClassOf>
      <owl:Class rdf:about="http://www.ontotext.com/proton/protonext#EducationalOrganization"/>
    </rdfs:subClassOf>
    <rdfs:label xml:lang="en">College</rdfs:label>
    <rdfs:comment xml:lang="en">An education organization between the school and the university. In some cases it is a part of university.</rdfs:comment>
    <rdfs:comment xml:lang="en">College</rdfs:comment>
  </owl:Class>
  <owl:Class rdf:about="http://www.ontotext.com/proton/protonext#SportGame">
    <rdfs:subClassOf rdf:resource="http://www.ontotext.com/proton/protonext#Game"/>
    <rdfs:subClassOf>
      <owl:Class rdf:about="http://www.ontotext.com/proton/protonext#SportEvent"/>
    </rdfs:subClassOf>
    <rdfs:label xml:lang="en">Sport Game</rdfs:label>
    <rdfs:comment xml:lang="en">A sport game is any instance of a sport event, where teams or individuals gather to play according to particular predetermined rules, such as soccer match, tennis match, car race, etc. It can also denote the activity of playing a particular sport game.</rdfs:comment>
  </owl:Class>
  <owl:Class rdf:about="http://www.ontotext.com/proton/protonext#MountainRange">
    <rdfs:subClassOf>
      <owl:Class rdf:about="http://www.ontotext.com/proton/protonext#Mountain"/>
    </rdfs:subClassOf>
    <rdfs:label xml:lang="en">Mountain Range</rdfs:label>
    <rdfs:comment xml:lang="en">(ADL FT) (a) Chains of hills or mountains; (b) somewhat linear, complex mountainous or hilly areas. ... We use this category for ranges (physiographic); and for sierra. NIMA GNS designator RNGU.</rdfs:comment>
  </owl:Class>
  <owl:Class rdf:about="http://www.ontotext.com/proton/protonext#LocalCapital">
    <rdfs:subClassOf rdf:resource="http://www.ontotext.com/proton/protonext#Capital"/>
    <rdfs:label xml:lang="en">Local Capital</rdfs:label>
    <rdfs:comment xml:lang="en">A capital of a Province or smaller administrative region. NIMA GNS designator PPLA.</rdfs:comment>
  </owl:Class>
  <owl:Class rdf:about="http://www.ontotext.com/proton/protonext#StockExchange">
    <rdfs:subClassOf rdf:resource="http://www.ontotext.com/proton/protontop#Organization"/>
    <rdfs:label xml:lang="en">Stock Exchange</rdfs:label>
    <rdfs:comment xml:lang="en">Stock Exchange where public companies are traded, e. g. Nasdaq, NYSE, etc.</rdfs:comment>
  </owl:Class>
  <owl:Class rdf:about="http://www.ontotext.com/proton/protonext#Art">
    <rdfs:subClassOf>
      <owl:Class rdf:about="http://www.ontotext.com/proton/protonext#SocialAbstraction"/>
    </rdfs:subClassOf>
    <rdfs:label xml:lang="en">Art</rdfs:label>
    <rdfs:comment xml:lang="en">Art is the product or process of deliberately arranging items (often with symbolic significance) in a way that influences and affects one or more of the senses, emotions, and intellect. Wikipedia.</rdfs:comment>
  </owl:Class>
  <owl:Class rdf:about="http://www.ontotext.com/proton/protonext#Restaurant">
    <rdfs:subClassOf>
      <owl:Class rdf:about="http://www.ontotext.com/proton/protonext#Building"/>
    </rdfs:subClassOf>
    <rdfs:label xml:lang="en">Restaurant</rdfs:label>
    <rdfs:comment xml:lang="en">Any restaurant, a place where food, drink and dessert to customers is prepared and served in return for money. (Wikipedia)</rdfs:comment>
  </owl:Class>
  <owl:Class rdf:about="http://www.ontotext.com/proton/protonext#FInlet">
    <rdfs:subClassOf>
      <owl:Class rdf:about="http://www.ontotext.com/proton/protonext#WaterRegion"/>
    </rdfs:subClassOf>
    <rdfs:label xml:lang="en">Former Inlet</rdfs:label>
    <rdfs:comment xml:lang="en">An inlet which has been filled in, or blocked by deposits</rdfs:comment>
  </owl:Class>
  <owl:Class rdf:about="http://www.ontotext.com/proton/protonext#EntertainmentCompany">
    <rdfs:subClassOf>
      <owl:Class rdf:about="http://www.ontotext.com/proton/protonext#Company"/>
    </rdfs:subClassOf>
    <rdfs:label xml:lang="en">Entertainment Company</rdfs:label>
    <rdfs:comment xml:lang="en">Any Entertainment Company, a company involved in the entertainment business, e.g. Warner Brothers, MTV, Lido, etc.</rdfs:comment>
  </owl:Class>
  <owl:Class rdf:about="http://www.ontotext.com/proton/protonext#Percent">
    <rdfs:subClassOf rdf:resource="http://www.ontotext.com/proton/protontop#Number"/>
    <rdfs:label xml:lang="en">Percent</rdfs:label>
    <rdfs:comment xml:lang="en">A specific percent value</rdfs:comment>
  </owl:Class>
  <owl:Class rdf:about="http://www.ontotext.com/proton/protonext#MeetingProceedings">
    <rdfs:subClassOf>
      <owl:Class rdf:about="http://www.ontotext.com/proton/protonext#Book"/>
    </rdfs:subClassOf>
    <rdfs:subClassOf>
      <owl:Class rdf:about="http://www.ontotext.com/proton/protonext#ResourceCollection"/>
    </rdfs:subClassOf>
    <rdfs:label xml:lang="en">Meeting Proceedings</rdfs:label>
    <rdfs:comment xml:lang="en">A collection of articles or presentations published as a book.</rdfs:comment>
  </owl:Class>
  <owl:Class rdf:about="http://www.ontotext.com/proton/protonext#Protein">
    <rdfs:subClassOf>
      <owl:Class rdf:about="http://www.ontotext.com/proton/protonext#BiologicalSubstance"/>
    </rdfs:subClassOf>
    <rdfs:label xml:lang="en">Protein</rdfs:label>
    <rdfs:comment xml:lang="en">Denotes any protein as a biological substance.</rdfs:comment>
  </owl:Class>
  <owl:Class rdf:about="http://www.ontotext.com/proton/protonext#Arena">
    <rdfs:subClassOf>
      <owl:Class rdf:about="http://www.ontotext.com/proton/protonext#Building"/>
    </rdfs:subClassOf>
    <rdfs:label xml:lang="en">Arena</rdfs:label>
    <rdfs:comment xml:lang="en">Any arena</rdfs:comment>
  </owl:Class>
  <owl:Class rdf:about="http://www.ontotext.com/proton/protonext#Nationality">
    <rdfs:subClassOf rdf:resource="http://www.ontotext.com/proton/protontop#Abstract"/>
    <rdfs:label>Nationality</rdfs:label>
    <rdfs:comment xml:lang="en">Any nationality. In most cases it is connected with a country name, but there are notionalities without countries - Kurd, etc.</rdfs:comment>
  </owl:Class>
  <owl:Class rdf:about="http://www.ontotext.com/proton/protonext#Celebrity">
    <rdfs:subClassOf rdf:resource="http://www.ontotext.com/proton/protontop#SocialPosition"/>
    <rdfs:label xml:lang="en">Celebrity</rdfs:label>
    <rdfs:comment xml:lang="en">The situation of holding a position in a society as celebrity.</rdfs:comment>
  </owl:Class>
  <owl:Class rdf:about="http://www.ontotext.com/proton/protonext#RailroadTunnel">
    <rdfs:subClassOf rdf:resource="http://www.ontotext.com/proton/protonext#RailroadFacility"/>
    <rdfs:subClassOf>
      <owl:Class rdf:about="http://www.ontotext.com/proton/protonext#Tunnel"/>
    </rdfs:subClassOf>
    <rdfs:label xml:lang="en">Railroad Tunnel</rdfs:label>
    <rdfs:comment xml:lang="en">A tunnel for trains. NIMA GNS designator RTNL.</rdfs:comment>
  </owl:Class>
  <owl:Class rdf:about="http://www.ontotext.com/proton/protonext#ArtificialSatellite">
    <rdfs:subClassOf>
      <owl:Class rdf:about="http://www.ontotext.com/proton/protonext#Satellite"/>
    </rdfs:subClassOf>
    <rdfs:label xml:lang="en">Artificial Satellite</rdfs:label>
    <rdfs:comment xml:lang="en">A satellite created by humans</rdfs:comment>
  </owl:Class>
  <owl:Class rdf:about="http://www.ontotext.com/proton/protonext#HydrographicStructure">
    <rdfs:subClassOf rdf:resource="http://www.ontotext.com/proton/protonext#Facility"/>
    <rdfs:label xml:lang="en">Hydrographic Structure</rdfs:label>
    <rdfs:comment xml:lang="en">(ADL FT) For constructed bodies of water. For natural water bodies, use 'hydrographic features'. We use this category for boat landings; for boat launches; for boat ramps; for sluices; and for water mills. Many sub-classes omitted; those considered are also made sub-classes of WaterRegion. NIMA GNS ... no direct equivalent.</rdfs:comment>
  </owl:Class>
  <owl:Class rdf:about="http://www.ontotext.com/proton/protonext#PoloLeague">
    <rdfs:subClassOf rdf:resource="http://www.ontotext.com/proton/protonext#SportsLeague"/>
    <rdfs:label xml:lang="en">Polo League</rdfs:label>
    <rdfs:comment xml:lang="en">Any Polo league</rdfs:comment>
  </owl:Class>
  <owl:Class rdf:about="http://www.ontotext.com/proton/protonext#EmbryoBodyPart">
    <rdfs:subClassOf rdf:resource="http://www.ontotext.com/proton/protonext#BodyPart"/>
    <rdfs:label xml:lang="en">Embryo Body Part</rdfs:label>
    <rdfs:comment xml:lang="en">Embryology is a science that studies the development of the embryo. This class denotes different composing substances/elements of the embryo and related body parts, and hence is referred to as a body part. It is inspired form DBPedia Embryology/AnatomicalStructure, which has instances as Blastocyst, Amniotic cavity, Vitelline membrane, etc.</rdfs:comment>
  </owl:Class>
  <owl:Class rdf:about="http://www.ontotext.com/proton/protonext#Month">
    <rdfs:subClassOf rdf:resource="http://www.ontotext.com/proton/protontop#TimeInterval"/>
    <rdfs:label xml:lang="en">Month</rdfs:label>
    <rdfs:comment xml:lang="en">A specific month, like Dec 2000, as a time period.</rdfs:comment>
  </owl:Class>
  <owl:Class rdf:about="http://www.ontotext.com/proton/protonext#GovernmentOrganization">
    <rdfs:subClassOf rdf:resource="http://www.ontotext.com/proton/protontop#Organization"/>
    <rdfs:label xml:lang="en">Government Organization</rdfs:label>
    <rdfs:comment xml:lang="en">The government of a country, i.e. the authorized country administration, without account for a specific government elected and being in power for some period. This notion of government groups all the administration, including any sort of ministries, agencies, commissions, etc.</rdfs:comment>
  </owl:Class>
  <owl:Class rdf:about="http://www.ontotext.com/proton/protonext#Station">
    <rdfs:subClassOf>
      <owl:Class rdf:about="http://www.ontotext.com/proton/protonext#Building"/>
    </rdfs:subClassOf>
    <rdfs:label xml:lang="en">Station</rdfs:label>
    <rdfs:comment xml:lang="en">Any station, a place where busses, trains, sheeps, boats, etc. stop, like railway station, bussstop, etc.</rdfs:comment>
  </owl:Class>
  <owl:Class rdf:about="http://www.ontotext.com/proton/protonext#Confluence">
    <rdfs:subClassOf>
      <owl:Class rdf:about="http://www.ontotext.com/proton/protonext#WaterRegion"/>
    </rdfs:subClassOf>
    <rdfs:label xml:lang="en">Confluence</rdfs:label>
    <rdfs:comment xml:lang="en">in geography, describes the meeting of two or more bodies of water. The opposite of a watershed. NIMA GNS designator H.CNFL.</rdfs:comment>
  </owl:Class>
  <owl:Class rdf:about="http://www.ontotext.com/proton/protonext#Ditch">
    <rdfs:subClassOf>
      <owl:Class rdf:about="http://www.ontotext.com/proton/protonext#Canal"/>
    </rdfs:subClassOf>
    <rdfs:subClassOf rdf:resource="http://www.ontotext.com/proton/protonext#HydrographicStructure"/>
    <rdfs:label xml:lang="en">Ditch</rdfs:label>
    <rdfs:comment xml:lang="en">A ditch is usually defined as a small to moderate depression created to channel water.(Wikipedia). http://www.eionet.europa.eu/gemet/concept/2276. NIMA GNS designators H.DTCH, H.DTCHD, H.DTCHI, H.DTCHM.</rdfs:comment>
  </owl:Class>
  <owl:Class rdf:about="http://www.ontotext.com/proton/protonext#HomePage">
    <rdfs:subClassOf>
      <owl:Class rdf:about="http://www.ontotext.com/proton/protonext#WebPage"/>
    </rdfs:subClassOf>
    <rdfs:label xml:lang="en">Home Page</rdfs:label>
    <rdfs:comment xml:lang="en">The web page address of a page that is considered main for a web cite.</rdfs:comment>
  </owl:Class>
  <owl:Class rdf:about="http://www.ontotext.com/proton/protonext#MediaBrand">
    <rdfs:subClassOf>
      <owl:Class rdf:about="http://www.ontotext.com/proton/protonext#Brand"/>
    </rdfs:subClassOf>
    <rdfs:label xml:lang="en">Media Brand</rdfs:label>
    <rdfs:comment xml:lang="en">A brand of a media company.</rdfs:comment>
  </owl:Class>
  <owl:Class rdf:about="http://www.ontotext.com/proton/protonext#Meeting">
    <rdfs:subClassOf rdf:resource="http://www.ontotext.com/proton/protontop#Event"/>
    <rdfs:label xml:lang="en">Meeting</rdfs:label>
    <rdfs:comment xml:lang="en">A meeting is a gathering of two or more people that has been convened for the purpose of achieving a common goal through verbal interaction, such as sharing information or reaching an agreement. Wikipedia.</rdfs:comment>
  </owl:Class>
  <owl:Class rdf:about="http://www.ontotext.com/proton/protonext#RadioControlledRacingLeague">
    <rdfs:subClassOf rdf:resource="http://www.ontotext.com/proton/protonext#SportsLeague"/>
    <rdfs:label xml:lang="en">Radio Controlled Racing League</rdfs:label>
    <rdfs:comment xml:lang="en">Any Radio Controlled Racing league</rdfs:comment>
  </owl:Class>
  <owl:Class rdf:about="http://www.ontotext.com/proton/protonext#Address">
    <rdfs:subClassOf rdf:resource="http://www.ontotext.com/proton/protontop#ContactInformation"/>
    <rdfs:label xml:lang="en">Address</rdfs:label>
    <rdfs:comment xml:lang="en">Any sort of address, specifying how to locate something somewhere.</rdfs:comment>
  </owl:Class>
  <owl:Class rdf:about="http://www.ontotext.com/proton/protonext#Cleric">
    <rdfs:subClassOf rdf:resource="http://www.ontotext.com/proton/protontop#SocialPosition"/>
    <rdfs:label xml:lang="en">Cleric</rdfs:label>
    <rdfs:comment xml:lang="en">The situation of holding a position in society as cleric.</rdfs:comment>
  </owl:Class>
  <owl:Class rdf:about="http://www.ontotext.com/proton/protonext#Canal">
    <rdfs:subClassOf rdf:resource="http://www.ontotext.com/proton/protonext#HydrographicStructure"/>
    <rdfs:subClassOf>
      <owl:Class rdf:about="http://www.ontotext.com/proton/protonext#WaterRegion"/>
    </rdfs:subClassOf>
    <rdfs:label xml:lang="en">Canal</rdfs:label>
    <rdfs:comment xml:lang="en">(ADL FT) Artificial waterways with no flow or a controlled flow used for navigation (canal), or for draining or irrigating land (ditch). We use this category for canal bends; for canalized streams; for ditch mouths; for ditches; for drainage canals; for drainage ditches; for drains (channels); for flumes (manmade); for irrigation canals; for irrigation ditches; for irrigation systems; for laterals; for navigation canals; and for underground irrigation canals. NIMA GNS designators CNL,CNLA, CNLB, CNLD, CNLI, CNLN, CNLQ, CNLSB, CNLX.</rdfs:comment>
  </owl:Class>
  <owl:Class rdf:about="http://www.ontotext.com/proton/protonext#Zone">
    <rdfs:subClassOf>
      <owl:Class rdf:about="http://www.ontotext.com/proton/protonext#LandRegion"/>
    </rdfs:subClassOf>
    <rdfs:label xml:lang="en">Zone</rdfs:label>
    <rdfs:comment xml:lang="en">A land region defined to play a role. For example, a buffer between two nations in which military presence is minimal or absent or zone around the site of the Chernobyl disaster to protect people from radiation. (NIMA GNS designator A.ZN, A.ZNB.</rdfs:comment>
  </owl:Class>
  <owl:Class rdf:about="http://www.ontotext.com/proton/protonext#MediaProduct">
    <rdfs:subClassOf rdf:resource="http://www.ontotext.com/proton/protontop#ProductModel"/>
    <rdfs:label xml:lang="en">Media Product</rdfs:label>
    <rdfs:comment xml:lang="en">A mass media product (for instance a newspaper) abstracted from its organizational and ownership aspects (i.e. from its publisher) and considered more as a social phenomenon, partly a brand.</rdfs:comment>
  </owl:Class>
  <owl:Class rdf:about="http://www.ontotext.com/proton/protonext#TimeZone">
    <rdfs:subClassOf>
      <owl:Class rdf:about="http://www.ontotext.com/proton/protonext#TemporalAbstraction"/>
    </rdfs:subClassOf>
    <rdfs:label xml:lang="en">Time Zone</rdfs:label>
    <rdfs:comment xml:lang="en">A time zone is a region on Earth that has a uniform standard time for legal, commercial, and social purposes. Wikipedia.</rdfs:comment>
  </owl:Class>
  <owl:Class rdf:about="http://www.ontotext.com/proton/protonext#Tundra">
    <rdfs:subClassOf>
      <owl:Class rdf:about="http://www.ontotext.com/proton/protonext#BiogeographicRegion"/>
    </rdfs:subClassOf>
    <rdfs:label xml:lang="en">Tundra</rdfs:label>
    <rdfs:comment xml:lang="en">(ADL FT) Treeless, level, or gently rolling plains characteristic of arctic or subarctic regions, having a permanently frozen subsoil, and usually supporting low growing vegetation such as lichens, mosses, and stunted shrubs. [USGS Circ 1048] We use this category for Arctic land. NIMA GNS designator TUND, LAND.</rdfs:comment>
  </owl:Class>
  <owl:Class rdf:about="http://www.ontotext.com/proton/protonext#Profession">
    <rdfs:subClassOf>
      <owl:Class rdf:about="http://www.ontotext.com/proton/protonext#SocialFunction"/>
    </rdfs:subClassOf>
    <rdfs:label xml:lang="en">Profession</rdfs:label>
    <rdfs:comment xml:lang="en">A profession is a vocation founded upon specialized educational training. Wikipedia.</rdfs:comment>
  </owl:Class>
  <owl:Class rdf:about="http://www.ontotext.com/proton/protonext#BoxingLeague">
    <rdfs:subClassOf rdf:resource="http://www.ontotext.com/proton/protonext#SportsLeague"/>
    <rdfs:label xml:lang="en">Boxing League</rdfs:label>
    <rdfs:comment xml:lang="en">Any Boxing league</rdfs:comment>
  </owl:Class>
  <owl:Class rdf:about="http://www.ontotext.com/proton/protonext#Band">
    <rdfs:subClassOf rdf:resource="http://www.ontotext.com/proton/protontop#Organization"/>
    <rdfs:label xml:lang="en">Band</rdfs:label>
    <rdfs:comment xml:lang="en">Any band, a group performing music or other activity together.</rdfs:comment>
  </owl:Class>
  <owl:Class rdf:about="http://www.ontotext.com/proton/protonext#EthnicGroup">
    <rdfs:subClassOf rdf:resource="http://www.ontotext.com/proton/protontop#Group"/>
    <rdfs:label xml:lang="en">Ethnic Group</rdfs:label>
    <rdfs:comment xml:lang="en">Any ethnic group. A group of people whose members identify with each other, through a common heritage, often consisting of a common language, a common culture (often including a shared religion) and an ideology that stresses common ancestry or endogamy. (Wikipedia).</rdfs:comment>
  </owl:Class>
  <owl:Class rdf:about="http://www.ontotext.com/proton/protonext#Festival">
    <rdfs:subClassOf rdf:resource="http://www.ontotext.com/proton/protonext#RecurringEvent"/>
    <rdfs:label xml:lang="en">Festival</rdfs:label>
    <rdfs:comment xml:lang="en">Any widely recognized festival or holiday, such as, Christmas or St. Valentine's Day.</rdfs:comment>
  </owl:Class>
  <owl:Class rdf:about="http://www.ontotext.com/proton/protonext#BushLand">
    <rdfs:subClassOf>
      <owl:Class rdf:about="http://www.ontotext.com/proton/protonext#BiogeographicRegion"/>
    </rdfs:subClassOf>
    <rdfs:label xml:lang="en">Bush</rdfs:label>
    <rdfs:comment xml:lang="en">A small clump of conspicuous bushes in an otherwise bare area</rdfs:comment>
  </owl:Class>
  <owl:Class rdf:about="http://www.ontotext.com/proton/protonext#Beacon">
    <rdfs:subClassOf rdf:resource="http://www.ontotext.com/proton/protonext#Facility"/>
    <rdfs:label xml:lang="en">Beacon</rdfs:label>
    <rdfs:comment xml:lang="en">A fixed artificial navigation mark</rdfs:comment>
  </owl:Class>
  <owl:Class rdf:about="http://www.ontotext.com/proton/protonext#SportsFederation">
    <rdfs:subClassOf rdf:resource="http://www.ontotext.com/proton/protonext#SportOrganization"/>
    <rdfs:label xml:lang="en">Sports Federation</rdfs:label>
    <rdfs:comment xml:lang="en">An organization representing which controls the practice of some sport on national, regional or international level.</rdfs:comment>
  </owl:Class>
  <owl:Class rdf:about="http://www.ontotext.com/proton/protonext#Report">
    <rdfs:subClassOf rdf:resource="http://www.ontotext.com/proton/protontop#Document"/>
    <rdfs:label xml:lang="en">Report</rdfs:label>
    <rdfs:comment xml:lang="en">A document describing the result of some event.</rdfs:comment>
  </owl:Class>
  <owl:Class rdf:about="http://www.ontotext.com/proton/protonext#Musical">
    <rdfs:subClassOf rdf:resource="http://www.ontotext.com/proton/protontop#ProductModel"/>
    <rdfs:label xml:lang="en">Musical</rdfs:label>
    <rdfs:comment xml:lang="en">Musical is a form of theatre or movie combining music, songs, spoken dialogue and dance. (Wikipedia)</rdfs:comment>
  </owl:Class>
  <owl:Class rdf:about="http://www.ontotext.com/proton/protonext#LibraryBuilding">
    <rdfs:subClassOf>
      <owl:Class rdf:about="http://www.ontotext.com/proton/protonext#Building"/>
    </rdfs:subClassOf>
    <rdfs:label xml:lang="en">Library</rdfs:label>
    <rdfs:comment xml:lang="en">A building in which library organization is housed.</rdfs:comment>
  </owl:Class>
  <owl:Class rdf:about="http://www.ontotext.com/proton/protonext#Pool">
    <rdfs:subClassOf>
      <owl:Class rdf:about="http://www.ontotext.com/proton/protonext#WaterRegion"/>
    </rdfs:subClassOf>
    <rdfs:label xml:lang="en">Pool</rdfs:label>
    <rdfs:comment xml:lang="en">A small and comparatively still, deep part of a larger body of water. NIMA GNS designator H.POOL, H.POOLI.</rdfs:comment>
  </owl:Class>
  <owl:Class rdf:about="http://www.ontotext.com/proton/protonext#Building">
    <rdfs:subClassOf rdf:resource="http://www.ontotext.com/proton/protonext#Facility"/>
    <rdfs:label xml:lang="en">Building</rdfs:label>
    <rdfs:comment xml:lang="en">(ADL FT) Permanent constructions that are roofed and usually walled. [USGS Circ 1048] We use this category for administrative facilities; for administrative facilities; for animal pounds; for animal shelters; for aquariums; for barns; for border posts; for cabins; for castles; for city halls; for civic centers; for civil buildings; for club houses; for coast guard stations; for commissaries; for community centers; for community houses; for conference facilities; for consulates; for convention centers; for customs houses; for customs posts; for depots; for embassy buildings; for exhibition buildings; for facilities; for facility centers; for fire stations; for firehouses; for forest stations; for government buildings; for guard stations; for halls; for headquarters; for hostels; for hotels; for houses; for inns; for inspection stations; for legation buildings; for lodges; for missions; for motels; for neighborhood centers; for offices; for park headquarters; for patrol posts; for pavilions; for planetariums; for plazas; for police posts; for public buildings; for ranger stations; for restaurants; for shelters; for shops; for stations; for structures; for student unions; for studios; for substations; for taverns; for town halls; for trading posts; for treatment plants; for United States Government establishments; for visitor centers; for walls; and for warehouses NIMA GNS designator BLDG.</rdfs:comment>
  </owl:Class>
  <owl:Class rdf:about="http://www.ontotext.com/proton/protonext#SoccerLeague">
    <rdfs:subClassOf rdf:resource="http://www.ontotext.com/proton/protonext#SportsLeague"/>
    <rdfs:label xml:lang="en">Soccer League</rdfs:label>
    <rdfs:comment xml:lang="en">Any Soccer league</rdfs:comment>
  </owl:Class>
  <owl:Class rdf:about="http://www.ontotext.com/proton/protonext#MilitaryConflict">
    <rdfs:subClassOf rdf:resource="http://www.ontotext.com/proton/protontop#Event"/>
    <rdfs:label xml:lang="en">Military Conflict</rdfs:label>
    <rdfs:comment xml:lang="en">An event of organized, armed, and often prolonged conflict carried on between states, nations, or other parties. Wikipedia.</rdfs:comment>
  </owl:Class>
  <owl:Class rdf:about="http://www.ontotext.com/proton/protonext#Narrows">
    <rdfs:subClassOf>
      <owl:Class rdf:about="http://www.ontotext.com/proton/protonext#WaterRegion"/>
    </rdfs:subClassOf>
    <rdfs:label xml:lang="en">Narrows</rdfs:label>
    <rdfs:comment xml:lang="en">A tidal strait. NIMA GNS designator H.NRWS.</rdfs:comment>
  </owl:Class>
  <owl:Class rdf:about="http://www.ontotext.com/proton/protonext#Ridge">
    <rdfs:subClassOf>
      <owl:Class rdf:about="http://www.ontotext.com/proton/protonext#Mountain"/>
    </rdfs:subClassOf>
    <rdfs:label xml:lang="en">Ridge</rdfs:label>
    <rdfs:comment xml:lang="en">(ADL FT) Elevations with a narrow, elongated crest which can be part of a hill or mountain. ... We use this category for aretes; for beach ridges; for cuestas; for eskers; for hogbacks; for icecap ridges; for rises (seafloor); and for spurs (physiographic). Omitted ADL sub-classes: Drumlin. NIMA GNS designators RDGB, RDGE, RDGG, RDGU, RISU, SPRU, SPUR.</rdfs:comment>
  </owl:Class>
  <owl:Class rdf:about="http://www.ontotext.com/proton/protonext#GeopoliticalOrganization">
    <rdfs:subClassOf rdf:resource="http://www.ontotext.com/proton/protontop#Organization"/>
    <rdfs:label xml:lang="en">Geopolitical Organisation</rdfs:label>
    <rdfs:comment xml:lang="en">Any geopolitical organization, an organization based on geo-political principles.</rdfs:comment>
  </owl:Class>
  <owl:Class rdf:about="http://www.ontotext.com/proton/protonext#MagazineIssue">
    <rdfs:subClassOf rdf:resource="http://www.ontotext.com/proton/protonext#IssueOfPeriodical"/>
    <rdfs:subClassOf>
      <owl:Class rdf:about="http://www.ontotext.com/proton/protonext#ResourceCollection"/>
    </rdfs:subClassOf>
    <rdfs:label xml:lang="en">Magazine Issue</rdfs:label>
    <rdfs:comment xml:lang="en">A specific issue of a magazine, journal or digest.</rdfs:comment>
  </owl:Class>
  <owl:Class rdf:about="http://www.ontotext.com/proton/protonext#Play">
    <rdfs:subClassOf>
      <owl:Class rdf:about="http://www.ontotext.com/proton/protonext#PublishedMaterial"/>
    </rdfs:subClassOf>
    <rdfs:label xml:lang="en">Play</rdfs:label>
    <rdfs:comment xml:lang="en">A play is a form of literature written by a playwright, usually consisting of scripted dialogue between characters, intended for theatrical performance rather than just reading. DBPedia</rdfs:comment>
  </owl:Class>
  <owl:Class rdf:about="http://www.ontotext.com/proton/protonext#TelevisionProduct">
    <rdfs:subClassOf rdf:resource="http://www.ontotext.com/proton/protonext#MediaProduct"/>
    <rdfs:label xml:lang="en">Television Product</rdfs:label>
    <rdfs:comment xml:lang="en">Denotes programms produced in the television and for television airing.</rdfs:comment>
  </owl:Class>
  <owl:Class rdf:about="http://www.ontotext.com/proton/protonext#AgriculturalFacility">
    <rdfs:subClassOf rdf:resource="http://www.ontotext.com/proton/protonext#Facility"/>
    <rdfs:label xml:lang="en">Agricultural Facility</rdfs:label>
    <rdfs:comment xml:lang="en">An agricultural facility; a building and/or tract of land used for improving agriculture</rdfs:comment>
  </owl:Class>
  <owl:Class rdf:about="http://www.ontotext.com/proton/protonext#ResearchArea">
    <rdfs:subClassOf>
      <owl:Class rdf:about="http://www.ontotext.com/proton/protonext#SocialAbstraction"/>
    </rdfs:subClassOf>
    <rdfs:label xml:lang="en">Research Area</rdfs:label>
    <rdfs:comment xml:lang="en">Specific research area, topic or field.</rdfs:comment>
  </owl:Class>
  <owl:Class rdf:about="http://www.ontotext.com/proton/protonext#WeaponModelOrSystem">
    <rdfs:subClassOf rdf:resource="http://www.ontotext.com/proton/protontop#ProductModel"/>
    <rdfs:label xml:lang="en">Weapon Model or System</rdfs:label>
    <rdfs:comment xml:lang="en">A concrete model of a weapon that determines its main features. For example, Patriot, SU-28, and Kalashnikov.</rdfs:comment>
  </owl:Class>
  <owl:Class rdf:about="http://www.ontotext.com/proton/protonext#Tower">
    <rdfs:subClassOf rdf:resource="http://www.ontotext.com/proton/protonext#Building"/>
    <rdfs:label xml:lang="en">Tower</rdfs:label>
    <rdfs:comment xml:lang="en">(ADL FT) Manmade structures, higher than their diameter, generally used for observation, storage, or electronic transmission. We use this category for carillons; for fire lookouts; and for pagodas. NIMA GNS designator TOWR.</rdfs:comment>
  </owl:Class>
  <owl:Class rdf:about="http://www.ontotext.com/proton/protonext#Drug">
    <rdfs:subClassOf>
      <owl:Class rdf:about="http://www.ontotext.com/proton/protonext#ChemicalCompound"/>
    </rdfs:subClassOf>
    <rdfs:label xml:lang="en">Drug</rdfs:label>
    <rdfs:comment xml:lang="en">A chemical substance used to improve the health condition of a person, animal, etc. For example, Aspirin, Viagra, etc.</rdfs:comment>
  </owl:Class>
  <owl:Class rdf:about="http://www.ontotext.com/proton/protonext#LandArea">
    <rdfs:subClassOf>
      <owl:Class rdf:about="http://www.ontotext.com/proton/protonext#LandRegion"/>
    </rdfs:subClassOf>
    <rdfs:label xml:lang="en">Area</rdfs:label>
    <rdfs:comment xml:lang="en">A tract of land without homogeneous character or boundaries. NIMA GNS designator L.AREA.</rdfs:comment>
  </owl:Class>
  <owl:Class rdf:about="http://www.ontotext.com/proton/protonext#Company">
    <rdfs:subClassOf>
      <owl:Class rdf:about="http://www.ontotext.com/proton/protonext#CommercialOrganization"/>
    </rdfs:subClassOf>
    <rdfs:label xml:lang="en">Company</rdfs:label>
    <rdfs:comment xml:lang="en">A private, legal, corporate entity with the legal rights to own property, manage itself, and sue or be sued. It is established by a charter or registration granted by the government.</rdfs:comment>
  </owl:Class>
  <owl:Class rdf:about="http://www.ontotext.com/proton/protonext#Battlefield">
    <rdfs:subClassOf>
      <owl:Class rdf:about="http://www.ontotext.com/proton/protonext#HistoricPlace"/>
    </rdfs:subClassOf>
    <rdfs:label xml:lang="en">Battlefield</rdfs:label>
    <rdfs:comment xml:lang="en">A site of a land battle of historical importance. NIMA GNS designator L.BTL.</rdfs:comment>
  </owl:Class>
  <owl:Class rdf:about="http://www.ontotext.com/proton/protonext#Grape">
    <rdfs:subClassOf>
      <owl:Class rdf:about="http://www.ontotext.com/proton/protonext#FloweringPlant"/>
    </rdfs:subClassOf>
    <rdfs:label xml:lang="en">Grape</rdfs:label>
    <rdfs:comment xml:lang="en">Any grape</rdfs:comment>
  </owl:Class>
  <owl:Class rdf:about="http://www.ontotext.com/proton/protonext#Parliament">
    <rdfs:subClassOf>
      <owl:Class rdf:about="http://www.ontotext.com/proton/protonext#PoliticalEntity"/>
    </rdfs:subClassOf>
    <rdfs:label xml:lang="en">Parliament</rdfs:label>
    <rdfs:comment xml:lang="en">A legislative assembly representative at national or regional level. It can also be called Senate, etc.</rdfs:comment>
  </owl:Class>
  <owl:Class rdf:about="http://www.ontotext.com/proton/protonext#AutoRacingLeague">
    <rdfs:subClassOf rdf:resource="http://www.ontotext.com/proton/protonext#SportsLeague"/>
    <rdfs:label xml:lang="en">Auto Racing League</rdfs:label>
    <rdfs:comment xml:lang="en">Any Auto Racing league</rdfs:comment>
  </owl:Class>
  <owl:Class rdf:about="http://www.ontotext.com/proton/protonext#Atoll">
    <rdfs:subClassOf>
      <owl:Class rdf:about="http://www.ontotext.com/proton/protonext#Island"/>
    </rdfs:subClassOf>
    <rdfs:label xml:lang="en">Atoll</rdfs:label>
    <rdfs:comment xml:lang="en">Any atoll</rdfs:comment>
  </owl:Class>
  <owl:Class rdf:about="http://www.ontotext.com/proton/protonext#Ministry">
    <rdfs:subClassOf rdf:resource="http://www.ontotext.com/proton/protonext#GovernmentOrganization"/>
    <rdfs:label xml:lang="en">Ministry</rdfs:label>
    <rdfs:comment xml:lang="en">(Department) A specific ministry or department, structural unit of the government of specific country with focus and authority on specific problems of the country.</rdfs:comment>
  </owl:Class>
  <owl:Class rdf:about="http://www.ontotext.com/proton/protonext#InlineHockeyLeague">
    <rdfs:subClassOf rdf:resource="http://www.ontotext.com/proton/protonext#SportsLeague"/>
    <rdfs:label xml:lang="en">Inline Hockey League</rdfs:label>
    <rdfs:comment xml:lang="en">Any Inline Hockey league</rdfs:comment>
  </owl:Class>
  <owl:Class rdf:about="http://www.ontotext.com/proton/protonext#CanadianFootballLeague">
    <rdfs:subClassOf rdf:resource="http://www.ontotext.com/proton/protonext#SportsLeague"/>
    <rdfs:label xml:lang="en">Canadian Football League</rdfs:label>
    <rdfs:comment xml:lang="en">Any Canadian Football league</rdfs:comment>
  </owl:Class>
  <owl:Class rdf:about="http://www.ontotext.com/proton/protonext#ElectronicMap">
    <rdfs:subClassOf rdf:resource="http://www.ontotext.com/proton/protontop#Document"/>
    <rdfs:label xml:lang="en">Map</rdfs:label>
    <rdfs:comment xml:lang="en">A webpage of a map</rdfs:comment>
  </owl:Class>
  <owl:Class rdf:about="http://www.ontotext.com/proton/protonext#AdministrativeRegion">
    <rdfs:subClassOf>
      <owl:Class rdf:about="http://www.ontotext.com/proton/protonext#PopulatedPlace"/>
    </rdfs:subClassOf>
    <rdfs:label xml:lang="en">Administrative Region</rdfs:label>
    <rdfs:comment xml:lang="en">Any administrative region. NIMA GNS designators - PCLIX</rdfs:comment>
  </owl:Class>
  <owl:Class rdf:about="http://www.ontotext.com/proton/protonext#SeaTrench">
    <rdfs:subClassOf>
      <owl:Class rdf:about="http://www.ontotext.com/proton/protonext#LandRegion"/>
    </rdfs:subClassOf>
    <rdfs:label xml:lang="en">Trench</rdfs:label>
    <rdfs:comment xml:lang="en">A long, narrow, characteristically very deep and asymmetrical depression of the sea floor, with relatively steep sides</rdfs:comment>
  </owl:Class>
  <owl:Class rdf:about="http://www.ontotext.com/proton/protonext#Vehicle">
    <rdfs:subClassOf rdf:resource="http://www.ontotext.com/proton/protontop#Object"/>
    <rdfs:label xml:lang="en">Vehicle</rdfs:label>
    <rdfs:comment xml:lang="en">Any sort of specific vehicle, mean of transportation.</rdfs:comment>
  </owl:Class>
  <owl:Class rdf:about="http://www.ontotext.com/proton/protonext#AlcoholicBeverage">
    <rdfs:subClassOf>
      <owl:Class rdf:about="http://www.ontotext.com/proton/protonext#Beverage"/>
    </rdfs:subClassOf>
    <rdfs:label xml:lang="en">Alcoholic Beverage</rdfs:label>
    <rdfs:comment xml:lang="en">A type (specific receipe) for a beverage. For instance: Guiness Beer, Absolut Currant, etc.</rdfs:comment>
  </owl:Class>
  <owl:Class rdf:about="http://www.ontotext.com/proton/protonext#Roadway">
    <rdfs:subClassOf>
      <owl:Class rdf:about="http://www.ontotext.com/proton/protonext#TransportFacility"/>
    </rdfs:subClassOf>
    <rdfs:label xml:lang="en">Roadway</rdfs:label>
    <rdfs:comment xml:lang="en">(ADL FT) Open ways for passage of vehicles. [USGS Circ 1048] We use this category for caravan routes; for causeways; for drives; for highways; for intersections; for parkways; for road bends; for road cuts; for road junctions; for roads; for streets; and for traffic circles. NIMA GNS designators CSWY, CSWYQ, RD, RDA, RDB, RDCUT, RDJCT, RDST, RTE, STKR.</rdfs:comment>
  </owl:Class>
  <owl:Class rdf:about="http://www.ontotext.com/proton/protonext#Painting">
    <rdfs:subClassOf>
      <owl:Class rdf:about="http://www.ontotext.com/proton/protonext#PieceOfArt"/>
    </rdfs:subClassOf>
    <rdfs:label xml:lang="en">painting</rdfs:label>
    <rdfs:comment xml:lang="en">Any painting, the results of a practice of applying paint, pigment, color or other medium[1] to a surface (support base). (Wikipedia)</rdfs:comment>
  </owl:Class>
  <owl:Class rdf:about="http://www.ontotext.com/proton/protonext#PieceOfArt">
    <rdfs:subClassOf rdf:resource="http://www.ontotext.com/proton/protontop#Object"/>
    <rdfs:label xml:lang="en">Piece of Art</rdfs:label>
    <rdfs:comment xml:lang="en">An artifact, namely a piece of art, usually, matterial object. Typical instances are paintings and sculptures. Corresponds to the Wordnet 1.7.1 synset "art, fine art - the products of human creativity; works of art collectively; "an art exhibition"@en ; "a fine collection of art")"</rdfs:comment>
  </owl:Class>
  <owl:Class rdf:about="http://www.ontotext.com/proton/protonext#TVCompany">
    <rdfs:subClassOf>
      <owl:Class rdf:about="http://www.ontotext.com/proton/protonext#Broadcaster"/>
    </rdfs:subClassOf>
    <rdfs:label xml:lang="en">TV company</rdfs:label>
    <rdfs:comment xml:lang="en">A company that broadcasts audio and video content.</rdfs:comment>
  </owl:Class>
  <owl:Class rdf:about="http://www.ontotext.com/proton/protonext#CoconutGrove">
    <rdfs:subClassOf>
      <owl:Class rdf:about="http://www.ontotext.com/proton/protonext#BiogeographicRegion"/>
    </rdfs:subClassOf>
    <rdfs:label xml:lang="en">Coconut grove</rdfs:label>
    <rdfs:comment xml:lang="en">A planting of coconut trees</rdfs:comment>
  </owl:Class>
  <owl:Class rdf:about="http://www.ontotext.com/proton/protonext#Isthmus">
    <rdfs:subClassOf>
      <owl:Class rdf:about="http://www.ontotext.com/proton/protonext#LandRegion"/>
    </rdfs:subClassOf>
    <rdfs:label xml:lang="en">Isthmus</rdfs:label>
    <rdfs:comment xml:lang="en">(ADL FT) Narrow sections of land in a body of water connecting two larger land areas. NIMA GNS designator ISTH.</rdfs:comment>
  </owl:Class>
  <owl:Class rdf:about="http://www.ontotext.com/proton/protonext#VideogamesLeague">
    <rdfs:subClassOf rdf:resource="http://www.ontotext.com/proton/protonext#SportsLeague"/>
    <rdfs:label xml:lang="en">Videogames League</rdfs:label>
    <rdfs:comment xml:lang="en">Any Videogames league</rdfs:comment>
  </owl:Class>
  <owl:Class rdf:about="http://www.ontotext.com/proton/protonext#Vineyard">
    <rdfs:subClassOf>
      <owl:Class rdf:about="http://www.ontotext.com/proton/protonext#BiogeographicRegion"/>
    </rdfs:subClassOf>
    <rdfs:label xml:lang="en">Vineyard</rdfs:label>
    <rdfs:comment xml:lang="en">Plantings of grapevines</rdfs:comment>
  </owl:Class>
  <owl:Class rdf:about="http://www.ontotext.com/proton/protonext#ResearchOrganization">
    <rdfs:subClassOf rdf:resource="http://www.ontotext.com/proton/protontop#Organization"/>
    <rdfs:label xml:lang="en">Research Organization</rdfs:label>
    <rdfs:comment xml:lang="en">An organization performing scientific research.</rdfs:comment>
  </owl:Class>
  <owl:Class rdf:about="http://www.ontotext.com/proton/protonext#CurlingLeague">
    <rdfs:subClassOf rdf:resource="http://www.ontotext.com/proton/protonext#SportsLeague"/>
    <rdfs:label xml:lang="en">Curling League</rdfs:label>
    <rdfs:comment xml:lang="en">Any Curling league</rdfs:comment>
  </owl:Class>
  <owl:Class rdf:about="http://www.ontotext.com/proton/protonext#RadioCompany">
    <rdfs:subClassOf>
      <owl:Class rdf:about="http://www.ontotext.com/proton/protonext#Broadcaster"/>
    </rdfs:subClassOf>
    <rdfs:label xml:lang="en">Radio company</rdfs:label>
    <rdfs:comment xml:lang="en">A company that broadcasts audio content.</rdfs:comment>
  </owl:Class>
  <owl:Class rdf:about="http://www.ontotext.com/proton/protonext#FilmFestival">
    <rdfs:subClassOf rdf:resource="http://www.ontotext.com/proton/protonext#Festival"/>
    <rdfs:label xml:lang="en">Film Festival</rdfs:label>
    <rdfs:comment xml:lang="en">Any festival involving showing a film.</rdfs:comment>
  </owl:Class>
  <owl:Class rdf:about="http://www.ontotext.com/proton/protonext#MilitaryAreas">
    <rdfs:subClassOf>
      <owl:Class rdf:about="http://www.ontotext.com/proton/protonext#PoliticalRegion"/>
    </rdfs:subClassOf>
    <rdfs:label xml:lang="en">Military Areas</rdfs:label>
    <rdfs:comment xml:lang="en">(ADL FTT) We use this category for air force bases; for army facilities; for arsenals; for artillery ranges; for barracks; for bases (military); for camps (military); for forts; for infantry camps; for maneuver areas; for military bases; for military installations; for national guard facilities; and for naval bases. The following NIMA designators fit here: MILB, INSM, SCHM. The following ADL types are skipped as irrelevant: Cadastral areas,</rdfs:comment>
  </owl:Class>
  <owl:Class rdf:about="http://www.ontotext.com/proton/protonext#Concert">
    <rdfs:subClassOf>
      <owl:Class rdf:about="http://www.ontotext.com/proton/protonext#ArtPerformance"/>
    </rdfs:subClassOf>
    <rdfs:label xml:lang="en">Concert</rdfs:label>
    <rdfs:comment xml:lang="en">An art performance consisting of playing music.</rdfs:comment>
  </owl:Class>
  <owl:Class rdf:about="http://www.ontotext.com/proton/protonext#FieldHockeyLeague">
    <rdfs:subClassOf rdf:resource="http://www.ontotext.com/proton/protonext#SportsLeague"/>
    <rdfs:label xml:lang="en">Field Hockey League</rdfs:label>
    <rdfs:comment xml:lang="en">Any Field Hockey league</rdfs:comment>
  </owl:Class>
  <owl:Class rdf:about="http://www.ontotext.com/proton/protonext#SingleSongOrAlbum">
    <rdfs:subClassOf>
      <owl:Class rdf:about="http://www.ontotext.com/proton/protonext#AudioRecording"/>
    </rdfs:subClassOf>
    <rdfs:label xml:lang="en">Single</rdfs:label>
    <rdfs:comment xml:lang="en">Any Single Song and Album</rdfs:comment>
  </owl:Class>
  <owl:Class rdf:about="http://www.ontotext.com/proton/protonext#Airline">
    <rdfs:subClassOf rdf:resource="http://www.ontotext.com/proton/protonext#Company"/>
    <rdfs:label xml:lang="en">Airline</rdfs:label>
    <rdfs:comment xml:lang="en">A company providing air transport services.</rdfs:comment>
  </owl:Class>
  <owl:Class rdf:about="http://www.ontotext.com/proton/protonext#SpeedwayTeam">
    <rdfs:subClassOf>
      <owl:Class rdf:about="http://www.ontotext.com/proton/protonext#Team"/>
    </rdfs:subClassOf>
    <rdfs:label xml:lang="en">Speedway team</rdfs:label>
    <rdfs:comment xml:lang="en">Any speedway team</rdfs:comment>
  </owl:Class>
  <owl:Class rdf:about="http://www.ontotext.com/proton/protonext#Artery">
    <rdfs:subClassOf rdf:resource="http://www.ontotext.com/proton/protonext#BodyPart"/>
    <rdfs:label xml:lang="en">Artery</rdfs:label>
    <rdfs:comment xml:lang="en">Any artery as a part of the body.</rdfs:comment>
  </owl:Class>
  <owl:Class rdf:about="http://www.ontotext.com/proton/protonext#IndustrySector">
    <rdfs:subClassOf>
      <owl:Class rdf:about="http://www.ontotext.com/proton/protonext#BusinessAbstraction"/>
    </rdfs:subClassOf>
    <rdfs:label xml:lang="en">Industry Sector</rdfs:label>
    <rdfs:comment xml:lang="en">A classification of companies that have similar production processes, similar products, etc.</rdfs:comment>
  </owl:Class>
  <owl:Class rdf:about="http://www.ontotext.com/proton/protonext#Geyser">
    <rdfs:subClassOf>
      <owl:Class rdf:about="http://www.ontotext.com/proton/protonext#Spring"/>
    </rdfs:subClassOf>
    <rdfs:label xml:lang="en">Geyser</rdfs:label>
    <rdfs:comment xml:lang="en">A spring characterized by intermittent discharge of water ejected turbulently and accompanied by a vapour phase (steam). NIMA GNS designator H.GYSR.</rdfs:comment>
  </owl:Class>
  <owl:Class rdf:about="http://www.ontotext.com/proton/protonext#ChemicalCompound">
    <rdfs:subClassOf rdf:resource="http://www.ontotext.com/proton/protonext#ChemicalSubstance"/>
    <rdfs:subClassOf rdf:resource="http://www.ontotext.com/proton/protontop#ProductModel"/>
    <rdfs:label xml:lang="en">Chemical Compound</rdfs:label>
    <rdfs:comment xml:lang="en">A specific chemical compound, such as H2O or Zarin.</rdfs:comment>
  </owl:Class>
  <owl:Class rdf:about="http://www.ontotext.com/proton/protonext#NewspaperIssue">
    <rdfs:subClassOf rdf:resource="http://www.ontotext.com/proton/protonext#IssueOfPeriodical"/>
    <rdfs:subClassOf>
      <owl:Class rdf:about="http://www.ontotext.com/proton/protonext#ResourceCollection"/>
    </rdfs:subClassOf>
    <rdfs:label xml:lang="en">Newspaper Issue</rdfs:label>
    <rdfs:comment xml:lang="en">A specific issue of a newspaper.</rdfs:comment>
  </owl:Class>
  <owl:Class rdf:about="http://www.ontotext.com/proton/protonext#StreetNumber">
    <rdfs:subClassOf rdf:resource="http://www.ontotext.com/proton/protontop#ContactInformation"/>
    <rdfs:label xml:lang="en">Street Number</rdfs:label>
    <rdfs:comment xml:lang="en">Part of a postal address denoting the street number.</rdfs:comment>
  </owl:Class>
  <owl:Class rdf:about="http://www.ontotext.com/proton/protonext#Oasis">
    <rdfs:subClassOf>
      <owl:Class rdf:about="http://www.ontotext.com/proton/protonext#BiogeographicRegion"/>
    </rdfs:subClassOf>
    <rdfs:label xml:lang="en">Oasis</rdfs:label>
    <rdfs:comment xml:lang="en">(ADL FT) Fertile, vegetated areas in the midst of a desert, where the water table has come close enough to the surface for wells and springs or seepages to exist, thus making them suitable for human habitation. NIMA GNS designator OAS.</rdfs:comment>
  </owl:Class>
  <owl:Class rdf:about="http://www.ontotext.com/proton/protonext#Saint">
    <rdfs:subClassOf rdf:resource="http://www.ontotext.com/proton/protontop#Person"/>
    <rdfs:label xml:lang="en">Saint</rdfs:label>
    <rdfs:comment xml:lang="en">Any saint, a holy person, in whom Christ dwells, whether in heaven or in earth.</rdfs:comment>
  </owl:Class>
  <owl:Class rdf:about="http://www.ontotext.com/proton/protonext#AgriculturalColony">
    <rdfs:subClassOf>
      <owl:Class rdf:about="http://www.ontotext.com/proton/protonext#LandRegion"/>
    </rdfs:subClassOf>
    <rdfs:label xml:lang="en">Agricultural Colony</rdfs:label>
    <rdfs:comment xml:lang="en">A tract of land set aside for agricultural settlement. NIMA GNS designator L.AGRC.</rdfs:comment>
  </owl:Class>
  <owl:Class rdf:about="http://www.ontotext.com/proton/protonext#Quarter">
    <rdfs:subClassOf rdf:resource="http://www.ontotext.com/proton/protontop#TimeInterval"/>
    <rdfs:label xml:lang="en">Quarter</rdfs:label>
    <rdfs:comment xml:lang="en">A specific quarter of a specific year, such as Q4 1999</rdfs:comment>
  </owl:Class>
  <owl:Class rdf:about="http://www.ontotext.com/proton/protonext#TradeUnion">
    <rdfs:subClassOf rdf:resource="http://www.ontotext.com/proton/protontop#Organization"/>
    <rdfs:label xml:lang="en">Trade Union</rdfs:label>
    <rdfs:comment xml:lang="en">Any Trade Union, an organization of workers that have banded together to achieve common goals such as better working conditions. (Wikipedia)</rdfs:comment>
  </owl:Class>
  <owl:Class rdf:about="http://www.ontotext.com/proton/protonext#Brand">
    <rdfs:subClassOf rdf:resource="http://www.ontotext.com/proton/protontop#Object"/>
    <rdfs:label xml:lang="en">Brand</rdfs:label>
    <rdfs:comment xml:lang="en">The American Marketing Association defines a brand as a "Name, term, design, symbol, or any other feature that identifies one seller's good or service as distinct from those of other sellers." Wikipedia. Examples: Dodge and Milka</rdfs:comment>
  </owl:Class>
  <owl:Class rdf:about="http://www.ontotext.com/proton/protonext#PublishedMaterial">
    <rdfs:subClassOf rdf:resource="http://www.ontotext.com/proton/protonext#MediaProduct"/>
    <rdfs:subClassOf rdf:resource="http://www.ontotext.com/proton/protontop#Document"/>
    <rdfs:label xml:lang="en">Published Material</rdfs:label>
    <rdfs:comment xml:lang="en">A document that is published or intended for publishing</rdfs:comment>
  </owl:Class>
  <owl:Class rdf:about="http://www.ontotext.com/proton/protonext#Pond">
    <rdfs:subClassOf>
      <owl:Class rdf:about="http://www.ontotext.com/proton/protonext#WaterRegion"/>
    </rdfs:subClassOf>
    <rdfs:label xml:lang="en">Pond</rdfs:label>
    <rdfs:comment xml:lang="en">A pond is a body of standing water, either natural or man-made, that is usually smaller than a lake. (Wikipedia). http://www.eionet.europa.eu/gemet/concept/6507. NIMA GNS designator H.PND, H.PNDI, H.PNDN, H.PNDNI, H.PNDS, H.PNDSF, H.PNDSI, H.PNDSN, H.MFGN.</rdfs:comment>
  </owl:Class>
  <owl:Class rdf:about="http://www.ontotext.com/proton/protonext#Peninsula">
    <rdfs:subClassOf>
      <owl:Class rdf:about="http://www.ontotext.com/proton/protonext#LandRegion"/>
    </rdfs:subClassOf>
    <rdfs:label xml:lang="en">Peninsula</rdfs:label>
    <rdfs:comment xml:lang="en">A land region surrounded by water from most sides, but having land connect to bigger land region. NIMA GNS designator PEN, PENX.</rdfs:comment>
  </owl:Class>
  <owl:Class rdf:about="http://www.ontotext.com/proton/protonext#Food">
    <rdfs:subClassOf rdf:resource="http://www.ontotext.com/proton/protontop#Object"/>
    <rdfs:label xml:lang="en">Food</rdfs:label>
    <rdfs:comment xml:lang="en">Food is any eatable or drinkable substance that is normally consumed by humans. DBPedia</rdfs:comment>
  </owl:Class>
  <owl:Class rdf:about="http://www.ontotext.com/proton/protonext#SportClub">
    <rdfs:subClassOf rdf:resource="http://www.ontotext.com/proton/protonext#Company"/>
    <rdfs:subClassOf rdf:resource="http://www.ontotext.com/proton/protonext#SportOrganization"/>
    <rdfs:label xml:lang="en">Sport Club</rdfs:label>
    <rdfs:comment xml:lang="en">A sports club, football club or F1 team. Those should be considered commercial although in many cases they are not run for profit.</rdfs:comment>
    <rdfs:comment xml:lang="en">An organization arranging the practice of some sports by teams or individuals.</rdfs:comment>
  </owl:Class>
  <owl:Class rdf:about="http://www.ontotext.com/proton/protonext#Island">
    <rdfs:subClassOf>
      <owl:Class rdf:about="http://www.ontotext.com/proton/protonext#LandRegion"/>
    </rdfs:subClassOf>
    <rdfs:label xml:lang="en">Island</rdfs:label>
    <rdfs:comment xml:lang="en">(ADL FT) Tracts of land smaller than a continent, surrounded by the water of an ocean, sea, lake or stream. [Glossary of Geology, 4th ed.] We use this category for atolls; for cays; for island arcs; for isles; for islets; for keys (islands); for land-tied islands; and for mangrove islands. NIMA GNS designator ISL, ISLF, ISLM, ISLS, ISLT, ISLX</rdfs:comment>
  </owl:Class>
  <owl:Class rdf:about="http://www.ontotext.com/proton/protonext#HandballLeague">
    <rdfs:subClassOf rdf:resource="http://www.ontotext.com/proton/protonext#SportsLeague"/>
    <rdfs:label xml:lang="en">Handball League</rdfs:label>
    <rdfs:comment xml:lang="en">Any Handball league</rdfs:comment>
  </owl:Class>
  <owl:Class rdf:about="http://www.ontotext.com/proton/protonext#School">
    <rdfs:subClassOf>
      <owl:Class rdf:about="http://www.ontotext.com/proton/protonext#EducationalOrganization"/>
    </rdfs:subClassOf>
    <rdfs:label xml:lang="en">School</rdfs:label>
    <rdfs:comment xml:lang="en">An education organization teaching pupils from first grade to tenth/eleventh/twelfth grade. It could be a primary school, or a secondary school.</rdfs:comment>
  </owl:Class>
  <owl:Class rdf:about="http://www.ontotext.com/proton/protonext#IrrigationSystem">
    <rdfs:subClassOf>
      <owl:Class rdf:about="http://www.ontotext.com/proton/protonext#WaterRegion"/>
    </rdfs:subClassOf>
    <rdfs:label xml:lang="en">Irrigation System</rdfs:label>
    <rdfs:comment xml:lang="en">A network of ditches and one or more of the following elements: water supply, reservoir, canal, pump, well, drain, etc. NIMA GNS designator H.SYSI.</rdfs:comment>
  </owl:Class>
  <owl:Class rdf:about="http://www.ontotext.com/proton/protonext#AirplaneModel">
    <rdfs:subClassOf rdf:resource="http://www.ontotext.com/proton/protontop#ProductModel"/>
    <rdfs:label xml:lang="en">Airplane Model</rdfs:label>
    <rdfs:comment xml:lang="en">A concrete model of an airplane which determines the main features of any airplane of this model. For example, Boeing 737, Airbus A330, etc.</rdfs:comment>
  </owl:Class>
  <owl:Class rdf:about="http://www.ontotext.com/proton/protonext#MusicCompany">
    <rdfs:subClassOf rdf:resource="http://www.ontotext.com/proton/protonext#EntertainmentCompany"/>
    <rdfs:label xml:lang="en">Musical Company</rdfs:label>
    <rdfs:comment xml:lang="en">Any Musical company, a company involved in the music business, e.g. sells compositions, recordings and performances of music, like Soni Music Entertainment.</rdfs:comment>
  </owl:Class>
  <owl:Class rdf:about="http://www.ontotext.com/proton/protonext#MusicGenre">
    <rdfs:subClassOf rdf:resource="http://www.ontotext.com/proton/protonext#Genre"/>
    <rdfs:label xml:lang="en">Music Genre</rdfs:label>
    <rdfs:comment xml:lang="en">Any genre which pertians to music, e.g. classical, folk, pop, etc.</rdfs:comment>
  </owl:Class>
  <owl:Class rdf:about="http://www.ontotext.com/proton/protonext#Crater">
    <rdfs:subClassOf>
      <owl:Class rdf:about="http://www.ontotext.com/proton/protonext#LandRegion"/>
    </rdfs:subClassOf>
    <rdfs:label xml:lang="en">Crater</rdfs:label>
    <rdfs:comment xml:lang="en">(ADL FT) Circular-shaped depressions at the summit of a volcanic core or on the surface of the land caused by the impact of a meteorite; man-made depressions caused by an explosion. ... We use this category for calderas. NIMA GNS designator CRTR, CLDA.</rdfs:comment>
  </owl:Class>
  <owl:Class rdf:about="http://www.ontotext.com/proton/protonext#Satellite">
    <rdfs:subClassOf>
      <owl:Class rdf:about="http://www.ontotext.com/proton/protonext#AstronomicalObject"/>
    </rdfs:subClassOf>
    <rdfs:label xml:lang="en">Satellite</rdfs:label>
    <rdfs:comment xml:lang="en">An astronomic object orbiting around a planet or star. Definition partly derived from WordNet 1.7</rdfs:comment>
  </owl:Class>
  <owl:Class rdf:about="http://www.ontotext.com/proton/protonext#City">
    <rdfs:subClassOf rdf:resource="http://www.ontotext.com/proton/protonext#Settlement"/>
    <rdfs:label xml:lang="en">City</rdfs:label>
    <rdfs:comment xml:lang="en">(ADL FT) For smaller, less formally established communities, use 'populated places'. For independent cities, use 'countries, 2nd order divisions. Incorporated populated places. [Adapted from USGS Circ 1048] We use this category for municipalities; for towns; and for urban areas. NIMA GNS designator PPL.</rdfs:comment>
  </owl:Class>
  <owl:Class rdf:about="http://www.ontotext.com/proton/protonext#Database">
    <rdfs:subClassOf rdf:resource="http://www.ontotext.com/proton/protonext#Dataset"/>
    <rdfs:label xml:lang="en">Database</rdfs:label>
    <rdfs:comment xml:lang="en">A dataset loaded in a system supporting search, update and other operations over the information in the dataset.</rdfs:comment>
  </owl:Class>
  <owl:Class rdf:about="http://www.ontotext.com/proton/protonext#Estuary">
    <rdfs:subClassOf>
      <owl:Class rdf:about="http://www.ontotext.com/proton/protonext#WaterRegion"/>
    </rdfs:subClassOf>
    <rdfs:label xml:lang="en">Estuary</rdfs:label>
    <rdfs:comment xml:lang="en">A partly enclosed coastal body of water with one or more rivers or streams flowing into it, and with a free connection to the open sea. NIMA GNS designator H.ESTY.</rdfs:comment>
  </owl:Class>
  <owl:Class rdf:about="http://www.ontotext.com/proton/protonext#DayTime">
    <rdfs:subClassOf>
      <owl:Class rdf:about="http://www.ontotext.com/proton/protonext#TemporalAbstraction"/>
    </rdfs:subClassOf>
    <rdfs:label xml:lang="en">Daytime</rdfs:label>
    <rdfs:comment xml:lang="en">Specific time (point) during the day, when the day is not specified. Like in "the supermarket is closing 20:30 p.m."</rdfs:comment>
  </owl:Class>
  <owl:Class rdf:about="http://www.ontotext.com/proton/protonext#Device">
    <rdfs:subClassOf rdf:resource="http://www.ontotext.com/proton/protontop#ProductModel"/>
    <rdfs:label>Device</rdfs:label>
  </owl:Class>
  <owl:Class rdf:about="http://www.ontotext.com/proton/protonext#Institute">
    <rdfs:subClassOf rdf:resource="http://www.ontotext.com/proton/protonext#ResearchOrganization"/>
    <rdfs:label xml:lang="en">Institute</rdfs:label>
    <rdfs:comment xml:lang="en">A research organization devoted primarily on search in some scientific research.</rdfs:comment>
  </owl:Class>
  <owl:Class rdf:about="http://www.ontotext.com/proton/protonext#CelebrityTitle">
    <rdfs:subClassOf>
      <owl:Class rdf:about="http://www.ontotext.com/proton/protonext#SocialFunction"/>
    </rdfs:subClassOf>
    <rdfs:label xml:lang="en">Celebrity</rdfs:label>
    <rdfs:comment xml:lang="en">The social function of celebrity, a status of notoriety in the society.</rdfs:comment>
  </owl:Class>
  <owl:Class rdf:about="http://www.ontotext.com/proton/protonext#Movie">
    <rdfs:subClassOf rdf:resource="http://www.ontotext.com/proton/protonext#MediaProduct"/>
    <rdfs:label xml:lang="en">Movie</rdfs:label>
    <rdfs:comment xml:lang="en">A film, also called a movie or motion picture, is a series of still or moving images. Wikipedia.</rdfs:comment>
  </owl:Class>
  <owl:Class rdf:about="http://www.ontotext.com/proton/protonext#Meadow">
    <rdfs:subClassOf>
      <owl:Class rdf:about="http://www.ontotext.com/proton/protonext#BiogeographicRegion"/>
    </rdfs:subClassOf>
    <rdfs:label xml:lang="en">Meadow</rdfs:label>
    <rdfs:comment xml:lang="en">A small, poorly drained area dominated by grassy vegetation</rdfs:comment>
  </owl:Class>
  <owl:Class rdf:about="http://www.ontotext.com/proton/protonext#Watercourse">
    <rdfs:subClassOf rdf:resource="http://www.ontotext.com/proton/protonext#HydrographicStructure"/>
    <rdfs:subClassOf>
      <owl:Class rdf:about="http://www.ontotext.com/proton/protonext#WaterRegion"/>
    </rdfs:subClassOf>
    <rdfs:label xml:lang="en">Watercourse</rdfs:label>
    <rdfs:comment xml:lang="en">A natural, well-defined channel produced by flowing water, or an artificial channel designed to carry flowing water. NIMA GNS designator H.WTRC.</rdfs:comment>
  </owl:Class>
  <owl:Class rdf:about="http://www.ontotext.com/proton/protonext#Album">
    <rdfs:subClassOf>
      <owl:Class rdf:about="http://www.ontotext.com/proton/protonext#AudioRecording"/>
    </rdfs:subClassOf>
    <rdfs:label xml:lang="en">Album</rdfs:label>
    <rdfs:comment xml:lang="en">An recording of a several songs. Usually from the same singer.</rdfs:comment>
  </owl:Class>
  <owl:Class rdf:about="http://www.ontotext.com/proton/protonext#IceHockeyLeague">
    <rdfs:subClassOf rdf:resource="http://www.ontotext.com/proton/protonext#SportsLeague"/>
    <rdfs:label xml:lang="en">Ice Hockey League</rdfs:label>
    <rdfs:comment xml:lang="en">Any Ice Hockey league</rdfs:comment>
  </owl:Class>
  <owl:Class rdf:about="http://www.ontotext.com/proton/protonext#Charity">
    <rdfs:subClassOf rdf:resource="http://www.ontotext.com/proton/protonext#Non-ProfitOrganisation"/>
    <rdfs:label xml:lang="en">Charity</rdfs:label>
    <rdfs:comment xml:lang="en">Any Charity, an organization involved in the practice of benevolent giving and caring. (Wikipedia)</rdfs:comment>
  </owl:Class>
  <owl:Class rdf:about="http://www.ontotext.com/proton/protonext#VolleyballLeague">
    <rdfs:subClassOf rdf:resource="http://www.ontotext.com/proton/protonext#SportsLeague"/>
    <rdfs:label xml:lang="en">Volleyball League</rdfs:label>
    <rdfs:comment xml:lang="en">Any Volleyball league</rdfs:comment>
  </owl:Class>
  <owl:Class rdf:about="http://www.ontotext.com/proton/protonext#SingleSong">
    <rdfs:subClassOf rdf:resource="http://www.ontotext.com/proton/protonext#SingleSongOrAlbum"/>
    <rdfs:subClassOf>
      <owl:Class rdf:about="http://www.ontotext.com/proton/protonext#Song"/>
    </rdfs:subClassOf>
    <rdfs:label xml:lang="en">Single</rdfs:label>
    <rdfs:comment xml:lang="en">A representative for an album or a musician song.</rdfs:comment>
  </owl:Class>
  <owl:Class rdf:about="http://www.ontotext.com/proton/protonext#AmericanFootballTeam">
    <rdfs:subClassOf>
      <owl:Class rdf:about="http://www.ontotext.com/proton/protonext#Team"/>
    </rdfs:subClassOf>
    <rdfs:label xml:lang="en">American Football Team</rdfs:label>
    <rdfs:comment xml:lang="en">Any American Football Team</rdfs:comment>
  </owl:Class>
  <owl:Class rdf:about="http://www.ontotext.com/proton/protonext#FaxNumber">
    <rdfs:subClassOf>
      <owl:Class rdf:about="http://www.ontotext.com/proton/protonext#PhoneNumber"/>
    </rdfs:subClassOf>
    <rdfs:label xml:lang="en">Fax Number</rdfs:label>
    <rdfs:comment xml:lang="en">A phone number connected to a fax machine.</rdfs:comment>
  </owl:Class>
  <owl:Class rdf:about="http://www.ontotext.com/proton/protonext#Bay">
    <rdfs:subClassOf>
      <owl:Class rdf:about="http://www.ontotext.com/proton/protonext#WaterRegion"/>
    </rdfs:subClassOf>
    <rdfs:label xml:lang="en">Bay</rdfs:label>
    <rdfs:comment xml:lang="en">(ADL FT) Indentations of a coastline or shoreline enclosing a part of a body of water; bodies of water partly surrounded by land. We use this category for bahias; for coves; and for embayments. NIMA GNS designators BAY, BAYS.</rdfs:comment>
  </owl:Class>
  <owl:Class rdf:about="http://www.ontotext.com/proton/protonext#BiologicalDatabase">
    <rdfs:subClassOf rdf:resource="http://www.ontotext.com/proton/protonext#Database"/>
    <rdfs:label xml:lang="en">Biological Database</rdfs:label>
    <rdfs:comment xml:lang="en">A database containing information about biological entities.</rdfs:comment>
  </owl:Class>
  <owl:Class rdf:about="http://www.ontotext.com/proton/protonext#InternetAddress">
    <rdfs:subClassOf rdf:resource="http://www.ontotext.com/proton/protonext#Address"/>
    <rdfs:label xml:lang="en">Internet Address</rdfs:label>
    <rdfs:comment xml:lang="en">An identifier that determines a resource on the Internet.</rdfs:comment>
  </owl:Class>
  <owl:Class rdf:about="http://www.ontotext.com/proton/protonext#TelevisionShow">
    <rdfs:subClassOf rdf:resource="http://www.ontotext.com/proton/protonext#TelevisionProduct"/>
    <rdfs:label xml:lang="en">Television Show</rdfs:label>
    <rdfs:comment xml:lang="en">Any television show</rdfs:comment>
  </owl:Class>
  <owl:Class rdf:about="http://www.ontotext.com/proton/protonext#Gene">
    <rdfs:subClassOf>
      <owl:Class rdf:about="http://www.ontotext.com/proton/protonext#BiologicalSubstance"/>
    </rdfs:subClassOf>
    <rdfs:label xml:lang="en">Gene</rdfs:label>
    <rdfs:comment xml:lang="en">A gene is a molecular unit of heredity of a living organism. Wikipedia</rdfs:comment>
  </owl:Class>
  <owl:Class rdf:about="http://www.ontotext.com/proton/protonext#ProtectedArea">
    <rdfs:subClassOf>
      <owl:Class rdf:about="http://www.ontotext.com/proton/protonext#LocationOfSpecialInterest"/>
    </rdfs:subClassOf>
    <rdfs:label xml:lang="en">Protected Area</rdfs:label>
    <rdfs:comment xml:lang="en">Any Protected Area, an area which benefits of special attention and is with limited access or protected in other ways.</rdfs:comment>
  </owl:Class>
  <owl:Class rdf:about="http://www.ontotext.com/proton/protonext#Disease">
    <rdfs:subClassOf rdf:resource="http://www.ontotext.com/proton/protontop#Event"/>
    <rdfs:label xml:lang="en">Disease</rdfs:label>
    <rdfs:comment xml:lang="en">A specific sort of desease, such as AIDS, SARS, Parcinson, etc. The instances of those class can often by considered as terms instead of entities, but in all cases, those are the general phenomena, not the particular situations when somebody is suffering the disease.</rdfs:comment>
  </owl:Class>
  <owl:Class rdf:about="http://www.ontotext.com/proton/protonext#Cape">
    <rdfs:subClassOf>
      <owl:Class rdf:about="http://www.ontotext.com/proton/protonext#LandRegion"/>
    </rdfs:subClassOf>
    <rdfs:label xml:lang="en">Cape</rdfs:label>
    <rdfs:comment xml:lang="en">(ADL FT) Projection of land extending into a body of water that prominently marks a change in or interrupts the coastal trend of that water body. We use this category for headlands; for peninsulas; for points (physiographic); and for promontories. NIMA GNS designator CAPE, HDLD, PROM.</rdfs:comment>
  </owl:Class>
  <owl:Class rdf:about="http://www.ontotext.com/proton/protonext#TVChannel">
    <rdfs:subClassOf rdf:resource="http://www.ontotext.com/proton/protonext#MediaBrand"/>
    <rdfs:label xml:lang="en">TV Channel</rdfs:label>
    <rdfs:comment xml:lang="en">A brand of a television channel.</rdfs:comment>
  </owl:Class>
  <owl:Class rdf:about="http://www.ontotext.com/proton/protonext#EMail">
    <rdfs:subClassOf rdf:resource="http://www.ontotext.com/proton/protonext#InternetAddress"/>
    <rdfs:label xml:lang="en">E-mail</rdfs:label>
    <rdfs:comment xml:lang="en">An identifier that determines a electronic mail box.</rdfs:comment>
  </owl:Class>
  <owl:Class rdf:about="http://www.ontotext.com/proton/protonext#Colour">
    <rdfs:subClassOf rdf:resource="http://www.ontotext.com/proton/protontop#Abstract"/>
    <rdfs:label xml:lang="en">Colour</rdfs:label>
    <rdfs:comment xml:lang="en">Any colour, a visual perceptual property, e.g. red, blue, yellow, etc. (Wikipedia)</rdfs:comment>
  </owl:Class>
  <owl:Class rdf:about="http://www.ontotext.com/proton/protonext#Guyot">
    <rdfs:subClassOf>
      <owl:Class rdf:about="http://www.ontotext.com/proton/protonext#LandRegion"/>
    </rdfs:subClassOf>
    <rdfs:label xml:lang="en">Guyot</rdfs:label>
    <rdfs:label xml:lang="en">Tablemount</rdfs:label>
    <rdfs:comment xml:lang="en">A seamount having a comparatively smooth, flat top</rdfs:comment>
  </owl:Class>
  <owl:Class rdf:about="http://www.ontotext.com/proton/protonext#Hospital">
    <rdfs:subClassOf rdf:resource="http://www.ontotext.com/proton/protonext#Building"/>
    <rdfs:label xml:lang="en">Hospital</rdfs:label>
    <rdfs:comment xml:lang="en">Any Hospital, a building which is a hospital.</rdfs:comment>
  </owl:Class>
  <owl:Class rdf:about="http://www.ontotext.com/proton/protonext#SportFacility">
    <rdfs:subClassOf>
      <owl:Class rdf:about="http://www.ontotext.com/proton/protonext#RecreationalFacility"/>
    </rdfs:subClassOf>
    <rdfs:label xml:lang="en">Sport Facility</rdfs:label>
    <rdfs:comment xml:lang="en">(ADL FT) Fields, centers, or open areas maintained for the purpose of holding sporting events and activities. [USGS Circ 1048] We use this category for aquatic centers; for arenas; for athletic complexes; for athletic fields; for ball parks; for baseball fields; for dragways; for equestrian centers; for fields; for football fields; for golf clubs; for golf courses; for gymnasiums; for natatoriums; for physical education facilities; for pistol ranges (sport); for polo fields; for pools, swimming; for race tracks; for racecourses; for racetracks; for raceways; for rifle ranges; for rodeo grounds; for shooting ranges (sport); for skeet shooting ranges; for ski areas; for ski facilities; for ski trails; for speedways; for stadiums; for swim clubs; for swimming pools; for tennis clubs; and for tennis courts. NIMA GNS designators RECG, RECR, STDM, ATHF.</rdfs:comment>
  </owl:Class>
  <owl:Class rdf:about="http://www.ontotext.com/proton/protonext#Lagoon">
    <rdfs:subClassOf>
      <owl:Class rdf:about="http://www.ontotext.com/proton/protonext#WaterRegion"/>
    </rdfs:subClassOf>
    <rdfs:label xml:lang="en">Lagoon</rdfs:label>
    <rdfs:comment xml:lang="en">A body of water cut off from the open sea by coral reefs or sand bars. http://www.eionet.europa.eu/gemet/concept/4589. NIMA GNS designator H.LGN, H.LGNS, H.LGNX.</rdfs:comment>
  </owl:Class>
  <owl:Class rdf:about="http://www.ontotext.com/proton/protonext#Scrubland">
    <rdfs:subClassOf>
      <owl:Class rdf:about="http://www.ontotext.com/proton/protonext#BiogeographicRegion"/>
    </rdfs:subClassOf>
    <rdfs:label xml:lang="en">Scrubland</rdfs:label>
    <rdfs:comment xml:lang="en">An area of low trees, bushes, and shrubs stunted by some environmental limitation</rdfs:comment>
  </owl:Class>
  <owl:Class rdf:about="http://www.ontotext.com/proton/protonext#PoliticalEntity">
    <rdfs:subClassOf rdf:resource="http://www.ontotext.com/proton/protontop#Organization"/>
    <rdfs:label xml:lang="en">Political Entity</rdfs:label>
    <rdfs:comment xml:lang="en">Any organization which has a political functions.</rdfs:comment>
  </owl:Class>
  <owl:Class rdf:about="http://www.ontotext.com/proton/protonext#Money">
    <rdfs:subClassOf>
      <owl:Class rdf:about="http://www.ontotext.com/proton/protonext#SocialAbstraction"/>
    </rdfs:subClassOf>
    <rdfs:label xml:lang="en">Money</rdfs:label>
    <rdfs:comment xml:lang="en">A specific amount of money in specific currency</rdfs:comment>
  </owl:Class>
  <owl:Class rdf:about="http://www.ontotext.com/proton/protonext#Continent">
    <rdfs:subClassOf>
      <owl:Class rdf:about="http://www.ontotext.com/proton/protonext#LandRegion"/>
    </rdfs:subClassOf>
    <rdfs:subClassOf>
      <owl:Class rdf:about="http://www.ontotext.com/proton/protonext#PopulatedPlace"/>
    </rdfs:subClassOf>
    <rdfs:label xml:lang="en">Continent</rdfs:label>
    <rdfs:comment xml:lang="en">(ADL FT) Earth's major land masses, including both dry land and continental shelves. NIMA GNS designator - no equivalent.</rdfs:comment>
  </owl:Class>
  <owl:Class rdf:about="http://www.ontotext.com/proton/protonext#PopulatedPlace">
    <rdfs:subClassOf rdf:resource="http://www.ontotext.com/proton/protontop#Location"/>
    <rdfs:label xml:lang="en">Populated Place</rdfs:label>
    <rdfs:comment xml:lang="en">(ADL FT) Places or areas with clustered or scattered buildings and a permanent human population. ... We use this category for agricultural colonies; for communes; for communities; for hamlets; for homesteads; for locales; for localities; for metropolitan areas; for populated localities; for ppl; for pueblos; for settlements; for suburbs; for villages; and with religious facilities for religious populated places. NIMA GNS designator PPL, PPL(x)</rdfs:comment>
  </owl:Class>
  <owl:Class rdf:about="http://www.ontotext.com/proton/protonext#CultivatedArea">
    <rdfs:subClassOf>
      <owl:Class rdf:about="http://www.ontotext.com/proton/protonext#BiogeographicRegion"/>
    </rdfs:subClassOf>
    <rdfs:label xml:lang="en">Cultivated area</rdfs:label>
    <rdfs:comment xml:lang="en">An area under cultivation</rdfs:comment>
  </owl:Class>
  <owl:Class rdf:about="http://www.ontotext.com/proton/protonext#SoftwareAgent">
    <rdfs:subClassOf rdf:resource="http://www.ontotext.com/proton/protontop#Agent"/>
    <rdfs:label>Software Agent</rdfs:label>
    <rdfs:comment>An artificial agent which operates in a software environment.</rdfs:comment>
  </owl:Class>
  <owl:Class rdf:about="http://www.ontotext.com/proton/protonext#WineRegion">
    <rdfs:subClassOf>
      <owl:Class rdf:about="http://www.ontotext.com/proton/protonext#LandRegion"/>
    </rdfs:subClassOf>
    <rdfs:label xml:lang="en">Wine Region</rdfs:label>
    <rdfs:comment xml:lang="en">Any Wine Region, a region where wine is produced.</rdfs:comment>
  </owl:Class>
  <owl:Class rdf:about="http://www.ontotext.com/proton/protonext#Delta">
    <rdfs:subClassOf>
      <owl:Class rdf:about="http://www.ontotext.com/proton/protonext#LandRegion"/>
    </rdfs:subClassOf>
    <rdfs:label xml:lang="en">Delta</rdfs:label>
    <rdfs:label xml:lang="en">Delta of a River</rdfs:label>
    <rdfs:comment xml:lang="en">(ADL FT) Flat plains formed by alluvial deposits at the mouth of a stream. NIMA GNS designator DLTA.</rdfs:comment>
  </owl:Class>
  <owl:Class rdf:about="http://www.ontotext.com/proton/protonext#Sale">
    <rdfs:subClassOf rdf:resource="http://www.ontotext.com/proton/protontop#Event"/>
    <rdfs:label xml:lang="en">Sale</rdfs:label>
    <rdfs:comment xml:lang="en">Any event in which a participant is receiving a good from another participant of the event on the basis of some payment.</rdfs:comment>
  </owl:Class>
  <owl:Class rdf:about="http://www.ontotext.com/proton/protonext#PhoneNumber">
    <rdfs:subClassOf rdf:resource="http://www.ontotext.com/proton/protontop#ContactInformation"/>
    <rdfs:label xml:lang="en">Phone Number</rdfs:label>
    <rdfs:comment xml:lang="en">A sequence of digits which represents an address of a telephone device within a telephone net.</rdfs:comment>
  </owl:Class>
  <owl:Class rdf:about="http://www.ontotext.com/proton/protonext#Airbase">
    <rdfs:subClassOf rdf:resource="http://www.ontotext.com/proton/protonext#MilitaryAreas"/>
    <rdfs:label xml:lang="en">Airbase</rdfs:label>
    <rdfs:comment xml:lang="en">An area used to store supplies, provide barracks for air force personnel, hangars and runways for aircraft, and from which operations are initiated</rdfs:comment>
  </owl:Class>
  <owl:Class rdf:about="http://www.ontotext.com/proton/protonext#SportEvent">
    <rdfs:subClassOf rdf:resource="http://www.ontotext.com/proton/protontop#Event"/>
    <rdfs:label xml:lang="en">Sport Event</rdfs:label>
    <rdfs:comment xml:lang="en">An event involving use, maintain or improve of physical fitness of its participants. Usually it is organized.</rdfs:comment>
  </owl:Class>
  <owl:Class rdf:about="http://www.ontotext.com/proton/protonext#Orchard">
    <rdfs:subClassOf>
      <owl:Class rdf:about="http://www.ontotext.com/proton/protonext#BiogeographicRegion"/>
    </rdfs:subClassOf>
    <rdfs:label xml:lang="en">Orchard</rdfs:label>
    <rdfs:comment xml:lang="en">A planting of fruit or nut trees</rdfs:comment>
  </owl:Class>
  <owl:Class rdf:about="http://www.ontotext.com/proton/protonext#BasketballLeague">
    <rdfs:subClassOf rdf:resource="http://www.ontotext.com/proton/protonext#SportsLeague"/>
    <rdfs:label xml:lang="en">Basketball League</rdfs:label>
    <rdfs:comment xml:lang="en">Any Basketball league</rdfs:comment>
  </owl:Class>
  <owl:Class rdf:about="http://www.ontotext.com/proton/protonext#AirplaneEngine">
    <rdfs:subClassOf rdf:resource="http://www.ontotext.com/proton/protonext#Machine"/>
    <rdfs:label xml:lang="en">Airplane Engine</rdfs:label>
    <rdfs:comment xml:lang="en">Engines of airplanes</rdfs:comment>
  </owl:Class>
  <owl:Class rdf:about="http://www.ontotext.com/proton/protonext#HockeyTeam">
    <rdfs:subClassOf>
      <owl:Class rdf:about="http://www.ontotext.com/proton/protonext#Team"/>
    </rdfs:subClassOf>
    <rdfs:label xml:lang="en">Hockey Team</rdfs:label>
    <rdfs:comment xml:lang="en">Any Hockey team</rdfs:comment>
  </owl:Class>
  <owl:Class rdf:about="http://www.ontotext.com/proton/protonext#Seachannels">
    <rdfs:subClassOf>
      <owl:Class rdf:about="http://www.ontotext.com/proton/protonext#LandRegion"/>
    </rdfs:subClassOf>
    <rdfs:label xml:lang="en">Seachannels</rdfs:label>
    <rdfs:comment xml:lang="en">Continuously sloping, elongated depressions commonly found in fans or plains and customarily bordered by levees on one or two sides (U.SCSU; U.SCSU)</rdfs:comment>
  </owl:Class>
  <owl:Class rdf:about="http://www.ontotext.com/proton/protonext#ArtPerformance">
    <rdfs:subClassOf rdf:resource="http://www.ontotext.com/proton/protontop#Event"/>
    <rdfs:label xml:lang="en">Art Performance</rdfs:label>
    <rdfs:comment xml:lang="en">A specific performance taking place at some moment, somewhere. Quite often starting at 19:00 in the theatre, stadium, etc.</rdfs:comment>
  </owl:Class>
  <owl:Class rdf:about="http://www.ontotext.com/proton/protonext#AmusementPark">
    <rdfs:subClassOf>
      <owl:Class rdf:about="http://www.ontotext.com/proton/protonext#RecreationalFacility"/>
    </rdfs:subClassOf>
    <rdfs:label xml:lang="en">Amusement Park</rdfs:label>
    <rdfs:comment xml:lang="en">(ADL FT) Commercially operated enterprises that offer rides, games, and other forms of entertainment. NIMA GNS designator - no equivalents.</rdfs:comment>
  </owl:Class>
  <owl:Class rdf:about="http://www.ontotext.com/proton/protonext#SportGamePoint">
    <rdfs:subClassOf rdf:resource="http://www.ontotext.com/proton/protontop#Situation"/>
    <rdfs:label xml:lang="en">Sport Game Point</rdfs:label>
    <rdfs:comment xml:lang="en">Denotes a point scored in a given sport game.</rdfs:comment>
  </owl:Class>
  <owl:Class rdf:about="http://www.ontotext.com/proton/protonext#BoardMeeting">
    <rdfs:subClassOf rdf:resource="http://www.ontotext.com/proton/protonext#Meeting"/>
    <rdfs:label xml:lang="en">Board Meeting</rdfs:label>
    <rdfs:comment xml:lang="en">A meeting whose main participants are members of a board.</rdfs:comment>
  </owl:Class>
  <owl:Class rdf:about="http://www.ontotext.com/proton/protonext#County">
    <rdfs:subClassOf>
      <owl:Class rdf:about="http://www.ontotext.com/proton/protonext#PoliticalRegion"/>
    </rdfs:subClassOf>
    <rdfs:subClassOf rdf:resource="http://www.ontotext.com/proton/protonext#PopulatedPlace"/>
    <rdfs:label xml:lang="en">County</rdfs:label>
    <rdfs:comment xml:lang="en">(ADL FT: Countries, 2nd order divisions) Second-order divisions of a nation such as parishes, boroughs, counties, municipios, or judicial divisions, and independent cities such as those in Maryland, Missouri, Nevada, and Virginia. [Adapted from USGS Circ 1048] We use this category for boroughs; for counties; for judicial divisions; for municipios; for parishes; and for second-order administrative divisions. NIMA GNS designator ADM2.</rdfs:comment>
  </owl:Class>
  <owl:Class rdf:about="http://www.ontotext.com/proton/protonext#Cove">
    <rdfs:subClassOf rdf:resource="http://www.ontotext.com/proton/protonext#Bay"/>
    <rdfs:label xml:lang="en">Cove</rdfs:label>
    <rdfs:comment xml:lang="en">a small type of bay or coastal inlet. http://www.eionet.europa.eu/gemet/concept/10142 NIMA GNS designator H.COVE.</rdfs:comment>
  </owl:Class>
  <owl:Class rdf:about="http://www.ontotext.com/proton/protonext#LandRegion">
    <rdfs:subClassOf rdf:resource="http://www.ontotext.com/proton/protontop#Location"/>
    <rdfs:label xml:lang="en">Land Region</rdfs:label>
    <rdfs:comment xml:lang="en">Any sort of land regions which are sort of natural, i.e. excluding urban areas, political and administrative regions. It combines number of ADL feature types under Physiographic features and Regions. Omitted ADL sub-classes: Badlands, Bars, Basins, Bight, Cirques, Cliffs, Dunes, Flats, Karst areas. Ledges, Massifs, Mineral deposit areas, Moraines, Natural rock formations, Arches, Playas, Seafloor Features, Tectonic features, Volcanic features (Volcano put under Mountain), Subcontinents. NIMA GNS designators FSR, FURU, HMCK, PLDR, RKFL, SINK, SLID, SLP, SLPU, TERU, TRR.</rdfs:comment>
  </owl:Class>
  <owl:Class rdf:about="http://www.ontotext.com/proton/protonext#Planet">
    <rdfs:subClassOf>
      <owl:Class rdf:about="http://www.ontotext.com/proton/protonext#AstronomicalObject"/>
    </rdfs:subClassOf>
    <rdfs:label xml:lang="en">Planet</rdfs:label>
    <rdfs:comment xml:lang="en">Any of the celestial bodies (other than comets or satellites) that revolve around the sun in the solar system. Definition partly derived from WordNet 1.7</rdfs:comment>
  </owl:Class>
  <owl:Class rdf:about="http://www.ontotext.com/proton/protonext#PoliticalParty">
    <rdfs:subClassOf rdf:resource="http://www.ontotext.com/proton/protonext#PoliticalEntity"/>
    <rdfs:label xml:lang="en">Political Party</rdfs:label>
    <rdfs:comment xml:lang="en">An organization to gain political power. Definition taken from WordNet 1.7</rdfs:comment>
  </owl:Class>
  <owl:Class rdf:about="http://www.ontotext.com/proton/protonext#CountryCapital">
    <rdfs:subClassOf rdf:resource="http://www.ontotext.com/proton/protonext#Capital"/>
    <rdfs:label xml:lang="en">Country Capital</rdfs:label>
    <rdfs:comment xml:lang="en">A capital of a Country. NIMA GNS designator PPLC.</rdfs:comment>
  </owl:Class>
  <owl:Class rdf:about="http://www.ontotext.com/proton/protonext#DataSchema">
    <rdfs:subClassOf rdf:resource="http://www.ontotext.com/proton/protontop#InformationResource"/>
    <rdfs:label xml:lang="en">Data Schema</rdfs:label>
    <rdfs:comment xml:lang="en">A particular notation for representation, standardization, and/or structuring of infomation. It can range from db schema, through ontology, to any sort of taxonomies, nomenclatures and subject hierarchies. Examples are Dublin Core, KIMO, SIC, XML, RDFS</rdfs:comment>
  </owl:Class>
  <owl:Class rdf:about="http://www.ontotext.com/proton/protonext#TransportFacility">
    <rdfs:subClassOf rdf:resource="http://www.ontotext.com/proton/protonext#Facility"/>
    <rdfs:label xml:lang="en">Transport Facility</rdfs:label>
    <rdfs:comment xml:lang="en">(ADL FT: Transportation Features) We use this category for air routes; for caravan routes; for corridors; for crossings; for depots; for ferries; for fords (crossings); for fuel depots; for gates (manmade); for halting places (transportation); for highway maintenance sites; for portages; for rest houses; for routes; for ship tracks; for stock routes; for terminals (transportation); and for transit facilities. Omitted sub-classes: Aqueducts, Cableways, Parking Sites. NIMA GNS designator - no direct equivalents.</rdfs:comment>
  </owl:Class>
  <owl:Class rdf:about="http://www.ontotext.com/proton/protonext#Science">
    <rdfs:subClassOf rdf:resource="http://www.ontotext.com/proton/protonext#ResearchArea"/>
    <rdfs:label xml:lang="en">Science</rdfs:label>
    <rdfs:comment xml:lang="en">A well established, big research area</rdfs:comment>
  </owl:Class>
  <owl:Class rdf:about="http://www.ontotext.com/proton/protonext#Section">
    <rdfs:subClassOf rdf:resource="http://www.ontotext.com/proton/protontop#InformationResource"/>
    <rdfs:label>Section</rdfs:label>
    <rdfs:comment xml:lang="en">An area of a document that can be considered a document in itself. Compare with pext:Mention, which is also an area of a document. Imported from the iSIM ontology.</rdfs:comment>
  </owl:Class>
  <owl:Class rdf:about="http://www.ontotext.com/proton/protonext#LocationOfSpecialInterest">
    <rdfs:subClassOf rdf:resource="http://www.ontotext.com/proton/protontop#Location"/>
    <rdfs:label xml:lang="en">Location of Special Interest</rdfs:label>
    <rdfs:comment xml:lang="en">Any place with some particular value, which triggers interest.</rdfs:comment>
  </owl:Class>
  <owl:Class rdf:about="http://www.ontotext.com/proton/protonext#ATM">
    <rdfs:subClassOf>
      <owl:Class rdf:about="http://www.ontotext.com/proton/protonext#TelecomFacility"/>
    </rdfs:subClassOf>
    <rdfs:label xml:lang="en">Automatic Teller Machine (ATM)</rdfs:label>
    <rdfs:comment xml:lang="en">An unattended electronic machine in a public place, connected to a data system and related equipment and activated by a bank customer to obtain cash withdrawals and other banking services.</rdfs:comment>
  </owl:Class>
  <owl:Class rdf:about="http://www.ontotext.com/proton/protonext#Reptile">
    <rdfs:subClassOf rdf:resource="http://www.ontotext.com/proton/protonext#Animal"/>
    <rdfs:label xml:lang="en">Reptile</rdfs:label>
    <rdfs:comment xml:lang="en">Reptiles are animals in the class Reptilia. They are characterized by breathing air, laying shelled eggs, and having skin covered in scales and/or scutes. Reptiles are classically viewed as having a "cold-blooded" metabolism. They are tetrapods. Modern reptiles inhabit every continent with the exception of Antarctica. Example of an reptile is the crocodile. (Wikipedia)</rdfs:comment>
  </owl:Class>
  <owl:Class rdf:about="http://www.ontotext.com/proton/protonext#Crustacean">
    <rdfs:subClassOf rdf:resource="http://www.ontotext.com/proton/protonext#Animal"/>
    <rdfs:label xml:lang="en">Crustacean</rdfs:label>
    <rdfs:comment xml:lang="en">Crustaceans denotes a group of arthropods animals, which includes crabs, lobsters, crayfish, shrimp, krill and barnacles. (Wikipedia)</rdfs:comment>
  </owl:Class>
  <owl:Class rdf:about="http://www.ontotext.com/proton/protonext#ForestClearing">
    <rdfs:subClassOf>
      <owl:Class rdf:about="http://www.ontotext.com/proton/protonext#BiogeographicRegion"/>
    </rdfs:subClassOf>
    <rdfs:label xml:lang="en">Clearing</rdfs:label>
    <rdfs:comment xml:lang="en">An area in a forest with trees removed. NIMA GNS designator L.CLG.</rdfs:comment>
  </owl:Class>
  <owl:Class rdf:about="http://www.ontotext.com/proton/protonext#TelecomFacility">
    <rdfs:subClassOf rdf:resource="http://www.ontotext.com/proton/protonext#Facility"/>
    <rdfs:label xml:lang="en">Telecom Facility</rdfs:label>
    <rdfs:comment xml:lang="en">(ADL FT: Telecommunication Features) We use this category for antenna field sites; for communication centers; for radio stations; for television stations; and for transmission lines. NIMA GNS designators COMC, STNR, STNS.</rdfs:comment>
  </owl:Class>
  <owl:Class rdf:about="http://www.ontotext.com/proton/protonext#TennisLeague">
    <rdfs:subClassOf rdf:resource="http://www.ontotext.com/proton/protonext#SportsLeague"/>
    <rdfs:label xml:lang="en">Tennis League</rdfs:label>
    <rdfs:comment xml:lang="en">Any Tennis league</rdfs:comment>
  </owl:Class>
  <owl:Class rdf:about="http://www.ontotext.com/proton/protonext#BiogeographicRegion">
    <rdfs:subClassOf rdf:resource="http://www.ontotext.com/proton/protonext#LandRegion"/>
    <rdfs:label xml:lang="en">Biogeographic Region</rdfs:label>
    <rdfs:comment xml:lang="en">(ADL FT) Geographic regions characterized chiefly by the dominant forms of plant life and the prevailing climate. [Adapted from American Heritage Dict. of the English Language, 4th ed.] We use this category for biomes; for ecoregions; and for vegetation. Omitted ADL sub-classes: Barren lands, Grasslands, Habitats, Snow Regions, Wetlands. NIMA GNS designator - no equivalent. Some correspondence to class Hypsographic Features.</rdfs:comment>
  </owl:Class>
  <owl:Class rdf:about="http://www.ontotext.com/proton/protonext#Stadium">
    <rdfs:subClassOf>
      <owl:Class rdf:about="http://www.ontotext.com/proton/protonext#SportBuilding"/>
    </rdfs:subClassOf>
    <rdfs:label xml:lang="en">Stadium</rdfs:label>
    <rdfs:comment xml:lang="en">A special sort of sport building, usually for open-air sports such as soccer.</rdfs:comment>
  </owl:Class>
  <owl:Class rdf:about="http://www.ontotext.com/proton/protonext#MusicalComposition">
    <rdfs:subClassOf rdf:resource="http://www.ontotext.com/proton/protonext#MediaProduct"/>
    <rdfs:label xml:lang="en">Musical Composition</rdfs:label>
    <rdfs:comment xml:lang="en">An original piece of music.</rdfs:comment>
  </owl:Class>
  <owl:Class rdf:about="http://www.ontotext.com/proton/protonext#Reef">
    <rdfs:subClassOf rdf:resource="http://www.ontotext.com/proton/protonext#LandRegion"/>
    <rdfs:label xml:lang="en">Reef</rdfs:label>
    <rdfs:comment xml:lang="en">(ADL FT) Chains of rocks or coral at or near the surface of water. [USGS Circ 1048] We use this category for barrier reefs; and for fringing reefs. Collapsed ADL sub-class: Coral Reefs. NIMA GNS designator RF, RFSU, RFU, RFC, H.RFX.</rdfs:comment>
  </owl:Class>
  <owl:Class rdf:about="http://www.ontotext.com/proton/protonext#Order">
    <rdfs:subClassOf rdf:resource="http://www.ontotext.com/proton/protontop#Statement"/>
    <rdfs:label xml:lang="en">Order</rdfs:label>
    <rdfs:comment xml:lang="en">A statement used to request someone to supply something in return for payment and providing specifications and quantities. WordNet 2.1.</rdfs:comment>
  </owl:Class>
  <owl:Class rdf:about="http://www.ontotext.com/proton/protonext#Star">
    <rdfs:subClassOf>
      <owl:Class rdf:about="http://www.ontotext.com/proton/protonext#AstronomicalObject"/>
    </rdfs:subClassOf>
    <rdfs:label xml:lang="en">Star</rdfs:label>
    <rdfs:comment xml:lang="en">An astronomic object of hot gases that radiates energy derived from thermonuclear reactions in the interior. Definition partly derived from WordNet 1.7</rdfs:comment>
  </owl:Class>
  <owl:Class rdf:about="http://www.ontotext.com/proton/protonext#Ideology">
    <rdfs:subClassOf>
      <owl:Class rdf:about="http://www.ontotext.com/proton/protonext#SocialAbstraction"/>
    </rdfs:subClassOf>
    <rdfs:label xml:lang="en">Ideology</rdfs:label>
    <rdfs:comment xml:lang="en">An ideology is a set of ideas that constitute one's goals, expectations, and actions. Wikipedia.</rdfs:comment>
  </owl:Class>
  <owl:Class rdf:about="http://www.ontotext.com/proton/protonext#Marsh">
    <rdfs:subClassOf>
      <owl:Class rdf:about="http://www.ontotext.com/proton/protonext#WaterRegion"/>
    </rdfs:subClassOf>
    <rdfs:label xml:lang="en">Marsh</rdfs:label>
    <rdfs:comment xml:lang="en">An area of open ground overlaid with wet peaty soils; a wetland dominated by grass-like vegetation; a flat area, subject to periodic salt water inundation, dominated by grassy salt-tolerant plants; a salt flat or salt encrusted plain subject to periodic inundation from flooding or high tides</rdfs:comment>
  </owl:Class>
  <owl:Class rdf:about="http://www.ontotext.com/proton/protonext#MusicFestival">
    <rdfs:subClassOf rdf:resource="http://www.ontotext.com/proton/protonext#Festival"/>
    <rdfs:label xml:lang="en">Music Festival</rdfs:label>
    <rdfs:comment xml:lang="en">Any festival involving playing music.</rdfs:comment>
  </owl:Class>
  <owl:Class rdf:about="http://www.ontotext.com/proton/protonext#Fungus">
    <rdfs:subClassOf rdf:resource="http://www.ontotext.com/proton/protonext#LivingObject"/>
    <rdfs:label xml:lang="en">Fungus</rdfs:label>
    <rdfs:comment xml:lang="en">Fungus is a member of a large group of eukaryotic organisms that includes microorganisms such as yeasts and molds (Wikipedia)</rdfs:comment>
  </owl:Class>
  <owl:Class rdf:about="http://www.ontotext.com/proton/protonext#Valley">
    <rdfs:subClassOf rdf:resource="http://www.ontotext.com/proton/protonext#LandRegion"/>
    <rdfs:label xml:lang="en">Valley</rdfs:label>
    <rdfs:comment xml:lang="en">(ADL FT) Low-lying land bordered by higher ground; especially elongate, relatively large gently sloping depressions of the Earth's surface, commonly situated between two mountains or between ranges of hills or mountains, and often containing a stream with an outlet. [Glossary of Geology, 4th ed.] We use this category for forks (physiographic features); for glens; for hanging valleys; for hollows; for median valleys; and for shelf valleys (seafloor). NIMA GNS designators VAL, VALG, VALU, VALS, VALX, VLSU, FRKU, FRSU, MDVU, SHVU.</rdfs:comment>
  </owl:Class>
  <owl:Class rdf:about="http://www.ontotext.com/proton/protonext#FootballMatch">
    <rdfs:subClassOf rdf:resource="http://www.ontotext.com/proton/protonext#SportGame"/>
    <rdfs:label xml:lang="en">Football match</rdfs:label>
    <rdfs:comment xml:lang="en">Any instance of a soccer match.</rdfs:comment>
  </owl:Class>
  <owl:Class rdf:about="http://www.ontotext.com/proton/protonext#Activity">
    <rdfs:subClassOf rdf:resource="http://www.ontotext.com/proton/protontop#Happening"/>
    <rdfs:label xml:lang="en">Activity</rdfs:label>
    <rdfs:comment xml:lang="en">Each activity is a Happening which involves volition and participants. It has temporal dimension. It is distinguished from Events by the fact that the activity does not trigger change of state and does not have a conceptual end point.</rdfs:comment>
  </owl:Class>
  <owl:Class rdf:about="http://www.ontotext.com/proton/protonext#Village">
    <rdfs:subClassOf rdf:resource="http://www.ontotext.com/proton/protonext#Settlement"/>
    <rdfs:label xml:lang="en">Village</rdfs:label>
    <rdfs:comment xml:lang="en">Any village</rdfs:comment>
  </owl:Class>
  <owl:Class rdf:about="http://www.ontotext.com/proton/protonext#Holiday">
    <rdfs:subClassOf>
      <owl:Class rdf:about="http://www.ontotext.com/proton/protonext#Date"/>
    </rdfs:subClassOf>
    <rdfs:label xml:lang="en">Holiday</rdfs:label>
    <rdfs:comment xml:lang="en">A Holiday is a day designated as having special significance for which individuals, a government, or a religious group have deemed that observance is warranted. Wikipedia</rdfs:comment>
  </owl:Class>
  <owl:Class rdf:about="http://www.ontotext.com/proton/protonext#Patent">
    <rdfs:subClassOf rdf:resource="http://www.ontotext.com/proton/protontop#InformationResource"/>
    <rdfs:label xml:lang="en">Patent</rdfs:label>
    <rdfs:comment xml:lang="en">A registered (or awaiting registration) patent for specific invention or design.</rdfs:comment>
  </owl:Class>
  <owl:Class rdf:about="http://www.ontotext.com/proton/protonext#IPAddress">
    <rdfs:subClassOf rdf:resource="http://www.ontotext.com/proton/protonext#InternetAddress"/>
    <rdfs:label xml:lang="en">IP Address</rdfs:label>
    <rdfs:comment xml:lang="en">An Internet Protocol address (IP address) is a numerical label assigned to each device (e.g., computer, printer) participating in a computer network that uses the Internet Protocol for communication. Wikipedia</rdfs:comment>
  </owl:Class>
  <owl:Class rdf:about="http://www.ontotext.com/proton/protonext#EducationalOrganization">
    <rdfs:subClassOf rdf:resource="http://www.ontotext.com/proton/protontop#Organization"/>
    <rdfs:label xml:lang="en">Educational Organization</rdfs:label>
    <rdfs:comment xml:lang="en">An organization devoted to teaching activities.</rdfs:comment>
  </owl:Class>
  <owl:Class rdf:about="http://www.ontotext.com/proton/protonext#Gap">
    <rdfs:subClassOf rdf:resource="http://www.ontotext.com/proton/protonext#LandRegion"/>
    <rdfs:label xml:lang="en">Gap</rdfs:label>
    <rdfs:comment xml:lang="en">(ADL FT) Ravines or gorges cut deeply through mountain ridges, or between hills or mountains. We use this category for cols; for defiles; for passes; for saddles (physiographic); and for sills (physiographic). NIMA GNS designator GAP, GAPU, GAPF, PASS, SILL, SILU.</rdfs:comment>
  </owl:Class>
  <owl:Class rdf:about="http://www.ontotext.com/proton/protonext#TelevisionEpisode">
    <rdfs:subClassOf rdf:resource="http://www.ontotext.com/proton/protonext#TelevisionProduct"/>
    <rdfs:label xml:lang="en">Television Episode</rdfs:label>
    <rdfs:comment xml:lang="en">Denotes any episod of any television series.</rdfs:comment>
  </owl:Class>
  <owl:Class rdf:about="http://www.ontotext.com/proton/protonext#WaterRegion">
    <rdfs:subClassOf rdf:resource="http://www.ontotext.com/proton/protontop#Location"/>
    <rdfs:label xml:lang="en">Water Region</rdfs:label>
    <rdfs:comment xml:lang="en">(ADL FT: Hydrographic Features) For natural bodies of water. For constructed waterways, reservoirs, and such, use 'hydrographic structures'. We use this category for bodies of water; for eddies; for fluvial features; for marine features; for overfalls; for upwellings; for water bodies; for waterholes; and for whirlpools. Many of the ADL hydrographic features ignored. NIMA GNS class H.</rdfs:comment>
  </owl:Class>
  <owl:Class rdf:about="http://www.ontotext.com/proton/protonext#TemporalAbstraction">
    <rdfs:subClassOf rdf:resource="http://www.ontotext.com/proton/protontop#Abstract"/>
    <rdfs:label xml:lang="en">Temporal Abstraction</rdfs:label>
    <rdfs:comment xml:lang="en">Any sort of abstraction used to refer to specific periods of time. Thus, the month of September is an instance of this class, while Sept 1989 is not (it is a specific TimeInterval, and thus not abstract)</rdfs:comment>
  </owl:Class>
  <owl:Class rdf:about="http://www.ontotext.com/proton/protonext#Election">
    <rdfs:subClassOf rdf:resource="http://www.ontotext.com/proton/protonext#RecurringEvent"/>
    <rdfs:label xml:lang="en">Election</rdfs:label>
    <rdfs:comment xml:lang="en">Generic concept of Election which is normally held at regular periods of time, president elections of the US, municipal elections, etc..</rdfs:comment>
  </owl:Class>
  <owl:Class rdf:about="http://www.ontotext.com/proton/protonext#Woman">
    <rdfs:subClassOf>
      <owl:Class rdf:about="http://www.ontotext.com/proton/protonext#Human"/>
    </rdfs:subClassOf>
    <rdfs:subClassOf rdf:resource="http://www.ontotext.com/proton/protontop#Person"/>
    <rdfs:label xml:lang="en">Woman</rdfs:label>
    <rdfs:comment xml:lang="en">A female human.</rdfs:comment>
  </owl:Class>
  <owl:Class rdf:about="http://www.ontotext.com/proton/protonext#InternetDomain">
    <rdfs:subClassOf rdf:resource="http://www.ontotext.com/proton/protonext#InternetAddress"/>
    <rdfs:label xml:lang="en">Internet Domain</rdfs:label>
    <rdfs:comment xml:lang="en">A domain name is an identification string that defines the area of administrative autonomy, authority, or control in the Internet. Wikipedia.</rdfs:comment>
  </owl:Class>
  <owl:Class rdf:about="http://www.ontotext.com/proton/protonext#DrainageBasin">
    <rdfs:subClassOf rdf:resource="http://www.ontotext.com/proton/protonext#LandRegion"/>
    <rdfs:label xml:lang="en">Drainage Basin</rdfs:label>
    <rdfs:comment xml:lang="en">An area drained by a stream. NIMA GNS designator L.BSND.</rdfs:comment>
  </owl:Class>
  <owl:Class rdf:about="http://www.ontotext.com/proton/protonext#HistoricPlace">
    <rdfs:subClassOf rdf:resource="http://www.ontotext.com/proton/protonext#LocationOfSpecialInterest"/>
    <rdfs:label xml:lang="en">Historic Place</rdfs:label>
    <rdfs:comment xml:lang="en">Any Historic Place, an old place with historic value.</rdfs:comment>
  </owl:Class>
  <owl:Class rdf:about="http://www.ontotext.com/proton/protonext#PaintballLeague">
    <rdfs:subClassOf rdf:resource="http://www.ontotext.com/proton/protonext#SportsLeague"/>
    <rdfs:label xml:lang="en">Paintball League</rdfs:label>
    <rdfs:comment xml:lang="en">Any Paintball league</rdfs:comment>
  </owl:Class>
  <owl:Class rdf:about="http://www.ontotext.com/proton/protonext#ElectionOccurrence">
    <rdfs:subClassOf rdf:resource="http://www.ontotext.com/proton/protontop#Event"/>
    <rdfs:label xml:lang="en">Election</rdfs:label>
    <rdfs:comment xml:lang="en">Election happening at a particular date.</rdfs:comment>
  </owl:Class>
  <owl:Class rdf:about="http://www.ontotext.com/proton/protonext#LacrosseLeague">
    <rdfs:subClassOf rdf:resource="http://www.ontotext.com/proton/protonext#SportsLeague"/>
    <rdfs:label xml:lang="en">Lacrosse League</rdfs:label>
    <rdfs:comment xml:lang="en">Any Lacrosse league</rdfs:comment>
  </owl:Class>
  <owl:Class rdf:about="http://www.ontotext.com/proton/protonext#Heath">
    <rdfs:subClassOf rdf:resource="http://www.ontotext.com/proton/protonext#BiogeographicRegion"/>
    <rdfs:label xml:lang="en">Heath</rdfs:label>
    <rdfs:comment xml:lang="en">An upland moor or sandy area dominated by low shrubby vegetation including heather</rdfs:comment>
  </owl:Class>
  <owl:Class rdf:about="http://www.ontotext.com/proton/protonext#Icecap">
    <rdfs:subClassOf rdf:resource="http://www.ontotext.com/proton/protonext#LandRegion"/>
    <rdfs:label xml:lang="en">Icecap</rdfs:label>
    <rdfs:comment xml:lang="en">A dome-shaped mass of glacial ice covering an area of mountain summits or other high lands; smaller than an ice sheet</rdfs:comment>
  </owl:Class>
  <owl:Class rdf:about="http://www.ontotext.com/proton/protonext#InternationalOrganization">
    <rdfs:subClassOf rdf:resource="http://www.ontotext.com/proton/protontop#Organization"/>
    <rdfs:label xml:lang="en">International Organization</rdfs:label>
    <rdfs:comment xml:lang="en">Legal international organization. Legal in this case means officially recognized by more than one government.</rdfs:comment>
  </owl:Class>
  <owl:Class rdf:about="http://www.ontotext.com/proton/protonext#Harbor">
    <rdfs:subClassOf rdf:resource="http://www.ontotext.com/proton/protonext#HydrographicStructure"/>
    <rdfs:subClassOf rdf:resource="http://www.ontotext.com/proton/protonext#WaterRegion"/>
    <rdfs:label xml:lang="en">Harbor</rdfs:label>
    <rdfs:comment xml:lang="en">(ADL FT) Sheltered areas of water where ships or other watercraft can anchor or dock. We use this category for anchorages; for anclajes; for boat yards; for boatyards; for dock yards; for docking basins; for dockyards; for dry docks; for harbors; for marine terminals; for moorings; for ports; for roadsteads (anchorages); and for turning basins. The following sub-classes included (i.e. not-distinguishable): Marinas, Piers. NIMA GNS designators HBR, HBRX, MAR, BTYD, PIER, DCK, DCKB, DCKY, PRT, AIRS.</rdfs:comment>
  </owl:Class>
  <owl:Class rdf:about="http://www.ontotext.com/proton/protonext#Lake">
    <rdfs:subClassOf rdf:resource="http://www.ontotext.com/proton/protonext#WaterRegion"/>
    <rdfs:label xml:lang="en">Lake</rdfs:label>
    <rdfs:comment xml:lang="en">(ADL FT) Use 'reservoirs' for human engineered lakes. Natural inland bodies of standing water, generally of appreciable size, occupying a depression in the Earth's surface. [Adapted from Glossary of Geology, 4th ed.] We use this category for beaver ponds; for crater lakes; for dry lakes; for fish ponds; for fishponds; for inland seas; for intermittent lakes; for intermittent oxbow lakes; for intermittent ponds; for intermittent pools; for intermittent salt lakes; for intermittent salt ponds; for lagoons; for laguna; for lake beds; for lochs; for millponds; for oxbow lakes; for ponds; for pools (water bodies); for salt evaporation ponds; for salt lakes; for salt ponds; and for tarns. NIMA GNS designators LBED, LK, LKC, LKI, LKN, LKNI, LKO, LKOI, LKS, LKSB, LKSC, LKSI, LKSN, LKSNI, LKX</rdfs:comment>
  </owl:Class>
  <owl:Class rdf:about="http://www.ontotext.com/proton/protonext#JobTitle">
    <rdfs:subClassOf>
      <owl:Class rdf:about="http://www.ontotext.com/proton/protonext#SocialFunction"/>
    </rdfs:subClassOf>
    <rdfs:label xml:lang="en">Job Title</rdfs:label>
    <rdfs:comment xml:lang="en">The name of a position a person holds within an organization.</rdfs:comment>
  </owl:Class>
  <owl:Class rdf:about="http://www.ontotext.com/proton/protonext#Tunnel">
    <rdfs:subClassOf rdf:resource="http://www.ontotext.com/proton/protonext#TransportFacility"/>
    <rdfs:label xml:lang="en">Tunnel</rdfs:label>
    <rdfs:comment xml:lang="en">(ADL FT) Underground or underwater passages. [USGS Circ 1048] We use this category for canal tunnels; for railroad tunnels; and for road tunnels. NIMA GNS designator TNL, TNLC, TNLN, TNLRD, TNLS</rdfs:comment>
  </owl:Class>
  <owl:Class rdf:about="http://www.ontotext.com/proton/protonext#CalendarMonth">
    <rdfs:subClassOf rdf:resource="http://www.ontotext.com/proton/protonext#TemporalAbstraction"/>
    <rdfs:label xml:lang="en">Calendar Month</rdfs:label>
    <rdfs:comment xml:lang="en">A specific month of the year, such as: Jan., Feb., etc.</rdfs:comment>
  </owl:Class>
  <owl:Class rdf:about="http://www.ontotext.com/proton/protonext#Town">
    <rdfs:subClassOf rdf:resource="http://www.ontotext.com/proton/protonext#Settlement"/>
    <rdfs:label xml:lang="en">Town</rdfs:label>
    <rdfs:comment xml:lang="en">Any town</rdfs:comment>
  </owl:Class>
  <owl:Class rdf:about="http://www.ontotext.com/proton/protonext#Software">
    <rdfs:subClassOf rdf:resource="http://www.ontotext.com/proton/protontop#ProductModel"/>
    <rdfs:label xml:lang="en">Software</rdfs:label>
    <rdfs:comment xml:lang="en">Software is a collection of computer programs and related data that provide the instructions telling a computer what to do. (Wikipedia)</rdfs:comment>
  </owl:Class>
  <owl:Class rdf:about="http://www.ontotext.com/proton/protonext#MountainSummit">
    <rdfs:subClassOf>
      <owl:Class rdf:about="http://www.ontotext.com/proton/protonext#Mountain"/>
    </rdfs:subClassOf>
    <rdfs:label xml:lang="en">Mountain Summit</rdfs:label>
    <rdfs:comment xml:lang="en">(ADL FT) Peaks of mountains. [USGS Circ 1048] We use this category for ahus; for mountain crests; for nunataks; for peaks; and for summits. NIMA GNS designators PK, PKS, PKSU, PKU.</rdfs:comment>
  </owl:Class>
  <owl:Class rdf:about="http://www.ontotext.com/proton/protonext#Sculpture">
    <rdfs:subClassOf rdf:resource="http://www.ontotext.com/proton/protonext#PieceOfArt"/>
    <rdfs:label xml:lang="en">Sculpture</rdfs:label>
    <rdfs:comment xml:lang="en">Any sculpture, three-dimensional artwork created by shaping or combining hard materials. (Wikipedia)</rdfs:comment>
  </owl:Class>
  <owl:Class rdf:about="http://www.ontotext.com/proton/protonext#Insect">
    <rdfs:subClassOf rdf:resource="http://www.ontotext.com/proton/protonext#Animal"/>
    <rdfs:label xml:lang="en">Insect</rdfs:label>
    <rdfs:comment xml:lang="en">Insects are a class within the arthropods that have a chitinous exoskeleton, a three-part body (head, thorax, and abdomen), three pairs of jointed legs, compound eyes, and two antennae. (Wikipedia)</rdfs:comment>
  </owl:Class>
  <owl:Class rdf:about="http://www.ontotext.com/proton/protonext#SeaTongue">
    <rdfs:subClassOf rdf:resource="http://www.ontotext.com/proton/protonext#LandRegion"/>
    <rdfs:label xml:lang="en">Tongue</rdfs:label>
    <rdfs:comment xml:lang="en">An elongate (tongue-like) extension of a flat sea floor into an adjacent higher feature</rdfs:comment>
  </owl:Class>
  <owl:Class rdf:about="http://www.ontotext.com/proton/protonext#MixedMartialArtsLeague">
    <rdfs:subClassOf rdf:resource="http://www.ontotext.com/proton/protonext#SportsLeague"/>
    <rdfs:label xml:lang="en">Mixed Martial Arts League</rdfs:label>
    <rdfs:comment xml:lang="en">Any Mixed Martial Arts league</rdfs:comment>
  </owl:Class>
  <owl:Class rdf:about="http://www.ontotext.com/proton/protonext#Currency">
    <rdfs:subClassOf rdf:resource="http://www.ontotext.com/proton/protontop#Object"/>
    <rdfs:label xml:lang="en">Currency</rdfs:label>
    <rdfs:comment xml:lang="en">Specific currency, usually national</rdfs:comment>
  </owl:Class>
  <owl:Class rdf:about="http://www.ontotext.com/proton/protonext#WaterBank">
    <rdfs:subClassOf rdf:resource="http://www.ontotext.com/proton/protonext#LandRegion"/>
    <rdfs:label xml:lang="en">Water Bank</rdfs:label>
    <rdfs:comment xml:lang="en">(ADL FT: Banks) Sloping margins of, or the ground bordering, a stream, and serving to confine the water to the natural channel during the normal course of flow. [Glossary of Geology, 4th ed.] We use this category for stream banks. NIMA GNS designator BKSU, BNK, BNKR, BNKU, BNKX.</rdfs:comment>
  </owl:Class>
  <owl:Class rdf:about="http://www.ontotext.com/proton/protonext#LymphNode">
    <rdfs:subClassOf rdf:resource="http://www.ontotext.com/proton/protonext#BodyPart"/>
    <rdfs:label xml:lang="en">Lymphatic Node</rdfs:label>
    <rdfs:comment xml:lang="en">Lymph is a general concept gathering all lymph nodes of the body.</rdfs:comment>
  </owl:Class>
  <owl:Class rdf:about="http://www.ontotext.com/proton/protonext#NobeltyTitle">
    <rdfs:subClassOf>
      <owl:Class rdf:about="http://www.ontotext.com/proton/protonext#SocialFunction"/>
    </rdfs:subClassOf>
    <rdfs:label xml:lang="en">Nobelty</rdfs:label>
    <rdfs:comment xml:lang="en">The social function of a nobelty.</rdfs:comment>
  </owl:Class>
  <owl:Class rdf:about="http://www.ontotext.com/proton/protonext#PublicCompany">
    <rdfs:subClassOf rdf:resource="http://www.ontotext.com/proton/protonext#Company"/>
    <rdfs:label xml:lang="en">Public Company</rdfs:label>
    <rdfs:comment xml:lang="en">Company which is publicly traded on a Stock Exchange.</rdfs:comment>
  </owl:Class>
  <owl:Class rdf:about="http://www.ontotext.com/proton/protonext#Ocean">
    <rdfs:subClassOf>
      <owl:Class rdf:about="http://www.ontotext.com/proton/protonext#Sea"/>
    </rdfs:subClassOf>
    <rdfs:label xml:lang="en">Ocean</rdfs:label>
    <rdfs:comment xml:lang="en">(ADL FT) Continuous salt-water bodies that surround the continents and fill the Earth's great depressions. NIMA GNS designator OCN</rdfs:comment>
  </owl:Class>
  <owl:Class rdf:about="http://www.ontotext.com/proton/protonext#ChemicalElement">
    <rdfs:subClassOf rdf:resource="http://www.ontotext.com/proton/protonext#ChemicalSubstance"/>
    <rdfs:label xml:lang="en">Chemical element</rdfs:label>
    <rdfs:comment xml:lang="en">A chemical element is a pure chemical substance consisting of one type of atom distinguished by its atomic number, which is the number of protons in its nucleus. Wikipedia</rdfs:comment>
  </owl:Class>
  <owl:Class rdf:about="http://www.ontotext.com/proton/protonext#River">
    <rdfs:subClassOf rdf:resource="http://www.ontotext.com/proton/protonext#Stream"/>
    <rdfs:label xml:lang="en">River</rdfs:label>
    <rdfs:comment xml:lang="en">(ADL FT) Natural freshwater surface streams of considerable volume and a permanent or seasonal flow, moving in a definite channel toward a sea, lake, or another river; any large streams, or ones larger than brooks or creeks, such as the trunk stream and larger branches of a drainage system. We use this category for rios. NIM GNS designators ... no direct equivalents!</rdfs:comment>
  </owl:Class>
  <owl:Class rdf:about="http://www.ontotext.com/proton/protonext#University">
    <rdfs:subClassOf rdf:resource="http://www.ontotext.com/proton/protonext#EducationalOrganization"/>
    <rdfs:subClassOf rdf:resource="http://www.ontotext.com/proton/protonext#ResearchOrganization"/>
    <rdfs:label xml:lang="en">University</rdfs:label>
    <rdfs:comment xml:lang="en">An educational organization higher than school.</rdfs:comment>
  </owl:Class>
  <owl:Class rdf:about="http://www.ontotext.com/proton/protonext#PositionOrganization">
    <rdfs:subClassOf rdf:resource="http://www.ontotext.com/proton/protontop#Situation"/>
    <rdfs:label xml:lang="en">Position in an organization</rdfs:label>
    <rdfs:comment xml:lang="en">The situation of a job position which is available in a particular organization, such as CEO, CTO, executive assistant, etc.</rdfs:comment>
  </owl:Class>
  <owl:Class rdf:about="http://www.ontotext.com/proton/protonext#Spring">
    <rdfs:subClassOf rdf:resource="http://www.ontotext.com/proton/protonext#WaterRegion"/>
    <rdfs:label xml:lang="en">Spring</rdfs:label>
    <rdfs:comment xml:lang="en">(ADL FT) Places where underground water flows naturally to the surface of the Earth. ... We use this category for mineral springs; and for sulfur springs. NIMA GNS designators SPNG, SPNS, SPNT.</rdfs:comment>
  </owl:Class>
  <owl:Class rdf:about="http://www.ontotext.com/proton/protonext#Archaea">
    <rdfs:subClassOf rdf:resource="http://www.ontotext.com/proton/protonext#LivingObject"/>
    <rdfs:label xml:lang="en">Archaea</rdfs:label>
    <rdfs:comment xml:lang="en">Archaea (archeon) are a group of single-celled microorganisms without a cell nucleus or any other membrane-bound organelles (Wikipedia)</rdfs:comment>
  </owl:Class>
  <owl:Class rdf:about="http://www.ontotext.com/proton/protonext#GovernmentAgency">
    <rdfs:subClassOf rdf:resource="http://www.ontotext.com/proton/protonext#GovernmentOrganization"/>
    <rdfs:label xml:lang="en">Government</rdfs:label>
    <rdfs:comment xml:lang="en">A government agency is a permanent or semi-permanent organization in the machinery of government that is responsible for the oversight and administration of specific functions, such as an intelligence agency. DBPedia</rdfs:comment>
    <rdfs:comment xml:lang="en">The governmental cabinet</rdfs:comment>
  </owl:Class>
  <owl:Class rdf:about="http://www.ontotext.com/proton/protonext#PetroleumBasin">
    <rdfs:subClassOf>
      <owl:Class rdf:about="http://www.ontotext.com/proton/protonext#OilField"/>
    </rdfs:subClassOf>
    <rdfs:label xml:lang="en">Petroleum Basin</rdfs:label>
    <rdfs:comment xml:lang="en">An area underlain by an oil-rich structural basin. NIMA GNS designator L.BSNP.</rdfs:comment>
  </owl:Class>
  <owl:Class rdf:about="http://www.ontotext.com/proton/protonext#ZipCode">
    <rdfs:subClassOf rdf:resource="http://www.ontotext.com/proton/protontop#ContactInformation"/>
    <rdfs:label xml:lang="en">ZipCode</rdfs:label>
    <rdfs:comment xml:lang="en">Part of a postal address denoting the zip code.</rdfs:comment>
  </owl:Class>
  <owl:Class rdf:about="http://www.ontotext.com/proton/protonext#ComicsCharacter">
    <rdfs:subClassOf rdf:resource="http://www.ontotext.com/proton/protonext#FictionalCharacter"/>
    <rdfs:label xml:lang="en">Comics character</rdfs:label>
    <rdfs:comment xml:lang="en">A character from a comics.</rdfs:comment>
  </owl:Class>
  <owl:Class rdf:about="http://www.ontotext.com/proton/protonext#Creek">
    <rdfs:subClassOf rdf:resource="http://www.ontotext.com/proton/protonext#WaterRegion"/>
    <rdfs:label xml:lang="en">Creek</rdfs:label>
    <rdfs:comment xml:lang="en">(ADL FT: Guts) Relatively small coastal waterways connecting larger bodies of water or other waterways. NIMA GNS designator CRKT, INLT.</rdfs:comment>
  </owl:Class>
  <owl:Class rdf:about="http://www.ontotext.com/proton/protonext#Lock">
    <rdfs:subClassOf rdf:resource="http://www.ontotext.com/proton/protonext#HydrographicStructure"/>
    <rdfs:subClassOf rdf:resource="http://www.ontotext.com/proton/protonext#TransportFacility"/>
    <rdfs:label xml:lang="en">Lock</rdfs:label>
    <rdfs:comment xml:lang="en">(ADL FT) Stretches of water in canals, streams, or docks, enclosed by gates at each end, and used in raising and lowering boats as they pass from one water level to another. NIMA GNS designator LOCK.</rdfs:comment>
  </owl:Class>
  <owl:Class rdf:about="http://www.ontotext.com/proton/protonext#AutomobileEngine">
    <rdfs:subClassOf rdf:resource="http://www.ontotext.com/proton/protonext#Machine"/>
    <rdfs:label xml:lang="en">Automobile Engine</rdfs:label>
    <rdfs:comment xml:lang="en">Engines of automobiles</rdfs:comment>
  </owl:Class>
  <owl:Class rdf:about="http://www.ontotext.com/proton/protonext#BasketballTeam">
    <rdfs:subClassOf>
      <owl:Class rdf:about="http://www.ontotext.com/proton/protonext#Team"/>
    </rdfs:subClassOf>
    <rdfs:label xml:lang="en">Basketball Team</rdfs:label>
    <rdfs:comment xml:lang="en">Any basketball team</rdfs:comment>
  </owl:Class>
  <owl:Class rdf:about="http://www.ontotext.com/proton/protonext#SkiArea">
    <rdfs:subClassOf rdf:resource="http://www.ontotext.com/proton/protonext#LandRegion"/>
    <rdfs:label xml:lang="en">Ski Area</rdfs:label>
    <rdfs:comment xml:lang="en">Any Ski Area, a mounatain area (usually) where there re ski resorts or one can ski.</rdfs:comment>
  </owl:Class>
  <owl:Class rdf:about="http://www.ontotext.com/proton/protonext#ShoppingMall">
    <rdfs:subClassOf rdf:resource="http://www.ontotext.com/proton/protonext#Building"/>
    <rdfs:label xml:lang="en">Shopping Mall</rdfs:label>
    <rdfs:comment xml:lang="en">Any Shopping Mall, a building which is a shopping mall</rdfs:comment>
  </owl:Class>
  <owl:Class rdf:about="http://www.ontotext.com/proton/protonext#Volcano">
    <rdfs:subClassOf>
      <owl:Class rdf:about="http://www.ontotext.com/proton/protonext#Mountain"/>
    </rdfs:subClassOf>
    <rdfs:label xml:lang="en">Volcano</rdfs:label>
    <rdfs:comment xml:lang="en">(ADL FT) Vents in the surface of the Earth through which magma and associated gases erupt; also, the forms or structures, usually conical, that are produced by the erupted material. NIMA GNS designator VLC.</rdfs:comment>
  </owl:Class>
  <owl:Class rdf:about="http://www.ontotext.com/proton/protonext#MilitaryCommand">
    <rdfs:subClassOf>
      <owl:Class rdf:about="http://www.ontotext.com/proton/protonext#MilitaryUnit"/>
    </rdfs:subClassOf>
    <rdfs:label xml:lang="en">Military Command</rdfs:label>
    <rdfs:comment xml:lang="en">Any military command, the organization which has a commanding role in a military organization.</rdfs:comment>
  </owl:Class>
  <owl:Class rdf:about="http://www.ontotext.com/proton/protonext#OilField">
    <rdfs:subClassOf rdf:resource="http://www.ontotext.com/proton/protonext#Facility"/>
    <rdfs:label xml:lang="en">Oil Field</rdfs:label>
    <rdfs:comment xml:lang="en">(ADL FT) Areas with reserves of recoverable petroleum or where petroleum has been removed from the Earth. ... We use this category for gas fields; for gasfields; for oilfields; for petroleum fields; and for storage fields (petroleum). NIMA GNS designator CMPO, OILF, OILQ, OILW, PMPO, GASF.</rdfs:comment>
  </owl:Class>
  <owl:Class rdf:about="http://www.ontotext.com/proton/protonext#Shoal">
    <rdfs:subClassOf rdf:resource="http://www.ontotext.com/proton/protonext#LandRegion"/>
    <rdfs:label xml:lang="en">Shoal</rdfs:label>
    <rdfs:comment xml:lang="en">Hazards to surface navigation composed of unconsolidated material. (U.SHSU; U.SHLU)</rdfs:comment>
  </owl:Class>
  <owl:Class rdf:about="http://www.ontotext.com/proton/protonext#Grassland">
    <rdfs:subClassOf rdf:resource="http://www.ontotext.com/proton/protonext#BiogeographicRegion"/>
    <rdfs:label xml:lang="en">Grassland</rdfs:label>
    <rdfs:comment xml:lang="en">An area dominated by grass vegetation</rdfs:comment>
  </owl:Class>
  <owl:Class rdf:about="http://www.ontotext.com/proton/protonext#Locomotive">
    <rdfs:subClassOf rdf:resource="http://www.ontotext.com/proton/protonext#Vehicle"/>
    <rdfs:label xml:lang="en">Locomotive</rdfs:label>
    <rdfs:comment xml:lang="en">Locomotive, a railway vehicle that provides the motive power for a train. (Wikipedia)</rdfs:comment>
  </owl:Class>
  <owl:Class rdf:about="http://www.ontotext.com/proton/protonext#Amphibian">
    <rdfs:subClassOf rdf:resource="http://www.ontotext.com/proton/protonext#Animal"/>
    <rdfs:label xml:lang="en">Amphibian</rdfs:label>
    <rdfs:comment xml:lang="en">Amphibian denotes animals such as frogs, salamanders, and caecilians, that are ectothermic (or cold-blooded) animals and metamorphose from a juvenile water-breathing form, either to an adult air-breathing form, or to a paedomorph that retains some juvenile characteristics. (Wikipedia)</rdfs:comment>
  </owl:Class>
  <owl:Class rdf:about="http://www.ontotext.com/proton/protonext#Arch">
    <rdfs:subClassOf rdf:resource="http://www.ontotext.com/proton/protonext#LandRegion"/>
    <rdfs:label xml:lang="en">Arch</rdfs:label>
    <rdfs:comment xml:lang="en">A natural or man-made structure in the form of an arch</rdfs:comment>
  </owl:Class>
  <owl:Class rdf:about="http://www.ontotext.com/proton/protonext#Brain">
    <rdfs:subClassOf rdf:resource="http://www.ontotext.com/proton/protonext#BodyPart"/>
    <rdfs:label xml:lang="en">Brain</rdfs:label>
    <rdfs:comment xml:lang="en">Any brain as a part of the body.</rdfs:comment>
  </owl:Class>
  <owl:Class rdf:about="http://www.ontotext.com/proton/protonext#Season">
    <rdfs:subClassOf rdf:resource="http://www.ontotext.com/proton/protonext#TemporalAbstraction"/>
    <rdfs:label xml:lang="en">Season</rdfs:label>
    <rdfs:comment xml:lang="en">One of the seasons of the year. In the places with a temperate climate there are four seasons: spring, summer, autumn, and winter.</rdfs:comment>
  </owl:Class>
  <owl:Class rdf:about="http://www.ontotext.com/proton/protonext#HistoricBuilding">
    <rdfs:subClassOf rdf:resource="http://www.ontotext.com/proton/protonext#Building"/>
    <rdfs:label xml:lang="en">Historic Building</rdfs:label>
    <rdfs:comment xml:lang="en">Any Historic Building, an old building with historic value.</rdfs:comment>
  </owl:Class>
  <owl:Class rdf:about="http://www.ontotext.com/proton/protonext#Beach">
    <rdfs:subClassOf rdf:resource="http://www.ontotext.com/proton/protonext#LandRegion"/>
    <rdfs:label xml:lang="en">Beach</rdfs:label>
    <rdfs:comment xml:lang="en">(ADL FT) Sloping shores along a body of water that is washed by waves or tides and is usually covered by sand or gravel. ... We use this category for sandy areas; and for strands. NIMA GNS designator BCH, BCHS.</rdfs:comment>
  </owl:Class>
  <owl:Class rdf:about="http://www.ontotext.com/proton/protonext#Fish">
    <rdfs:subClassOf rdf:resource="http://www.ontotext.com/proton/protonext#Animal"/>
    <rdfs:label xml:lang="en">Fish</rdfs:label>
    <rdfs:comment xml:lang="en">A fish is any gill-bearing aquatic vertebrate (or craniate) animal that lacks limbs with digits. (Wikipedia)</rdfs:comment>
  </owl:Class>
  <owl:Class rdf:about="http://www.ontotext.com/proton/protonext#GlobalRegion">
    <rdfs:subClassOf rdf:resource="http://www.ontotext.com/proton/protontop#Location"/>
    <rdfs:label xml:lang="en">Global Region</rdfs:label>
    <rdfs:comment xml:lang="en">Things like Southeastern Europe, Middle East, Oceania are global regions</rdfs:comment>
  </owl:Class>
  <owl:Class rdf:about="http://www.ontotext.com/proton/protonext#User">
    <rdfs:subClassOf rdf:resource="http://www.ontotext.com/proton/protontop#Agent"/>
    <rdfs:label>User</rdfs:label>
  </owl:Class>
  <owl:Class rdf:about="http://www.ontotext.com/proton/protonext#CricketLeague">
    <rdfs:subClassOf rdf:resource="http://www.ontotext.com/proton/protonext#SportsLeague"/>
    <rdfs:label xml:lang="en">Cricket League</rdfs:label>
    <rdfs:comment xml:lang="en">Any Cricket league</rdfs:comment>
  </owl:Class>
  <owl:Class rdf:about="http://www.ontotext.com/proton/protonext#Bird">
    <rdfs:subClassOf rdf:resource="http://www.ontotext.com/proton/protonext#Animal"/>
    <rdfs:label xml:lang="en">Bird</rdfs:label>
    <rdfs:comment xml:lang="en">Bird denotes feathered, winged, bipedal, endothermic (warm-blooded), egg-laying, vertebrate animals. (Wikipedia)</rdfs:comment>
  </owl:Class>
  <owl:Class rdf:about="http://www.ontotext.com/proton/protonext#Sportsman">
    <rdfs:subClassOf rdf:resource="http://www.ontotext.com/proton/protonext#Profession"/>
    <rdfs:label xml:lang="en">Sportsman</rdfs:label>
    <rdfs:comment xml:lang="en">A profession of a person involved in a sport.</rdfs:comment>
  </owl:Class>
  <owl:Class rdf:about="http://www.ontotext.com/proton/protonext#LaunchFacility">
    <rdfs:subClassOf rdf:resource="http://www.ontotext.com/proton/protonext#TransportFacility"/>
    <rdfs:label xml:lang="en">Launch Facility</rdfs:label>
    <rdfs:comment xml:lang="en">(ADL FT) Areas from which rockets/missiles may be housed and projected, usually equipped with associated buildings and facilities. [USGS Circ 1048] We use this category for missile sites. NIMA GNS designator - no equivalent.</rdfs:comment>
  </owl:Class>
  <owl:Class rdf:about="http://www.ontotext.com/proton/protonext#OutOfLawsTitle">
    <rdfs:subClassOf>
      <owl:Class rdf:about="http://www.ontotext.com/proton/protonext#SocialFunction"/>
    </rdfs:subClassOf>
    <rdfs:label xml:lang="en">Criminal</rdfs:label>
    <rdfs:comment xml:lang="en">Criminal, the social function of a person who has committed a crime and is out of the law.</rdfs:comment>
  </owl:Class>
  <owl:Class rdf:about="http://www.ontotext.com/proton/protonext#Division">
    <rdfs:subClassOf rdf:resource="http://www.ontotext.com/proton/protontop#Organization"/>
    <rdfs:label xml:lang="en">Division</rdfs:label>
    <rdfs:comment xml:lang="en">Branch, division, department, laboratory, etc. within an organisation. Usually, not a legal agent and not independent.</rdfs:comment>
  </owl:Class>
  <owl:Class rdf:about="http://www.ontotext.com/proton/protonext#Fjord">
    <rdfs:subClassOf rdf:resource="http://www.ontotext.com/proton/protonext#Bay"/>
    <rdfs:label xml:lang="en">Fjord</rdfs:label>
    <rdfs:comment xml:lang="en">(ADL FT) Long narrow glacially-eroded inlets of the sea, U-shaped and steep-walled, generally several hundred meters deep, between high rocky cliffs or slopes along a mountainous coast. ... We use this category for fiords; and for lochs. NIMA GNS designator FJD, FJDS.</rdfs:comment>
  </owl:Class>
  <owl:Class rdf:about="http://www.ontotext.com/proton/protonext#Reservoir">
    <rdfs:subClassOf rdf:resource="http://www.ontotext.com/proton/protonext#HydrographicStructure"/>
    <rdfs:subClassOf rdf:resource="http://www.ontotext.com/proton/protonext#Lake"/>
    <rdfs:label xml:lang="en">Reservoir</rdfs:label>
    <rdfs:comment xml:lang="en">(ADL FT) Artificially impounded bodies of water. We use this category for covered reservoirs; and for intermittent reservoirs. (incl. dams) NIMA GNS designator RSV, RSVI.</rdfs:comment>
  </owl:Class>
  <owl:Class rdf:about="http://www.ontotext.com/proton/protonext#ContinentalShelf">
    <rdfs:subClassOf rdf:resource="http://www.ontotext.com/proton/protonext#LandRegion"/>
    <rdfs:label xml:lang="en">Shelf</rdfs:label>
    <rdfs:comment xml:lang="en">A zone adjacent to a continent (or around an island) that extends from the low water line to a depth at which there is usually a marked increase of slope towards oceanic depths</rdfs:comment>
  </owl:Class>
  <owl:Class rdf:about="http://www.ontotext.com/proton/protonext#Park">
    <rdfs:subClassOf rdf:resource="http://www.ontotext.com/proton/protonext#Facility"/>
    <rdfs:label xml:lang="en">Park</rdfs:label>
    <rdfs:comment xml:lang="en">(ADL FT) Places or areas developed for public use or recreation. [USGS Circ 1048] We use this category for arboretums; for botanical gardens; for commemorative areas; for commons; for gardens; for marine parks; for national forests; for national parks; for national seashores; for park gates; for picnic areas; for playgrounds; for provincial parks; for public use areas; for recreation areas; for rest areas; for scenic areas; for state forests; for state parks; for urban parks; for village squares; for wilderness areas; for zoological gardens; and for zoos. Omitted sub-classes: Viewing locations. NIMA GNS designators PRK, PRKHQ, PRKGT</rdfs:comment>
  </owl:Class>
  <owl:Class rdf:about="http://www.ontotext.com/proton/protonext#AstronomicalObject">
    <rdfs:subClassOf rdf:resource="http://www.ontotext.com/proton/protontop#Location"/>
    <rdfs:label xml:lang="en">Astronomical Object</rdfs:label>
    <rdfs:comment xml:lang="en">Any object studied by astronomers, (usually quite large natural and inanimate) object that is located in the physical universe and is not on the surface of the Earth. Definition partly derived from OpenCyc 0.7</rdfs:comment>
  </owl:Class>
  <owl:Class rdf:about="http://www.ontotext.com/proton/protonext#Nerve">
    <rdfs:subClassOf rdf:resource="http://www.ontotext.com/proton/protonext#BodyPart"/>
    <rdfs:label xml:lang="en">Nerve</rdfs:label>
    <rdfs:comment xml:lang="en">Nerve is a general concept gathering all nerves of a body.</rdfs:comment>
  </owl:Class>
  <owl:Class rdf:about="http://www.ontotext.com/proton/protonext#Song">
    <rdfs:subClassOf>
      <owl:Class rdf:about="http://www.ontotext.com/proton/protonext#AudioRecording"/>
    </rdfs:subClassOf>
    <rdfs:label xml:lang="en">Song</rdfs:label>
    <rdfs:comment xml:lang="en">An recording of a song.</rdfs:comment>
  </owl:Class>
  <owl:Class rdf:about="http://www.ontotext.com/proton/protonext#WaterTank">
    <rdfs:subClassOf rdf:resource="http://www.ontotext.com/proton/protonext#HydrographicStructure"/>
    <rdfs:subClassOf rdf:resource="http://www.ontotext.com/proton/protonext#WaterRegion"/>
    <rdfs:label xml:lang="en">Water Tank</rdfs:label>
    <rdfs:comment xml:lang="en">A contained pool or tank of water at, below, or above ground level. NIMA GNS designator H.RSVT.</rdfs:comment>
  </owl:Class>
  <owl:Class rdf:about="http://www.ontotext.com/proton/protonext#Plain">
    <rdfs:subClassOf rdf:resource="http://www.ontotext.com/proton/protonext#LandRegion"/>
    <rdfs:label xml:lang="en">Plain</rdfs:label>
    <rdfs:comment xml:lang="en">(ADL FT) Regions of general uniform slope, comparatively level and of considerable extent. [USGS Circ 1048] We use this category for interfluves; and for llanos. NIMA GNS designators PLN, PLNU, PLNX, INTF.</rdfs:comment>
  </owl:Class>
  <owl:Class rdf:about="http://www.ontotext.com/proton/protonext#Broadcaster">
    <rdfs:subClassOf>
      <owl:Class rdf:about="http://www.ontotext.com/proton/protonext#MediaCompany"/>
    </rdfs:subClassOf>
    <rdfs:label xml:lang="en">Broadcaster</rdfs:label>
    <rdfs:comment xml:lang="en">A company that broadcasts audio or video content to a dispersed audience via any audio visual medium. Wikipedia</rdfs:comment>
  </owl:Class>
  <owl:Class rdf:about="http://www.ontotext.com/proton/protonext#Bight">
    <rdfs:subClassOf rdf:resource="http://www.ontotext.com/proton/protonext#LandRegion"/>
    <rdfs:label xml:lang="en">Bight</rdfs:label>
    <rdfs:comment xml:lang="en">An open body of water forming a slight recession in a coastline</rdfs:comment>
  </owl:Class>
  <owl:Class rdf:about="http://www.ontotext.com/proton/protonext#Government">
    <rdfs:subClassOf rdf:resource="http://www.ontotext.com/proton/protonext#GovernmentOrganization"/>
    <rdfs:label xml:lang="en">Government</rdfs:label>
    <rdfs:comment xml:lang="en">The government of a country.</rdfs:comment>
    <rdfs:comment xml:lang="en">The governmental cabinet</rdfs:comment>
  </owl:Class>
  <owl:Class rdf:about="http://www.ontotext.com/proton/protonext#Saddleback">
    <rdfs:subClassOf rdf:resource="http://www.ontotext.com/proton/protonext#LandRegion"/>
    <rdfs:label xml:lang="en">Saddle</rdfs:label>
    <rdfs:comment xml:lang="en">A low part, resembling in shape a saddle, in a ridge or between contiguous seamounts</rdfs:comment>
  </owl:Class>
  <owl:Class rdf:about="http://www.ontotext.com/proton/protonext#NaturalSatellite">
    <rdfs:subClassOf rdf:resource="http://www.ontotext.com/proton/protonext#Satellite"/>
    <rdfs:label xml:lang="en">Natural Satellite</rdfs:label>
    <rdfs:comment xml:lang="en">A satellite which is not a direct result of human activity</rdfs:comment>
  </owl:Class>
  <owl:Class rdf:about="http://www.ontotext.com/proton/protonext#Account">
    <rdfs:subClassOf rdf:resource="http://www.ontotext.com/proton/protontop#Object"/>
    <rdfs:label xml:lang="en">Account</rdfs:label>
    <rdfs:comment xml:lang="en">An explicit agreement between agents. Typically, service providers (e.g. banks or ISPs) provide accounts to their customers or users, which are considered account owners. The existence of the account depends on the provider, even though the user owns it in some metaphoric sense. Examples could be bank, ISP, e-Commerce, ICQ, email accounts. The accounts are usually aligned with a sort of contract.</rdfs:comment>
  </owl:Class>
  <owl:Class rdf:about="http://www.ontotext.com/proton/protonext#DayOfWeek">
    <rdfs:subClassOf rdf:resource="http://www.ontotext.com/proton/protonext#TemporalAbstraction"/>
    <rdfs:label xml:lang="en">Day of Week</rdfs:label>
    <rdfs:comment xml:lang="en">A specific day of the week. The week has seven days: Monday, Tuesday, Wednesday, Thursday, Friday, Saturday, and Sunday.</rdfs:comment>
  </owl:Class>
  <owl:Class rdf:about="http://www.ontotext.com/proton/protonext#Museum">
    <rdfs:subClassOf rdf:resource="http://www.ontotext.com/proton/protonext#Building"/>
    <rdfs:label xml:lang="en">Museum</rdfs:label>
    <rdfs:comment xml:lang="en">Any museum, an institution that houses and cares for a collection of artifacts and other objects of scientific, artistic, or historical importance and makes them available for public viewing through exhibits that may be permanent or temporary. (Wikipedia)</rdfs:comment>
  </owl:Class>
  <owl:Class rdf:about="http://www.ontotext.com/proton/protonext#Overfalls">
    <rdfs:subClassOf rdf:resource="http://www.ontotext.com/proton/protonext#WaterRegion"/>
    <rdfs:label xml:lang="en">Overfalls</rdfs:label>
    <rdfs:comment xml:lang="en">An area of breaking waves caused by the meeting of currents or by waves moving against the current. NIMA GNS designator H.OVF.</rdfs:comment>
  </owl:Class>
  <owl:Class rdf:about="http://www.ontotext.com/proton/protonext#MudFlat">
    <rdfs:subClassOf rdf:resource="http://www.ontotext.com/proton/protonext#LandRegion"/>
    <rdfs:label xml:lang="en">Mud Flat</rdfs:label>
    <rdfs:comment xml:lang="en">A relatively level area of mud either between high and low tide lines, or subject to flooding; a large flat area of mud or sand attached to the shore and alternately covered and uncovered by the tide; a tropical tidal mud flat characterized by mangrove vegetation</rdfs:comment>
  </owl:Class>
  <owl:Class rdf:about="http://www.ontotext.com/proton/protonext#LightHouse">
    <rdfs:subClassOf rdf:resource="http://www.ontotext.com/proton/protonext#ReferenceLocation"/>
    <rdfs:label xml:lang="en">Lighthouse</rdfs:label>
    <rdfs:comment xml:lang="en">A tower, building, or other type of structure designed to emit light from a system of lamps and lenses and used as an aid to navigation for maritime pilots at sea or on inland waterways</rdfs:comment>
  </owl:Class>
  <owl:Class rdf:about="http://www.ontotext.com/proton/protonext#Forest">
    <rdfs:subClassOf rdf:resource="http://www.ontotext.com/proton/protonext#BiogeographicRegion"/>
    <rdfs:label xml:lang="en">Forest</rdfs:label>
    <rdfs:comment xml:lang="en">(ADL FT) Dense growths of trees, plants, and underbrush covering a large area. [American Heritage Dic. of the English Language, 4th ed.] We use this category for forest reserves; and for national forests. Omitted ADL sub-classes: Petrified forests, Rain forests, Woods (the sub-classes collapsed here). NIMA GNS designator FRST, FRSTF, GDVC, GRVO, GRVP, GRVPN, TREE.</rdfs:comment>
  </owl:Class>
  <owl:Class rdf:about="http://www.ontotext.com/proton/protonext#Telecom">
    <rdfs:subClassOf rdf:resource="http://www.ontotext.com/proton/protonext#Company"/>
    <rdfs:label xml:lang="en">Telecom</rdfs:label>
    <rdfs:comment xml:lang="en">A telecommunications company</rdfs:comment>
  </owl:Class>
  <owl:Class rdf:about="http://www.ontotext.com/proton/protonext#Waterhole">
    <rdfs:subClassOf rdf:resource="http://www.ontotext.com/proton/protonext#WaterRegion"/>
    <rdfs:label xml:lang="en">Waterhole</rdfs:label>
    <rdfs:comment xml:lang="en">A natural hole, hollow, or small depression that contains water, used by man and animals, especially in arid areas. NIMA GNS designator H.WTRH.</rdfs:comment>
  </owl:Class>
  <owl:Class rdf:about="http://www.ontotext.com/proton/protonext#Message">
    <rdfs:subClassOf rdf:resource="http://www.ontotext.com/proton/protontop#Document"/>
    <rdfs:label xml:lang="en">Message</rdfs:label>
    <rdfs:comment xml:lang="en">A written message, including various postings in newspapers or public sources, job position adverts, etc.</rdfs:comment>
  </owl:Class>
  <owl:Class rdf:about="http://www.ontotext.com/proton/protonext#MusicalInstrument">
    <rdfs:subClassOf rdf:resource="http://www.ontotext.com/proton/protontop#Object"/>
    <rdfs:label xml:lang="en">Musical Instrument</rdfs:label>
    <rdfs:comment xml:lang="en">Musical Instrument, a device created or adapted for the purpose of making musical sounds. (Wikipedia)</rdfs:comment>
  </owl:Class>
  <owl:Class rdf:about="http://www.ontotext.com/proton/protonext#Book">
    <rdfs:subClassOf rdf:resource="http://www.ontotext.com/proton/protonext#PublishedMaterial"/>
    <rdfs:label xml:lang="en">Book</rdfs:label>
    <rdfs:comment xml:lang="en">A relatively large published document. It may or may not have chapters. There could be series of books considered as volumes of a single one.</rdfs:comment>
  </owl:Class>
  <owl:Class rdf:about="http://www.ontotext.com/proton/protonext#Bog">
    <rdfs:subClassOf rdf:resource="http://www.ontotext.com/proton/protonext#WaterRegion"/>
    <rdfs:label xml:lang="en">Bog</rdfs:label>
    <rdfs:comment xml:lang="en">http://www.eionet.europa.eu/gemet/concept?ns=1&amp;cp=12161. NIMA GNS designator H.BOG.</rdfs:comment>
  </owl:Class>
  <owl:Class rdf:about="http://www.ontotext.com/proton/protonext#Team">
    <rdfs:subClassOf rdf:resource="http://www.ontotext.com/proton/protontop#Organization"/>
    <rdfs:label xml:lang="en">Team</rdfs:label>
    <rdfs:comment xml:lang="en">A group of people gathered for some task, say a project. Teams are usually not formally established and not meant to perform as a single agent for purposes outside the scope of their task. Teams may "live" within organizations, spread between multiple organizations, or be independent form any organization.</rdfs:comment>
  </owl:Class>
  <owl:Class rdf:about="http://www.ontotext.com/proton/protonext#Human">
    <rdfs:subClassOf rdf:resource="http://www.ontotext.com/proton/protonext#Mammal"/>
    <rdfs:label xml:lang="en">Human</rdfs:label>
    <rdfs:comment xml:lang="en">Human is a mammal referred to Primate. Also of the sort of hommo sapiens. It has two subClasses: Man and Woman.</rdfs:comment>
  </owl:Class>
  <owl:Class rdf:about="http://www.ontotext.com/proton/protonext#OutOfLaws">
    <rdfs:subClassOf rdf:resource="http://www.ontotext.com/proton/protontop#SocialPosition"/>
    <rdfs:label xml:lang="en">OutOfLaws</rdfs:label>
    <rdfs:comment xml:lang="en">The situation of holding a position in a society as out of law.</rdfs:comment>
  </owl:Class>
  <owl:Class rdf:about="http://www.ontotext.com/proton/protonext#Nobelty">
    <rdfs:subClassOf rdf:resource="http://www.ontotext.com/proton/protontop#SocialPosition"/>
    <rdfs:label xml:lang="en">Nobelty</rdfs:label>
    <rdfs:comment xml:lang="en">The situation of holding a position in society as nobelty.</rdfs:comment>
  </owl:Class>
  <owl:Class rdf:about="http://www.ontotext.com/proton/protonext#DayOfMonth">
    <rdfs:subClassOf rdf:resource="http://www.ontotext.com/proton/protonext#TemporalAbstraction"/>
    <rdfs:label xml:lang="en">Day of Month</rdfs:label>
    <rdfs:comment xml:lang="en">A specific day of a given month. The days are numbered from 1 to 28, 29, 30, or 31 depending on the month and the year.</rdfs:comment>
  </owl:Class>
  <owl:Class rdf:about="http://www.ontotext.com/proton/protonext#Airport">
    <rdfs:subClassOf rdf:resource="http://www.ontotext.com/proton/protonext#TransportFacility"/>
    <rdfs:label xml:lang="en">Airport</rdfs:label>
    <rdfs:comment xml:lang="en">An airport, including heliports. NIMA GNS designators AIRP, AIRH.</rdfs:comment>
  </owl:Class>
  <owl:Class rdf:about="http://www.ontotext.com/proton/protonext#ResourceCollection">
    <rdfs:subClassOf rdf:resource="http://www.ontotext.com/proton/protontop#InformationResource"/>
    <rdfs:label xml:lang="en">Resource Collection</rdfs:label>
    <rdfs:comment xml:lang="en">A collection is an aggregation of information resources. The term collection means that the resource is described as a group; its parts may be separately described and navigated. (DCMI type Collection)</rdfs:comment>
  </owl:Class>
  <owl:Class rdf:about="http://www.ontotext.com/proton/protonext#RaceCourse">
    <rdfs:subClassOf rdf:resource="http://www.ontotext.com/proton/protonext#SportFacility"/>
    <rdfs:label xml:lang="en">Race Course</rdfs:label>
    <rdfs:comment xml:lang="en">A racecourse is a horse racing track.</rdfs:comment>
  </owl:Class>
  <owl:Class rdf:about="http://www.ontotext.com/proton/protonext#CommercialOrganization">
    <rdfs:subClassOf rdf:resource="http://www.ontotext.com/proton/protontop#Organization"/>
    <rdfs:label xml:lang="en">Commercial Organization</rdfs:label>
    <rdfs:comment xml:lang="en">Organization that buys or sells goods or services for a profit. It may also be a Business or it may merely be a sub-organization of a Business entity.</rdfs:comment>
  </owl:Class>
  <owl:Class rdf:about="http://www.ontotext.com/proton/protonext#Ship">
    <rdfs:subClassOf rdf:resource="http://www.ontotext.com/proton/protonext#Vehicle"/>
    <rdfs:label xml:lang="en">Ship</rdfs:label>
    <rdfs:comment xml:lang="en">A vehicle which moves on water.</rdfs:comment>
  </owl:Class>
  <owl:Class rdf:about="http://www.ontotext.com/proton/protonext#Sea">
    <rdfs:subClassOf rdf:resource="http://www.ontotext.com/proton/protonext#WaterRegion"/>
    <rdfs:label xml:lang="en">Sea</rdfs:label>
    <rdfs:comment xml:lang="en">(ADL FT) Large bodies of salt water. NIMA GNS designator SEA</rdfs:comment>
  </owl:Class>
  <owl:Class rdf:about="http://www.ontotext.com/proton/protonext#UserProfile">
    <rdfs:subClassOf rdf:resource="http://www.ontotext.com/proton/protonext#Profile"/>
    <rdfs:label>User Profile</rdfs:label>
  </owl:Class>
  <owl:Class rdf:about="http://www.ontotext.com/proton/protonext#PublishingCompany">
    <rdfs:subClassOf>
      <owl:Class rdf:about="http://www.ontotext.com/proton/protonext#MediaCompany"/>
    </rdfs:subClassOf>
    <rdfs:label xml:lang="en">Publishing Company</rdfs:label>
    <rdfs:comment xml:lang="en">An organization which main activity is mass publishing of information. Often, the publishers issue periodic and/or non-periodic documents on paper media. While on-line publishing is considered a typical activity for publishers, the streaming electronic media such as TV and Radio Stations are not.</rdfs:comment>
  </owl:Class>
  <owl:Class rdf:about="http://www.ontotext.com/proton/protonext#NewsAgency">
    <rdfs:subClassOf>
      <owl:Class rdf:about="http://www.ontotext.com/proton/protonext#MediaCompany"/>
    </rdfs:subClassOf>
    <rdfs:label xml:lang="en">News agency</rdfs:label>
    <rdfs:comment xml:lang="en">A news agency is an organization of journalists established to supply news reports to news organizations: newspapers, magazines, and radio and television broadcasters. Wikipedia</rdfs:comment>
  </owl:Class>
  <owl:Class rdf:about="http://www.ontotext.com/proton/protonext#OlympicGames">
    <rdfs:subClassOf rdf:resource="http://www.ontotext.com/proton/protonext#RecurringEvent"/>
    <rdfs:label xml:lang="en">Olympic Games</rdfs:label>
    <rdfs:comment xml:lang="en">The institution of Olympic Games held every 4 years</rdfs:comment>
  </owl:Class>
  <owl:Class rdf:about="http://www.ontotext.com/proton/protonext#Offer">
    <rdfs:subClassOf rdf:resource="http://www.ontotext.com/proton/protontop#Statement"/>
    <rdfs:label xml:lang="en">Offer</rdfs:label>
    <rdfs:comment xml:lang="en">Something offered (as a proposal or bid), WordNet 1.7.1. An offer is a statement made by the offerer to a specific agent or without recepient.</rdfs:comment>
  </owl:Class>
  <owl:Class rdf:about="http://www.ontotext.com/proton/protonext#Contract">
    <rdfs:subClassOf rdf:resource="http://www.ontotext.com/proton/protontop#Document"/>
    <rdfs:label xml:lang="en">Contract</rdfs:label>
    <rdfs:comment xml:lang="en">Any sort of contract or treaty, as well, as other documents signed or otherwise accepted by more than one agent.</rdfs:comment>
  </owl:Class>
  <owl:Class rdf:about="http://www.ontotext.com/proton/protonext#Skyscraper">
    <rdfs:subClassOf rdf:resource="http://www.ontotext.com/proton/protonext#Building"/>
    <rdfs:label xml:lang="en">Skyscraper</rdfs:label>
    <rdfs:comment xml:lang="en">Any Skyscraper, a highrise building, usually in downtown city areas.</rdfs:comment>
  </owl:Class>
  <owl:Class rdf:about="http://www.ontotext.com/proton/protonext#Death">
    <rdfs:subClassOf rdf:resource="http://www.ontotext.com/proton/protontop#Event"/>
    <rdfs:label xml:lang="en">Death</rdfs:label>
    <rdfs:comment xml:lang="en">The event to die.</rdfs:comment>
  </owl:Class>
  <owl:Class rdf:about="http://www.ontotext.com/proton/protonext#Arachnid">
    <rdfs:subClassOf rdf:resource="http://www.ontotext.com/proton/protonext#Animal"/>
    <rdfs:label xml:lang="en">Arachnid</rdfs:label>
    <rdfs:comment xml:lang="en">Arachnid denotes a class of joint-legged invertebrate animals in the subphylum Chelicerata. All arachnids have eight legs, although in some species the front pair may convert to a sensory function. (Wikipedia)</rdfs:comment>
  </owl:Class>
  <owl:Class rdf:about="http://www.ontotext.com/proton/protonext#Street">
    <rdfs:subClassOf rdf:resource="http://www.ontotext.com/proton/protonext#Roadway"/>
    <rdfs:label xml:lang="en">Street</rdfs:label>
    <rdfs:comment xml:lang="en">The general notion for a roadway within a city or village, often, surrounded by buildings. We put here boulevards, streets, avenues, etc. NIMA GNS designator - missing.</rdfs:comment>
  </owl:Class>
  <owl:Class rdf:about="http://www.ontotext.com/proton/protonext#ArtProfession">
    <rdfs:subClassOf rdf:resource="http://www.ontotext.com/proton/protonext#Profession"/>
    <rdfs:label xml:lang="en">Sportsman</rdfs:label>
    <rdfs:comment xml:lang="en">A profession in the area of art.</rdfs:comment>
  </owl:Class>
  <owl:Class rdf:about="http://www.ontotext.com/proton/protonext#InformationSpaceProfile">
    <rdfs:subClassOf rdf:resource="http://www.ontotext.com/proton/protonext#Profile"/>
    <rdfs:label>Information Space Profile</rdfs:label>
  </owl:Class>
  <owl:Class rdf:about="http://www.ontotext.com/proton/protonext#LegalCases">
    <rdfs:subClassOf rdf:resource="http://www.ontotext.com/proton/protontop#Event"/>
    <rdfs:label xml:lang="en">Legal Cases</rdfs:label>
    <rdfs:comment xml:lang="en">Denotes concrete legal cases, such as Dennis v. United States, Francis v. Resweber, United_States v. Virginia, etc.</rdfs:comment>
  </owl:Class>
  <owl:Class rdf:about="http://www.ontotext.com/proton/protonext#GolfLeague">
    <rdfs:subClassOf rdf:resource="http://www.ontotext.com/proton/protonext#SportsLeague"/>
    <rdfs:label xml:lang="en">Golf League</rdfs:label>
    <rdfs:comment xml:lang="en">Any Golf league</rdfs:comment>
  </owl:Class>
  <owl:Class rdf:about="http://www.ontotext.com/proton/protonext#AmericanFootballLeague">
    <rdfs:subClassOf rdf:resource="http://www.ontotext.com/proton/protonext#SportsLeague"/>
    <rdfs:label xml:lang="en">American Football League</rdfs:label>
    <rdfs:comment xml:lang="en">Any American football league</rdfs:comment>
  </owl:Class>
  <owl:Class rdf:about="http://www.ontotext.com/proton/protonext#Galaxy">
    <rdfs:subClassOf rdf:resource="http://www.ontotext.com/proton/protonext#AstronomicalObject"/>
    <rdfs:label xml:lang="en">Galaxy</rdfs:label>
    <rdfs:comment xml:lang="en">A galaxy is a massive, gravitationally bound system that consists of stars and stellar remnants, an interstellar medium of gas and dust, and an important but poorly understood component tentatively dubbed dark matter. Wikipedia</rdfs:comment>
  </owl:Class>
  <owl:Class rdf:about="http://www.ontotext.com/proton/protonext#Jungle">
    <rdfs:subClassOf rdf:resource="http://www.ontotext.com/proton/protonext#BiogeographicRegion"/>
    <rdfs:label xml:lang="en">Jungle</rdfs:label>
    <rdfs:comment xml:lang="en">(ADL FT) Tropical regions of wild, tangled, dense vegetation. NIMA GNS designator - no equivalent.</rdfs:comment>
  </owl:Class>
  <owl:Class rdf:about="http://www.ontotext.com/proton/protonext#Parish">
    <rdfs:subClassOf rdf:resource="http://www.ontotext.com/proton/protonext#PopulatedPlace"/>
    <rdfs:label xml:lang="en">Parish</rdfs:label>
    <rdfs:comment xml:lang="en">A district of religious land. NIMA GNS designator A.PRSH.</rdfs:comment>
  </owl:Class>
  <owl:Class rdf:about="http://www.ontotext.com/proton/protonext#RugbyClub">
    <rdfs:subClassOf rdf:resource="http://www.ontotext.com/proton/protonext#SportClub"/>
    <rdfs:label xml:lang="en">Rugby Club</rdfs:label>
    <rdfs:comment xml:lang="en">A rugby team</rdfs:comment>
    <rdfs:comment xml:lang="en">A sport club that organizes the playing of rugby.</rdfs:comment>
  </owl:Class>
  <owl:Class rdf:about="http://www.ontotext.com/proton/protonext#Cave">
    <rdfs:subClassOf rdf:resource="http://www.ontotext.com/proton/protonext#LandRegion"/>
    <rdfs:label xml:lang="en">Cave</rdfs:label>
    <rdfs:comment xml:lang="en">(ADL FT) Natural underground passageways or chambers, or hollowed out cavities in the side of a cliff. ... We use this category for cave entrances; for caverns; for grottoes; for natural tunnels; and for underground lakes. NIMA GNS designator CAVE.</rdfs:comment>
  </owl:Class>
  <owl:Class rdf:about="http://www.ontotext.com/proton/protonext#Wadi">
    <rdfs:subClassOf rdf:resource="http://www.ontotext.com/proton/protonext#LandRegion"/>
    <rdfs:label xml:lang="en">Wadi</rdfs:label>
    <rdfs:comment xml:lang="en">A valley or ravine, bounded by relatively steep banks. NIMA GNS designator H.WAD, H.WADB, H.WADJ, H.WADM, H.WADS, H.WADX.</rdfs:comment>
  </owl:Class>
  <owl:Class rdf:about="http://www.ontotext.com/proton/protonext#CalendarYear">
    <rdfs:subClassOf rdf:resource="http://www.ontotext.com/proton/protontop#TimeInterval"/>
    <rdfs:label xml:lang="en">Calendar Year</rdfs:label>
    <rdfs:comment xml:lang="en">A specific year, such as 2000, taken as a time interval</rdfs:comment>
  </owl:Class>
  <owl:Class rdf:about="http://www.ontotext.com/proton/protonext#WebPage">
    <rdfs:subClassOf rdf:resource="http://www.ontotext.com/proton/protonext#InternetAddress"/>
    <rdfs:label xml:lang="en">Web Page</rdfs:label>
    <rdfs:comment xml:lang="en">The internet address of a web page on the net.</rdfs:comment>
  </owl:Class>
  <owl:Class rdf:about="http://www.ontotext.com/proton/protonext#InformationSpace">
    <rdfs:subClassOf rdf:resource="http://www.ontotext.com/proton/protontop#Agent"/>
    <rdfs:label>Information Space</rdfs:label>
  </owl:Class>
  <owl:Class rdf:about="http://www.ontotext.com/proton/protonext#Date">
    <rdfs:subClassOf rdf:resource="http://www.ontotext.com/proton/protontop#TimeInterval"/>
    <rdfs:label xml:lang="en">Date</rdfs:label>
    <rdfs:comment xml:lang="en">A specific date, as 12th of April, 1956, as the time period (the 24 hours of the day)</rdfs:comment>
  </owl:Class>
  <owl:Class rdf:about="http://www.ontotext.com/proton/protonext#AudioRecording">
    <rdfs:subClassOf rdf:resource="http://www.ontotext.com/proton/protonext#MusicalComposition"/>
    <rdfs:label xml:lang="en">Audio Recording</rdfs:label>
    <rdfs:comment xml:lang="en">An recording of a piece of music.</rdfs:comment>
  </owl:Class>
  <owl:Class rdf:about="http://www.ontotext.com/proton/protonext#SpaceShuttle">
    <rdfs:subClassOf rdf:resource="http://www.ontotext.com/proton/protonext#Spacecraft"/>
    <rdfs:label xml:lang="en">Space Shuttle</rdfs:label>
    <rdfs:comment xml:lang="en">A Spaceshuttle is a reusable launch system and orbital spacecraft operated by the U.S. National Aeronautics and Space Administration (NASA) (Wikipedia).</rdfs:comment>
  </owl:Class>
  <owl:Class rdf:about="http://www.ontotext.com/proton/protonext#RiverCutoff">
    <rdfs:subClassOf rdf:resource="http://www.ontotext.com/proton/protonext#WaterRegion"/>
    <rdfs:label xml:lang="en">Cutoff</rdfs:label>
    <rdfs:comment xml:lang="en">A new channel cut by a river across the neck of an oxbow. NIMA GNS designator H.CUTF.</rdfs:comment>
  </owl:Class>
  <owl:Class rdf:about="http://www.ontotext.com/proton/protonext#Breakwater">
    <rdfs:subClassOf rdf:resource="http://www.ontotext.com/proton/protonext#Facility"/>
    <rdfs:label xml:lang="en">Breakwater</rdfs:label>
    <rdfs:comment xml:lang="en">A structure erected to break the force of waves at the entrance to a harbor or port</rdfs:comment>
  </owl:Class>
  <owl:Class rdf:about="http://www.ontotext.com/proton/protonext#SocialFunction">
    <rdfs:subClassOf>
      <owl:Class rdf:about="http://www.ontotext.com/proton/protonext#SocialAbstraction"/>
    </rdfs:subClassOf>
    <rdfs:label xml:lang="en">Social Function</rdfs:label>
    <rdfs:comment xml:lang="en">The name of a function a person has in the society like nobely, job title, celebrity, etc.</rdfs:comment>
  </owl:Class>
  <owl:Class rdf:about="http://www.ontotext.com/proton/protonext#BusinessAbstraction">
    <rdfs:subClassOf rdf:resource="http://www.ontotext.com/proton/protontop#Abstract"/>
    <rdfs:label xml:lang="en">Business Abstraction</rdfs:label>
    <rdfs:comment xml:lang="en">An abstraction related to business.</rdfs:comment>
  </owl:Class>
  <owl:Class rdf:about="http://www.ontotext.com/proton/protonext#Barracks">
    <rdfs:subClassOf rdf:resource="http://www.ontotext.com/proton/protonext#MilitaryAreas"/>
    <rdfs:label xml:lang="en">Barracks</rdfs:label>
    <rdfs:comment xml:lang="en">A building for lodging military personnel</rdfs:comment>
  </owl:Class>
  <owl:Class rdf:about="http://www.ontotext.com/proton/protonext#Mollusca">
    <rdfs:subClassOf rdf:resource="http://www.ontotext.com/proton/protonext#Animal"/>
    <rdfs:label xml:lang="en">Mollusca</rdfs:label>
    <rdfs:comment xml:lang="en">Mollusca is a large phylum of invertebrate animals. This is the largest marine phylum, comprising about 23% of all the named marine organisms. Numerous molluscs also live in freshwater and terrestrial habitats. Molluscs are highly diverse, not only in size and in anatomical structure, but also in behaviour and in habitat. (Wikipedia)</rdfs:comment>
  </owl:Class>
  <owl:Class rdf:about="http://www.ontotext.com/proton/protonext#Desert">
    <rdfs:subClassOf rdf:resource="http://www.ontotext.com/proton/protonext#BiogeographicRegion"/>
    <rdfs:label xml:lang="en">Desert</rdfs:label>
    <rdfs:comment xml:lang="en">(ADL FT) Regions rendered barren or partially barren by environmental extremes, especially by low rainfall. [USGS Circ 1048] We use this category for arid regions; for bajadas; for rock deserts; for sandy areas; for sandy deserts; and for stony deserts. NIMA GNS designators DSRT, ERG, HMDA, REG.</rdfs:comment>
  </owl:Class>
  <owl:Class rdf:about="http://www.ontotext.com/proton/protonext#Article">
    <rdfs:subClassOf rdf:resource="http://www.ontotext.com/proton/protonext#PublishedMaterial"/>
    <rdfs:label xml:lang="en">Article</rdfs:label>
    <rdfs:comment xml:lang="en">A relatively short document published as a part of Resource Collection.</rdfs:comment>
  </owl:Class>
  <owl:Class rdf:about="http://www.ontotext.com/proton/protonext#Mountain">
    <rdfs:subClassOf rdf:resource="http://www.ontotext.com/proton/protonext#LandRegion"/>
    <rdfs:label xml:lang="en">Mountain</rdfs:label>
    <rdfs:comment xml:lang="en">(ADL FT) Landmasses that project conspicuously above their surroundings. [USGS Circ 1048] We use this category for cerros; for cordilleras; for foothills; for hills; for knolls; for mounds; and for mounts. Omitted ADL sub-classes: Continental divides. NIMA GNS designator MT, MTS, MTSU, MTU, MND, KNLU, KNSU, CDAU, HLL, HLLS, HLLU, HLSU.</rdfs:comment>
  </owl:Class>
  <owl:Class rdf:about="http://www.ontotext.com/proton/protonext#Well">
    <rdfs:subClassOf rdf:resource="http://www.ontotext.com/proton/protonext#HydrographicStructure"/>
    <rdfs:subClassOf rdf:resource="http://www.ontotext.com/proton/protonext#WaterRegion"/>
    <rdfs:label xml:lang="en">Well</rdfs:label>
    <rdfs:comment xml:lang="en">A cylindrical hole, pit, or tunnel drilled or dug down to a depth from which water, oil, or gas can be pumped or brought to the surface. NIMA GNS designator H.WLL, H.WLLQ, H.WLLS.</rdfs:comment>
  </owl:Class>
  <owl:Class rdf:about="http://www.ontotext.com/proton/protonext#Acquirement">
    <rdfs:subClassOf rdf:resource="http://www.ontotext.com/proton/protontop#Event"/>
    <rdfs:label xml:lang="en">Acquirement</rdfs:label>
    <rdfs:comment xml:lang="en">The event of the acquiring of one organization by another.</rdfs:comment>
  </owl:Class>
  <owl:Class rdf:about="http://www.ontotext.com/proton/protonext#BiologicalSubstance">
    <rdfs:subClassOf rdf:resource="http://www.ontotext.com/proton/protontop#Object"/>
    <rdfs:label xml:lang="en">Biological Substance</rdfs:label>
    <rdfs:comment xml:lang="en">Any substance or element that has biological nature or origine.</rdfs:comment>
  </owl:Class>
  <owl:Class rdf:about="http://www.ontotext.com/proton/protonext#SocialAbstraction">
    <rdfs:subClassOf rdf:resource="http://www.ontotext.com/proton/protontop#Abstract"/>
    <rdfs:label xml:lang="en">Social Abstraction</rdfs:label>
    <rdfs:comment xml:lang="en">Any sort of general social phenomenon, such as particular sort of art or science</rdfs:comment>
  </owl:Class>
  <owl:Class rdf:about="http://www.ontotext.com/proton/protonext#Asteroid">
    <rdfs:subClassOf rdf:resource="http://www.ontotext.com/proton/protonext#AstronomicalObject"/>
    <rdfs:label xml:lang="en">Asteroid</rdfs:label>
    <rdfs:comment xml:lang="en">Asteroids are a class of small Solar System bodies in orbit around the Sun. Wikipedia</rdfs:comment>
  </owl:Class>
  <owl:Class rdf:about="http://www.ontotext.com/proton/protonext#OfficialPoliticalMeeting">
    <rdfs:subClassOf rdf:resource="http://www.ontotext.com/proton/protonext#Meeting"/>
    <rdfs:label xml:lang="en">Official Political Meeting</rdfs:label>
    <rdfs:comment xml:lang="en">A meeting whose main participants are political entities playing official roles within it.</rdfs:comment>
  </owl:Class>
  <owl:Class rdf:about="http://www.ontotext.com/proton/protonext#SingleAlbum">
    <rdfs:subClassOf rdf:resource="http://www.ontotext.com/proton/protonext#Album"/>
    <rdfs:subClassOf rdf:resource="http://www.ontotext.com/proton/protonext#SingleSongOrAlbum"/>
    <rdfs:label xml:lang="en">Single</rdfs:label>
    <rdfs:comment xml:lang="en">A representative for a musician album.</rdfs:comment>
    <rdfs:comment xml:lang="en">Any Single Album</rdfs:comment>
  </owl:Class>
  <owl:Class rdf:about="http://www.ontotext.com/proton/protonext#Canyon">
    <rdfs:subClassOf rdf:resource="http://www.ontotext.com/proton/protonext#Valley"/>
    <rdfs:label xml:lang="en">Canyon</rdfs:label>
    <rdfs:comment xml:lang="en">(ADL FT) Relatively narrow, deep depressions with steep sides, the bottom of which generally has a continuous slope ... We use this category for barrancas; for chasms; for flumes (natural); for gorges; for gulches; for quebradas; and for ravines. NIMA GNS designator CNSU, CNYN, CNYU, GRGE, RAVU, RVN.</rdfs:comment>
  </owl:Class>
  <owl:Class rdf:about="http://www.ontotext.com/proton/protonext#RugbyLeague">
    <rdfs:subClassOf rdf:resource="http://www.ontotext.com/proton/protonext#SportsLeague"/>
    <rdfs:label xml:lang="en">Rugby League</rdfs:label>
    <rdfs:comment xml:lang="en">Any Rugby League</rdfs:comment>
  </owl:Class>
  <owl:Class rdf:about="http://www.ontotext.com/proton/protonext#MilitaryUnit">
    <rdfs:subClassOf>
      <owl:Class rdf:about="http://www.ontotext.com/proton/protonext#MilitaryOrganization"/>
    </rdfs:subClassOf>
    <rdfs:label xml:lang="en">Military Unit</rdfs:label>
    <rdfs:comment xml:lang="en">Any military unit, a smaller military organization.</rdfs:comment>
  </owl:Class>
  <owl:Class rdf:about="http://www.ontotext.com/proton/protonext#Beverage">
    <rdfs:subClassOf rdf:resource="http://www.ontotext.com/proton/protonext#ChemicalCompound"/>
    <rdfs:label xml:lang="en">Beverage</rdfs:label>
    <rdfs:comment xml:lang="en">Any liquid suitable for drinking (WordNet, 1.7). The instances of this class are types of drinks, specific receipts. For instance: Diet Coke, Bacardi Spice.</rdfs:comment>
  </owl:Class>
  <owl:Class rdf:about="http://www.ontotext.com/proton/protonext#StreetName">
    <rdfs:subClassOf rdf:resource="http://www.ontotext.com/proton/protontop#ContactInformation"/>
    <rdfs:label xml:lang="en">Street Name</rdfs:label>
    <rdfs:comment xml:lang="en">Part of a postal address denoting the street name.</rdfs:comment>
  </owl:Class>
  <owl:Class rdf:about="http://www.ontotext.com/proton/protonext#Province">
    <rdfs:subClassOf>
      <owl:Class rdf:about="http://www.ontotext.com/proton/protonext#PoliticalRegion"/>
    </rdfs:subClassOf>
    <rdfs:subClassOf rdf:resource="http://www.ontotext.com/proton/protonext#PopulatedPlace"/>
    <rdfs:label xml:lang="en">Province</rdfs:label>
    <rdfs:comment xml:lang="en">(ADL FT: Countries, 1st Order Divisions) First-order divisions of a nation. [USGS Circ 1048] We use this category for cantons; for first-order administrative divisions; for provinces; for states; and for territories. NIMA GNS designator ADM1. Also corresponds to the FIPS 10-4 principal administrative division defined as "an administrative area directly subordinate to the pertinent governing authority " NIMA GNS designator ADM1.</rdfs:comment>
  </owl:Class>
  <owl:Class rdf:about="http://www.ontotext.com/proton/protonext#Bone">
    <rdfs:subClassOf rdf:resource="http://www.ontotext.com/proton/protonext#BodyPart"/>
    <rdfs:label xml:lang="en">Bone</rdfs:label>
    <rdfs:comment xml:lang="en">Any bone as a part of the body.</rdfs:comment>
  </owl:Class>
  <owl:Class rdf:about="http://www.ontotext.com/proton/protonext#Seamount">
    <rdfs:subClassOf rdf:resource="http://www.ontotext.com/proton/protonext#LandRegion"/>
    <rdfs:label xml:lang="en">Seamount</rdfs:label>
    <rdfs:comment xml:lang="en">An elevation rising generally more than 1,000 meters and of limited extent across the summit. (U.SMSU; U.SMU)</rdfs:comment>
  </owl:Class>
  <owl:Class rdf:about="http://www.ontotext.com/proton/protonext#Legislation">
    <rdfs:subClassOf rdf:resource="http://www.ontotext.com/proton/protontop#InformationResource"/>
    <rdfs:label xml:lang="en">Legislation</rdfs:label>
    <rdfs:comment xml:lang="en">Various sorts of legislative documents, including consitutions, laws, etc.</rdfs:comment>
  </owl:Class>
  <owl:Class rdf:about="http://www.ontotext.com/proton/protonext#ImageDocument">
    <rdfs:subClassOf rdf:resource="http://www.ontotext.com/proton/protontop#Document"/>
    <rdfs:label>Image</rdfs:label>
  </owl:Class>
  <owl:Class rdf:about="http://www.ontotext.com/proton/protonext#SpaceStation">
    <rdfs:subClassOf rdf:resource="http://www.ontotext.com/proton/protonext#Spacecraft"/>
    <rdfs:label xml:lang="en">Space Station</rdfs:label>
    <rdfs:comment xml:lang="en">Any Spacestation. A space station (also called an orbital station) is a manned satellite designed to remain in space. (Wikipedia)</rdfs:comment>
  </owl:Class>
  <owl:Class rdf:about="http://www.ontotext.com/proton/protonext#BaseballTeam">
    <rdfs:subClassOf rdf:resource="http://www.ontotext.com/proton/protonext#Team"/>
    <rdfs:label xml:lang="en">Baseball Team</rdfs:label>
    <rdfs:comment xml:lang="en">Any Baseball team</rdfs:comment>
  </owl:Class>
  <owl:Class rdf:about="http://www.ontotext.com/proton/protonext#PoliticalRegion">
    <rdfs:subClassOf rdf:resource="http://www.ontotext.com/proton/protontop#Location"/>
    <rdfs:label xml:lang="en">Political Region</rdfs:label>
    <rdfs:comment xml:lang="en">(ADL, Political Entity) We use this category for commonwealths; for dependent political entities; for freely associated states; for independent political entities; for oblasts; for political entities; and for semi-independent political entities. Sub-classes omitted: Countries, 4th order divisions. NIMA GNS class: A, Administrative Boundary Features.</rdfs:comment>
  </owl:Class>
  <owl:Class rdf:about="http://www.ontotext.com/proton/protonext#ClericTitle">
    <rdfs:subClassOf rdf:resource="http://www.ontotext.com/proton/protonext#SocialFunction"/>
    <rdfs:label xml:lang="en">Cleric</rdfs:label>
    <rdfs:comment xml:lang="en">The social function of a cleric, involving the church.</rdfs:comment>
  </owl:Class>
  <owl:Class rdf:about="http://www.ontotext.com/proton/protonext#AustralianFootballLeague">
    <rdfs:subClassOf rdf:resource="http://www.ontotext.com/proton/protonext#SportsLeague"/>
    <rdfs:label xml:lang="en">Australian Football League</rdfs:label>
    <rdfs:comment xml:lang="en">Any Australian football league</rdfs:comment>
  </owl:Class>
  <owl:Class rdf:about="http://www.ontotext.com/proton/protonext#Country">
    <rdfs:subClassOf rdf:resource="http://www.ontotext.com/proton/protonext#PoliticalRegion"/>
    <rdfs:subClassOf rdf:resource="http://www.ontotext.com/proton/protonext#PopulatedPlace"/>
    <rdfs:label xml:lang="en">Country</rdfs:label>
    <rdfs:comment xml:lang="en">(ADL FTT) Territory occupied by a large group of people organized under a single, usually independent government, and recognized internationally as a country. [Adapted from American Heritage Dic. of the English Language, 4th ed.] We use this category for nations; and for republics. NIMA GNS designators PCL, PCLD, PCLF, PCLI, PCLS. FIPS 10-4 is applicable, difining: Basic geopolitical entities assigned country codes include the following categories: (a) independent states; (b) dependent areas; (c) areas of quasi-independence, non-contiguous territories, possessions without populations, areas with special sovereignty associations, areas without sovereignty; (d) political regimes not recognized by the United States; and (e) outlying areas of the United States. The list of basic entities provides complete coverage of the land areas of the world without overlap or duplication.</rdfs:comment>
  </owl:Class>
  <owl:Class rdf:about="http://www.ontotext.com/proton/protonext#OlympicGamesOccurrence">
    <rdfs:subClassOf rdf:resource="http://www.ontotext.com/proton/protonext#SportEvent"/>
    <rdfs:label xml:lang="en">Olympic Games</rdfs:label>
    <rdfs:comment xml:lang="en">A specific issue of the games, like Athens 2004</rdfs:comment>
  </owl:Class>
  <owl:Class rdf:about="http://www.ontotext.com/proton/protonext#MotorcycleRacingLeague">
    <rdfs:subClassOf rdf:resource="http://www.ontotext.com/proton/protonext#SportsLeague"/>
    <rdfs:label xml:lang="en">Motorcycle Racing League</rdfs:label>
    <rdfs:comment xml:lang="en">Any Motorcycle Racing league</rdfs:comment>
  </owl:Class>
  <owl:Class rdf:about="http://www.ontotext.com/proton/protonext#LibraryOrganization">
    <rdfs:subClassOf rdf:resource="http://www.ontotext.com/proton/protonext#EducationalOrganization"/>
    <rdfs:label xml:lang="en">Library</rdfs:label>
    <rdfs:comment xml:lang="en">An education organization teaching pupils from first grade to tenth/eleventh/twelfth grade. It could be a primary school, or a secondary school.</rdfs:comment>
  </owl:Class>
  <owl:Class rdf:about="http://www.ontotext.com/proton/protonext#Channel">
    <rdfs:subClassOf rdf:resource="http://www.ontotext.com/proton/protonext#Canal"/>
    <rdfs:label xml:lang="en">Channel</rdfs:label>
    <rdfs:comment xml:lang="en">(ADL FT) (a) Relatively narrow seas or stretches of water between two close landmasses and connecting two larger bodies of water; (b) Deeper parts of a moving body of water (as bays, estuaries, or straits) through which the main current flows or which affords the best passage through an area otherwise too shallow to navigate. ... We use this category for chutes (hydrographic); for cutoffs (hydrographic); for inlets; for lake channels; for marine channels; for narrows (hydrographic); for navigation channels; for reaches (hydrographic); for sounds (bodies of water); and for straits. NIMA GNS designators CHN, CHNL, CHNM, CHNN, STRT.</rdfs:comment>
  </owl:Class>
  <owl:Class rdf:about="http://www.ontotext.com/proton/protonext#ReligiousLocation">
    <rdfs:subClassOf rdf:resource="http://www.ontotext.com/proton/protonext#Facility"/>
    <rdfs:label xml:lang="en">Religious Location</rdfs:label>
    <rdfs:comment xml:lang="en">Things like Monastery, Church</rdfs:comment>
  </owl:Class>
  <owl:Class rdf:about="http://www.ontotext.com/proton/protonext#MediaCompany">
    <rdfs:subClassOf rdf:resource="http://www.ontotext.com/proton/protonext#Company"/>
    <rdfs:label xml:lang="en">Media Company</rdfs:label>
  </owl:Class>
  <owl:Class rdf:about="http://www.ontotext.com/proton/protonext#SpaceMission">
    <rdfs:subClassOf rdf:resource="http://www.ontotext.com/proton/protontop#Event"/>
    <rdfs:label xml:lang="en">Space Mission</rdfs:label>
    <rdfs:comment xml:lang="en">Any Mission in space in which space shuttles or space crafts are involved.</rdfs:comment>
  </owl:Class>
  <owl:Class rdf:about="http://www.ontotext.com/proton/protonext#RecreationalFacility">
    <rdfs:subClassOf rdf:resource="http://www.ontotext.com/proton/protonext#Facility"/>
    <rdfs:label xml:lang="en">Recreational Facility</rdfs:label>
    <rdfs:comment xml:lang="en">(ADL FT) We use this category for access areas; for access sites; for boardwalks; for casinos; for clubs (recreational); for country clubs; for fairgrounds; for fishing areas; for fishing lodges; for fitness centers; for gun clubs; for hunt posts; for hunting lodges; for ice skating rinks; for playgrounds; for recreation sites; for resorts; for riding stables; for spas; for sportsman lodges; for stables; for yacht clubs; for youth centers; and for youth facilities. NIMA GNS designators - no direct equivalents.</rdfs:comment>
  </owl:Class>
  <owl:Class rdf:about="http://www.ontotext.com/proton/protonext#SportBuilding">
    <rdfs:subClassOf rdf:resource="http://www.ontotext.com/proton/protonext#Building"/>
    <rdfs:subClassOf rdf:resource="http://www.ontotext.com/proton/protonext#SportFacility"/>
    <rdfs:label xml:lang="en">Sport Building</rdfs:label>
    <rdfs:comment xml:lang="en">A building providing facilities for practice of sport(s).</rdfs:comment>
  </owl:Class>
  <owl:Class rdf:about="http://www.ontotext.com/proton/protonext#FloweringPlant">
    <rdfs:subClassOf rdf:resource="http://www.ontotext.com/proton/protonext#Plant"/>
    <rdfs:label xml:lang="en">Flowering plant</rdfs:label>
    <rdfs:comment xml:lang="en">Any flowering plant</rdfs:comment>
  </owl:Class>
  <owl:Class rdf:about="http://www.ontotext.com/proton/protonext#SiteOfSpecialScientificInterest">
    <rdfs:subClassOf rdf:resource="http://www.ontotext.com/proton/protonext#LocationOfSpecialInterest"/>
    <rdfs:label xml:lang="en">Site of Special Scientific Interest</rdfs:label>
    <rdfs:comment xml:lang="en">Any sites of special scientific interest, a place with scientific value, where some scientific activities or experiments are carried out, or which is observed for scientific reasons.</rdfs:comment>
  </owl:Class>
  <owl:Class rdf:about="http://www.ontotext.com/proton/protonext#Archipelago">
    <rdfs:subClassOf rdf:resource="http://www.ontotext.com/proton/protonext#LandRegion"/>
    <rdfs:label xml:lang="en">Archipelago</rdfs:label>
    <rdfs:comment xml:lang="en">(ADL FT) Seas or areas in a sea that contain numerous islands; also, the island groups themselves. NIMA GNS designator - no equivalent.</rdfs:comment>
  </owl:Class>
  <owl:Class rdf:about="http://www.ontotext.com/proton/protonext#WorldHeritageSite">
    <rdfs:subClassOf rdf:resource="http://www.ontotext.com/proton/protonext#LocationOfSpecialInterest"/>
    <rdfs:label xml:lang="en">World Heritage Site</rdfs:label>
    <rdfs:comment xml:lang="en">Any world heritage site, a old site with historic value of world magnitude to be preserved.</rdfs:comment>
  </owl:Class>
  <owl:Class rdf:about="http://www.ontotext.com/proton/protonext#Pipeline">
    <rdfs:subClassOf rdf:resource="http://www.ontotext.com/proton/protonext#TransportFacility"/>
    <rdfs:label xml:lang="en">Pipeline</rdfs:label>
    <rdfs:comment xml:lang="en">(ADL FT) Tubular conduits of substantial length, with pumps, valves, and control devices, for conveying fluids, gases, or finely divided solids. [USGS Circ 1048] We use this category for compressor stations; for gas pipelines; for oil pipeline junctions; for oil pipeline terminals; for oil pipelines; for oil pumping stations; for pump houses; for pumphouses; for pumping stations; and for water pumping stations. NIMA GNS designators OILP, OILJ, TRMO, PMPO, PMPW.</rdfs:comment>
  </owl:Class>
  <owl:Class rdf:about="http://www.ontotext.com/proton/protonext#NonAlcoholicBeverage">
    <rdfs:subClassOf rdf:resource="http://www.ontotext.com/proton/protonext#Beverage"/>
    <rdfs:label xml:lang="en">Non Alcoholic Beverage</rdfs:label>
    <rdfs:comment xml:lang="en">A type (specific receipe) for a beverage. For instance: Coca Cola, Schweppes, Apple Juice, etc.</rdfs:comment>
  </owl:Class>
  <owl:Class rdf:about="http://www.ontotext.com/proton/protonext#OperaPerformance">
    <rdfs:subClassOf rdf:resource="http://www.ontotext.com/proton/protonext#ArtPerformance"/>
    <rdfs:label xml:lang="en">Opera Performance</rdfs:label>
    <rdfs:comment xml:lang="en">An art performance following an opera music and script.</rdfs:comment>
  </owl:Class>
  <owl:Class rdf:about="http://www.ontotext.com/proton/protonext#MilitaryOrganization">
    <rdfs:subClassOf rdf:resource="http://www.ontotext.com/proton/protontop#Organization"/>
    <rdfs:label xml:lang="en">Military Organisation</rdfs:label>
    <rdfs:comment xml:lang="en">Any military organisation, the structuring of the armed forces of a state so as to offer military capability required by the national defence policy. (Wikipedia)</rdfs:comment>
  </owl:Class>
  <owl:ObjectProperty rdf:about="http://www.ontotext.com/proton/protonext#hasFather">
    <rdfs:subPropertyOf rdf:resource="http://www.ontotext.com/proton/protontop#hasParent"/>
    <rdfs:range rdf:resource="http://www.ontotext.com/proton/protonext#Man"/>
    <rdfs:label xml:lang="en">has Father</rdfs:label>
    <rdfs:comment xml:lang="en">Relates a person and his/her father.</rdfs:comment>
  </owl:ObjectProperty>
  <owl:ObjectProperty rdf:about="http://www.ontotext.com/proton/protonext#hasMobilePhone">
    <rdfs:subPropertyOf>
      <owl:ObjectProperty rdf:about="http://www.ontotext.com/proton/protonext#hasPhone"/>
    </rdfs:subPropertyOf>
    <rdfs:label xml:lang="en">has Mobile Phone</rdfs:label>
    <rdfs:comment xml:lang="en">Relates an object (usually a person) to its mobile phone number.</rdfs:comment>
  </owl:ObjectProperty>
  <owl:ObjectProperty rdf:about="http://www.ontotext.com/proton/protonext#socialPositionCelebrity">
    <owl:inverseOf>
      <owl:ObjectProperty rdf:about="http://www.ontotext.com/proton/protonext#hasSocialPositionCelebrity"/>
    </owl:inverseOf>
    <rdfs:subPropertyOf rdf:resource="http://www.ontotext.com/proton/protontop#socialPositionHolder"/>
    <rdfs:range rdf:resource="http://www.ontotext.com/proton/protontop#Person"/>
    <rdfs:label xml:lang="en">Social Position Holder Celebrity</rdfs:label>
    <rdfs:domain rdf:resource="http://www.ontotext.com/proton/protonext#Celebrity"/>
    <rdfs:comment xml:lang="en">The relation between a social position of Celebrity and the person who has it.</rdfs:comment>
  </owl:ObjectProperty>
  <owl:ObjectProperty rdf:about="http://www.ontotext.com/proton/protonext#organizationPosition">
    <owl:inverseOf rdf:resource="http://www.ontotext.com/proton/protontop#withinOrganization"/>
    <rdfs:range rdf:resource="http://www.ontotext.com/proton/protontop#JobPosition"/>
    <rdfs:label xml:lang="en">within Organization</rdfs:label>
    <rdfs:domain rdf:resource="http://www.ontotext.com/proton/protontop#Organization"/>
    <rdfs:comment xml:lang="en">The relation between an organization and a concrete job position in it.</rdfs:comment>
  </owl:ObjectProperty>
  <owl:ObjectProperty rdf:about="http://www.ontotext.com/proton/protonext#hasGovernment">
    <rdfs:range rdf:resource="http://www.ontotext.com/proton/protonext#GovernmentOrganization"/>
    <rdfs:label xml:lang="en">has Government</rdfs:label>
    <rdfs:domain rdf:resource="http://www.ontotext.com/proton/protonext#Country"/>
    <rdfs:comment xml:lang="en">A relation between a country and its government</rdfs:comment>
  </owl:ObjectProperty>
  <owl:ObjectProperty rdf:about="http://www.ontotext.com/proton/protonext#hasSocialPositionNobelty">
    <owl:inverseOf>
      <owl:ObjectProperty rdf:about="http://www.ontotext.com/proton/protonext#socialPositionNobelty"/>
    </owl:inverseOf>
    <rdfs:subPropertyOf rdf:resource="http://www.ontotext.com/proton/protontop#hasSocialPosition"/>
    <rdfs:range rdf:resource="http://www.ontotext.com/proton/protonext#Nobelty"/>
    <rdfs:label xml:lang="en">has Social Position Nobelty</rdfs:label>
    <rdfs:domain rdf:resource="http://www.ontotext.com/proton/protontop#Person"/>
    <rdfs:comment xml:lang="en">The relation between a person and the social position of Nobelty he has.</rdfs:comment>
  </owl:ObjectProperty>
  <owl:ObjectProperty rdf:about="http://www.ontotext.com/proton/protonext#hasSection">
    <rdfs:range rdf:resource="http://www.ontotext.com/proton/protonext#Section"/>
    <rdfs:label>has Section</rdfs:label>
    <rdfs:domain rdf:resource="http://www.ontotext.com/proton/protontop#Document"/>
    <rdfs:comment>Natural relation between documents and sections. Imported from the iSIM ontology.</rdfs:comment>
  </owl:ObjectProperty>
  <owl:ObjectProperty rdf:about="http://www.ontotext.com/proton/protonext#pointAwardedTo">
    <rdfs:range rdf:resource="http://www.ontotext.com/proton/protonext#SportClub"/>
    <rdfs:label xml:lang="en">Awarded Sport Club</rdfs:label>
    <rdfs:domain rdf:resource="http://www.ontotext.com/proton/protonext#SportGamePoint"/>
    <rdfs:comment xml:lang="en">The relation between the scored point in a sport game and the sport club who won it.</rdfs:comment>
  </owl:ObjectProperty>
  <owl:ObjectProperty rdf:about="http://www.ontotext.com/proton/protonext#hasPhone">
    <rdfs:subPropertyOf rdf:resource="http://www.ontotext.com/proton/protontop#hasContactInfo"/>
    <rdfs:range rdf:resource="http://www.ontotext.com/proton/protonext#PhoneNumber"/>
    <rdfs:label xml:lang="en">has Phone</rdfs:label>
    <rdfs:comment xml:lang="en">Relates an object (usually a person or an organization) to its telephone number.</rdfs:comment>
  </owl:ObjectProperty>
  <owl:ObjectProperty rdf:about="http://www.ontotext.com/proton/protonext#hasSocialPositionOutOfLaws">
    <owl:inverseOf>
      <owl:ObjectProperty rdf:about="http://www.ontotext.com/proton/protonext#socialPositionOutOfLaws"/>
    </owl:inverseOf>
    <rdfs:subPropertyOf rdf:resource="http://www.ontotext.com/proton/protontop#hasSocialPosition"/>
    <rdfs:range rdf:resource="http://www.ontotext.com/proton/protonext#OutOfLaws"/>
    <rdfs:label xml:lang="en">has Social Position OutOfLaws</rdfs:label>
    <rdfs:domain rdf:resource="http://www.ontotext.com/proton/protontop#Person"/>
    <rdfs:comment xml:lang="en">The relation between a person and the social position of OutOfLaws he has.</rdfs:comment>
  </owl:ObjectProperty>
  <owl:ObjectProperty rdf:about="http://www.ontotext.com/proton/protonext#hasAddress">
    <rdfs:subPropertyOf rdf:resource="http://www.ontotext.com/proton/protontop#hasContactInfo"/>
    <rdfs:range rdf:resource="http://www.ontotext.com/proton/protonext#Address"/>
    <rdfs:label xml:lang="en">has Address</rdfs:label>
    <rdfs:comment xml:lang="en">Relates address to an agent. Will be used for URL, email and other addresses.</rdfs:comment>
  </owl:ObjectProperty>
  <owl:ObjectProperty rdf:about="http://www.ontotext.com/proton/protonext#compliantWithSchema">
    <rdfs:range rdf:resource="http://www.ontotext.com/proton/protonext#DataSchema"/>
    <rdfs:label xml:lang="en">Compliant with Schema</rdfs:label>
    <rdfs:domain rdf:resource="http://www.ontotext.com/proton/protontop#InformationResource"/>
    <rdfs:comment xml:lang="en">It links a dataset with a schema it complies to.</rdfs:comment>
  </owl:ObjectProperty>
  <owl:ObjectProperty rdf:about="http://www.ontotext.com/proton/protonext#hasDaughter">
    <rdfs:subPropertyOf rdf:resource="http://www.ontotext.com/proton/protontop#hasChild"/>
    <rdfs:range rdf:resource="http://www.ontotext.com/proton/protonext#Woman"/>
    <rdfs:label xml:lang="en">has Daughter</rdfs:label>
    <rdfs:comment xml:lang="en">Relates a person and his/her daughter.</rdfs:comment>
  </owl:ObjectProperty>
  <owl:ObjectProperty rdf:about="http://www.ontotext.com/proton/protonext#combatantFrom">
    <rdfs:subPropertyOf rdf:resource="http://www.ontotext.com/proton/protontop#partOf"/>
    <rdfs:range rdf:resource="http://www.ontotext.com/proton/protontop#Organization"/>
    <rdfs:label xml:lang="en">Combatant from</rdfs:label>
    <rdfs:domain rdf:resource="http://www.ontotext.com/proton/protonext#MilitaryUnit"/>
    <rdfs:comment xml:lang="en">the relation between a military unit and the organization it represents in a military conflict.</rdfs:comment>
  </owl:ObjectProperty>
  <owl:ObjectProperty rdf:about="http://www.ontotext.com/proton/protonext#publishedWithin">
    <rdfs:range rdf:resource="http://www.ontotext.com/proton/protonext#ResourceCollection"/>
    <rdfs:label xml:lang="en">Published within</rdfs:label>
    <rdfs:domain rdf:resource="http://www.ontotext.com/proton/protonext#Article"/>
    <rdfs:comment xml:lang="en">A relation between an article and the colelction within which the article is published.</rdfs:comment>
  </owl:ObjectProperty>
  <owl:ObjectProperty rdf:about="http://www.ontotext.com/proton/protonext#hasSister">
    <rdfs:subPropertyOf rdf:resource="http://www.ontotext.com/proton/protontop#hasSibling"/>
    <rdfs:range rdf:resource="http://www.ontotext.com/proton/protonext#Woman"/>
    <rdfs:label xml:lang="en">has Sister</rdfs:label>
    <rdfs:comment xml:lang="en">Relates a person to his/her sister.</rdfs:comment>
  </owl:ObjectProperty>
  <owl:ObjectProperty rdf:about="http://www.ontotext.com/proton/protonext#hasSocialPositionCelebrity">
    <owl:inverseOf rdf:resource="http://www.ontotext.com/proton/protonext#socialPositionCelebrity"/>
    <rdfs:subPropertyOf rdf:resource="http://www.ontotext.com/proton/protontop#hasSocialPosition"/>
    <rdfs:range rdf:resource="http://www.ontotext.com/proton/protonext#Celebrity"/>
    <rdfs:label xml:lang="en">has Social Position Celebrity</rdfs:label>
    <rdfs:domain rdf:resource="http://www.ontotext.com/proton/protontop#Person"/>
    <rdfs:comment xml:lang="en">The relation between a person and the social position of Celebrity he has.</rdfs:comment>
  </owl:ObjectProperty>
  <owl:ObjectProperty rdf:about="http://www.ontotext.com/proton/protonext#locationMap">
    <rdfs:range rdf:resource="http://www.ontotext.com/proton/protonext#ElectronicMap"/>
    <rdfs:label xml:lang="en">Location Map</rdfs:label>
    <rdfs:domain rdf:resource="http://www.ontotext.com/proton/protontop#Location"/>
    <rdfs:comment xml:lang="en">The relation between a geographic region and a map depicting its location</rdfs:comment>
  </owl:ObjectProperty>
  <owl:ObjectProperty rdf:about="http://www.ontotext.com/proton/protonext#hasCapital">
    <rdfs:range rdf:resource="http://www.ontotext.com/proton/protonext#Capital"/>
    <rdfs:label xml:lang="en">has Capital</rdfs:label>
    <rdfs:domain rdf:resource="http://www.ontotext.com/proton/protonext#PoliticalRegion"/>
  </owl:ObjectProperty>
  <owl:ObjectProperty rdf:about="http://www.ontotext.com/proton/protonext#hasHusband">
    <rdfs:subPropertyOf rdf:resource="http://www.ontotext.com/proton/protontop#hasSpouse"/>
    <rdfs:range rdf:resource="http://www.ontotext.com/proton/protonext#Man"/>
    <rdfs:label xml:lang="en">has Husband</rdfs:label>
    <rdfs:domain rdf:resource="http://www.ontotext.com/proton/protonext#Woman"/>
    <rdfs:comment xml:lang="en">Relates a woman to her spouse.</rdfs:comment>
  </owl:ObjectProperty>
  <owl:ObjectProperty rdf:about="http://www.ontotext.com/proton/protonext#hasSocialFunctionTitle">
    <rdfs:range rdf:resource="http://www.ontotext.com/proton/protonext#SocialFunction"/>
    <rdfs:label xml:lang="en">has Title</rdfs:label>
    <rdfs:domain rdf:resource="http://www.ontotext.com/proton/protontop#SocialPosition"/>
    <rdfs:comment xml:lang="en">Generic property relating a Social Position to its name defined as an instance of a sub-class of pext:SocialFunction</rdfs:comment>
  </owl:ObjectProperty>
  <owl:ObjectProperty rdf:about="http://www.ontotext.com/proton/protonext#hasShareholder">
    <rdfs:subPropertyOf rdf:resource="http://www.ontotext.com/proton/protontop#hasMember"/>
    <rdfs:label xml:lang="en">has shareholder</rdfs:label>
    <rdfs:domain rdf:resource="http://www.ontotext.com/proton/protonext#CommercialOrganization"/>
    <rdfs:comment xml:lang="en">A relation between a commercial organization and a person that owns shares of the organization.</rdfs:comment>
  </owl:ObjectProperty>
  <owl:ObjectProperty rdf:about="http://www.ontotext.com/proton/protonext#tradedOn">
    <rdfs:label xml:lang="en">Traded on</rdfs:label>
    <rdfs:domain rdf:resource="http://www.ontotext.com/proton/protonext#PublicCompany"/>
    <rdfs:comment xml:lang="en">Relates the Public Company to the Stock Exchange where it is traded</rdfs:comment>
  </owl:ObjectProperty>
  <owl:ObjectProperty rdf:about="http://www.ontotext.com/proton/protonext#hasStationaryPhone">
    <rdfs:subPropertyOf rdf:resource="http://www.ontotext.com/proton/protonext#hasPhone"/>
    <rdfs:label xml:lang="en">has Stationary Phone</rdfs:label>
    <rdfs:comment xml:lang="en">Relates an object (usually a person) to its stationary phone number.</rdfs:comment>
  </owl:ObjectProperty>
  <owl:ObjectProperty rdf:about="http://www.ontotext.com/proton/protonext#isCurrentlyInterestedIn">
    <rdfs:range rdf:resource="http://www.ontotext.com/proton/protontop#Topic"/>
    <rdfs:label>isCurrentlyInterestedIn</rdfs:label>
    <rdfs:domain rdf:resource="http://www.ontotext.com/proton/protonext#UserProfile"/>
  </owl:ObjectProperty>
  <owl:ObjectProperty rdf:about="http://www.ontotext.com/proton/protonext#activeInSector">
    <ptop:transitiveOver>
      <owl:ObjectProperty rdf:about="http://www.ontotext.com/proton/protonext#subSectorOf"/>
    </ptop:transitiveOver>
    <rdfs:range rdf:resource="http://www.ontotext.com/proton/protonext#IndustrySector"/>
    <rdfs:label xml:lang="en">Active in Sector</rdfs:label>
    <rdfs:domain rdf:resource="http://www.ontotext.com/proton/protonext#CommercialOrganization"/>
    <rdfs:comment xml:lang="en">Denotes that the organization is active within the industry sector</rdfs:comment>
  </owl:ObjectProperty>
  <owl:ObjectProperty rdf:about="http://www.ontotext.com/proton/protonext#carAssemblyIn">
    <rdfs:range rdf:resource="http://www.ontotext.com/proton/protonext#Country"/>
    <rdfs:label xml:lang="en">Car Assembly in</rdfs:label>
    <rdfs:domain rdf:resource="http://www.ontotext.com/proton/protonext#CarModel"/>
    <rdfs:comment xml:lang="en">The relation between a car model and the country it is assembled in.</rdfs:comment>
  </owl:ObjectProperty>
  <owl:ObjectProperty rdf:about="http://www.ontotext.com/proton/protonext#architect">
    <rdfs:range>
      <owl:Restriction>
        <owl:onProperty>
          <owl:ObjectProperty rdf:about="http://www.ontotext.com/proton/protonext#hasProfession"/>
        </owl:onProperty>
        <owl:hasValue>
          <pext:Profession rdf:about="http://www.ontotext.com/proton/protonext#Architect">
            <rdfs:label xml:lang="en">Architect</rdfs:label>
            <rdfs:comment xml:lang="en">Any architect, a profession of planning, design and oversight of the construction of buildings. (Wikipedia)</rdfs:comment>
          </pext:Profession>
        </owl:hasValue>
      </owl:Restriction>
    </rdfs:range>
    <rdfs:label xml:lang="en">Architect</rdfs:label>
    <rdfs:domain rdf:resource="http://www.ontotext.com/proton/protonext#Facility"/>
    <rdfs:comment xml:lang="en">The relation between a facility and its architect.</rdfs:comment>
  </owl:ObjectProperty>
  <owl:ObjectProperty rdf:about="http://www.ontotext.com/proton/protonext#causeOfDeath">
    <rdfs:range rdf:resource="http://www.ontotext.com/proton/protontop#Event"/>
    <rdfs:label xml:lang="en">Cause of a Death</rdfs:label>
    <rdfs:domain rdf:resource="http://www.ontotext.com/proton/protonext#Death"/>
    <rdfs:comment xml:lang="en">Any cause of death.</rdfs:comment>
  </owl:ObjectProperty>
  <owl:ObjectProperty rdf:about="http://www.ontotext.com/proton/protonext#hasTitle">
    <rdfs:subPropertyOf rdf:resource="http://www.ontotext.com/proton/protonext#hasSocialFunctionTitle"/>
    <rdfs:range rdf:resource="http://www.ontotext.com/proton/protonext#JobTitle"/>
    <rdfs:label xml:lang="en">has Title</rdfs:label>
    <rdfs:domain rdf:resource="http://www.ontotext.com/proton/protontop#JobPosition"/>
    <rdfs:comment xml:lang="en">Relates a job position to its title.</rdfs:comment>
  </owl:ObjectProperty>
  <owl:ObjectProperty rdf:about="http://www.ontotext.com/proton/protonext#positionContactInformation">
    <rdfs:subPropertyOf rdf:resource="http://www.ontotext.com/proton/protontop#hasParticipatingEntity"/>
    <rdfs:range rdf:resource="http://www.ontotext.com/proton/protontop#ContactInformation"/>
    <rdfs:label xml:lang="en">Contact Information for a Position within Organization</rdfs:label>
    <rdfs:domain rdf:resource="http://www.ontotext.com/proton/protonext#PositionOrganization"/>
    <rdfs:comment xml:lang="en">The relation between a position and the contact information for it. This contact information can be the postal address of the office for the position or an virtual address in the Internet.</rdfs:comment>
  </owl:ObjectProperty>
  <owl:ObjectProperty rdf:about="http://www.ontotext.com/proton/protonext#hasSon">
    <rdfs:subPropertyOf rdf:resource="http://www.ontotext.com/proton/protontop#hasChild"/>
    <rdfs:range rdf:resource="http://www.ontotext.com/proton/protonext#Man"/>
    <rdfs:label xml:lang="en">has Son</rdfs:label>
    <rdfs:comment xml:lang="en">Relates a person to his/her son.</rdfs:comment>
  </owl:ObjectProperty>
  <owl:ObjectProperty rdf:about="http://www.ontotext.com/proton/protonext#socialPositionNobelty">
    <owl:inverseOf rdf:resource="http://www.ontotext.com/proton/protonext#hasSocialPositionNobelty"/>
    <rdfs:subPropertyOf rdf:resource="http://www.ontotext.com/proton/protontop#socialPositionHolder"/>
    <rdfs:range rdf:resource="http://www.ontotext.com/proton/protontop#Person"/>
    <rdfs:label xml:lang="en">Social Position Holder Nobelty</rdfs:label>
    <rdfs:domain rdf:resource="http://www.ontotext.com/proton/protonext#Nobelty"/>
    <rdfs:comment xml:lang="en">The relation between a social position of Nobelty and the person who has it.</rdfs:comment>
  </owl:ObjectProperty>
  <owl:ObjectProperty rdf:about="http://www.ontotext.com/proton/protonext#hasMother">
    <rdfs:subPropertyOf rdf:resource="http://www.ontotext.com/proton/protontop#hasParent"/>
    <rdfs:range rdf:resource="http://www.ontotext.com/proton/protonext#Woman"/>
    <rdfs:label xml:lang="en">has Mother</rdfs:label>
    <rdfs:comment xml:lang="en">Relates a person to his/her mother.</rdfs:comment>
  </owl:ObjectProperty>
  <owl:ObjectProperty rdf:about="http://www.ontotext.com/proton/protonext#isWrittenAbout">
    <rdfs:range rdf:resource="http://www.ontotext.com/proton/protonext#Article"/>
    <rdfs:label xml:lang="en">RDF document containing the descriptions of locations that share a common border</rdfs:label>
    <rdfs:domain rdf:resource="http://www.ontotext.com/proton/protontop#Location"/>
    <rdfs:comment xml:lang="en">The relation between an RDF document containing the descriptions of locations that share a common border</rdfs:comment>
  </owl:ObjectProperty>
  <owl:ObjectProperty rdf:about="http://www.ontotext.com/proton/protonext#hasClericTitle">
    <rdfs:subPropertyOf rdf:resource="http://www.ontotext.com/proton/protonext#hasSocialFunctionTitle"/>
    <rdfs:range rdf:resource="http://www.ontotext.com/proton/protonext#ClericTitle"/>
    <rdfs:label xml:lang="en">has Cleric Title</rdfs:label>
    <rdfs:domain rdf:resource="http://www.ontotext.com/proton/protonext#Cleric"/>
    <rdfs:comment xml:lang="en">The relation between a Cleric and its cleric title, like Bishop, Pole, etc.</rdfs:comment>
  </owl:ObjectProperty>
  <owl:ObjectProperty rdf:about="http://www.ontotext.com/proton/protonext#ownershipOf">
    <rdfs:range rdf:resource="http://www.ontotext.com/proton/protonext#Possession"/>
    <rdfs:label xml:lang="en">Ownership</rdfs:label>
    <rdfs:domain rdf:resource="http://www.ontotext.com/proton/protontop#Object"/>
    <rdfs:comment xml:lang="en">The relationship between an object being a property/possessions of somebody.</rdfs:comment>
  </owl:ObjectProperty>
  <owl:ObjectProperty rdf:about="http://www.ontotext.com/proton/protonext#isAuthorOf">
    <owl:inverseOf>
      <owl:ObjectProperty rdf:about="http://www.ontotext.com/proton/protonext#authorOf"/>
    </owl:inverseOf>
    <rdfs:range rdf:resource="http://www.ontotext.com/proton/protontop#Object"/>
    <rdfs:label xml:lang="en">Author</rdfs:label>
    <rdfs:domain rdf:resource="http://www.ontotext.com/proton/protontop#Agent"/>
    <rdfs:comment xml:lang="en">Any author of a product. Links an author (producer) to its creation .</rdfs:comment>
  </owl:ObjectProperty>
  <owl:ObjectProperty rdf:about="http://www.ontotext.com/proton/protonext#issueOf">
    <rdfs:range rdf:resource="http://www.ontotext.com/proton/protonext#PeriodicalPublication"/>
    <rdfs:label xml:lang="en">Issue of</rdfs:label>
    <rdfs:domain rdf:resource="http://www.ontotext.com/proton/protonext#IssueOfPeriodical"/>
    <rdfs:comment xml:lang="en">A relation of a specific issue, number, and/or volume and a periodical publication.</rdfs:comment>
  </owl:ObjectProperty>
  <owl:ObjectProperty rdf:about="http://www.ontotext.com/proton/protonext#hasEMail">
    <rdfs:subPropertyOf>
      <owl:ObjectProperty rdf:about="http://www.ontotext.com/proton/protonext#hasInternetAddress"/>
    </rdfs:subPropertyOf>
    <rdfs:range rdf:resource="http://www.ontotext.com/proton/protonext#EMail"/>
    <rdfs:label xml:lang="en">has E-mail</rdfs:label>
    <rdfs:comment xml:lang="en">Relates an object (usually a person) to its email.</rdfs:comment>
  </owl:ObjectProperty>
  <owl:ObjectProperty rdf:about="http://www.ontotext.com/proton/protonext#hasISProfile">
    <rdfs:range rdf:resource="http://www.ontotext.com/proton/protonext#InformationSpaceProfile"/>
    <rdfs:label>hasISProfile</rdfs:label>
    <rdfs:domain rdf:resource="http://www.ontotext.com/proton/protonext#InformationSpace"/>
    <rdfs:comment>a relation between an Information Space and its Profile</rdfs:comment>
  </owl:ObjectProperty>
  <owl:ObjectProperty rdf:about="http://www.ontotext.com/proton/protonext#musicInstrument">
    <rdfs:range rdf:resource="http://www.ontotext.com/proton/protonext#MusicalInstrument"/>
    <rdfs:label xml:lang="en">Instrument of a Musician</rdfs:label>
    <rdfs:domain rdf:resource="http://www.ontotext.com/proton/protontop#Person"/>
    <rdfs:comment xml:lang="en">The relation between a musician and the instrument he plays</rdfs:comment>
  </owl:ObjectProperty>
  <owl:ObjectProperty rdf:about="http://www.ontotext.com/proton/protonext#nationalityOf">
    <rdfs:range rdf:resource="http://www.ontotext.com/proton/protonext#Nationality"/>
    <rdfs:label xml:lang="en">Nationality of a Person</rdfs:label>
    <rdfs:domain rdf:resource="http://www.ontotext.com/proton/protontop#Person"/>
    <rdfs:comment xml:lang="en">The nationality of a person. The relation between a person and his nationality.</rdfs:comment>
  </owl:ObjectProperty>
  <owl:ObjectProperty rdf:about="http://www.ontotext.com/proton/protonext#hasCommander">
    <rdfs:subPropertyOf rdf:resource="http://www.ontotext.com/proton/protontop#hasLeader"/>
    <rdfs:range rdf:resource="http://www.ontotext.com/proton/protontop#Person"/>
    <rdfs:label xml:lang="en">Commander</rdfs:label>
    <rdfs:domain rdf:resource="http://www.ontotext.com/proton/protonext#MilitaryUnit"/>
    <rdfs:comment xml:lang="en">The relation between a military unit and the person who commands it.</rdfs:comment>
  </owl:ObjectProperty>
  <owl:ObjectProperty rdf:about="http://www.ontotext.com/proton/protonext#officialPositionIn">
    <rdfs:range rdf:resource="http://www.ontotext.com/proton/protontop#Location"/>
    <rdfs:label xml:lang="en">Official Position in</rdfs:label>
    <rdfs:domain rdf:resource="http://www.ontotext.com/proton/protonext#OfficialPosition"/>
    <rdfs:comment xml:lang="en">This property models the Person-&gt;hasPosition-&gt;Location.</rdfs:comment>
  </owl:ObjectProperty>
  <owl:ObjectProperty rdf:about="http://www.ontotext.com/proton/protonext#acquired">
    <rdfs:range rdf:resource="http://www.ontotext.com/proton/protontop#Organization"/>
    <rdfs:label xml:lang="en">Acquired</rdfs:label>
    <rdfs:domain rdf:resource="http://www.ontotext.com/proton/protonext#Acquirement"/>
    <rdfs:comment xml:lang="en">The participant of an acquirement event which became a property of another participant in this event.</rdfs:comment>
  </owl:ObjectProperty>
  <owl:ObjectProperty rdf:about="http://www.ontotext.com/proton/protonext#genreOfAgent">
    <rdfs:range rdf:resource="http://www.ontotext.com/proton/protonext#Genre"/>
    <rdfs:label xml:lang="en">Genre Of</rdfs:label>
    <rdfs:domain rdf:resource="http://www.ontotext.com/proton/protontop#Agent"/>
    <rdfs:comment xml:lang="en">The relation between an agent and the genre he is occupied in.</rdfs:comment>
  </owl:ObjectProperty>
  <owl:ObjectProperty rdf:about="http://www.ontotext.com/proton/protonext#hasRole">
    <rdfs:label>hasRole</rdfs:label>
    <rdfs:domain rdf:resource="http://www.ontotext.com/proton/protonext#UserProfile"/>
    <owl:inverseOf rdf:resource="http://www.ontotext.com/proton/protontop#roleIn"/>
    <rdfs:range rdf:resource="http://www.ontotext.com/proton/protontop#Role"/>
    <rdfs:label xml:lang="en">has role</rdfs:label>
    <rdfs:domain rdf:resource="http://www.ontotext.com/proton/protontop#Happening"/>
    <rdfs:comment xml:lang="en">Relates a happening with some of the roles in it</rdfs:comment>
  </owl:ObjectProperty>
  <owl:ObjectProperty rdf:about="http://www.ontotext.com/proton/protonext#accountProvider">
    <rdfs:range rdf:resource="http://www.ontotext.com/proton/protontop#Agent"/>
    <rdfs:label xml:lang="en">Account Provider</rdfs:label>
    <rdfs:domain rdf:resource="http://www.ontotext.com/proton/protonext#Account"/>
    <rdfs:comment xml:lang="en">A relation between an account and an agent (usually organization) providing and managing it</rdfs:comment>
  </owl:ObjectProperty>
  <owl:ObjectProperty rdf:about="http://www.ontotext.com/proton/protonext#industryOf">
    <rdfs:range rdf:resource="http://www.ontotext.com/proton/protonext#IndustrySector"/>
    <rdfs:label xml:lang="en">Industry</rdfs:label>
    <rdfs:domain rdf:resource="http://www.ontotext.com/proton/protontop#Organization"/>
    <rdfs:comment xml:lang="en">The relation between an organization and the industry sector it is active in.</rdfs:comment>
  </owl:ObjectProperty>
  <owl:ObjectProperty rdf:about="http://www.ontotext.com/proton/protonext#conflictCombatant">
    <rdfs:subPropertyOf rdf:resource="http://www.ontotext.com/proton/protontop#hasParticipant"/>
    <rdfs:range rdf:resource="http://www.ontotext.com/proton/protonext#MilitaryOrganization"/>
    <rdfs:label xml:lang="en">Combatant</rdfs:label>
    <rdfs:domain rdf:resource="http://www.ontotext.com/proton/protonext#MilitaryConflict"/>
    <rdfs:comment xml:lang="en">The relation between a military organization, which participates as a combatant in a military conflict</rdfs:comment>
  </owl:ObjectProperty>
  <owl:ObjectProperty rdf:about="http://www.ontotext.com/proton/protonext#hasMinister">
    <rdfs:subPropertyOf rdf:resource="http://www.ontotext.com/proton/protontop#hasEmployee"/>
    <rdfs:range rdf:resource="http://www.ontotext.com/proton/protontop#Person"/>
    <rdfs:label xml:lang="en">has Minister</rdfs:label>
    <rdfs:domain rdf:resource="http://www.ontotext.com/proton/protonext#Ministry"/>
    <rdfs:comment xml:lang="en">The relation between a minister and his/her ministry.</rdfs:comment>
  </owl:ObjectProperty>
  <owl:ObjectProperty rdf:about="http://www.ontotext.com/proton/protonext#hasProfession">
    <rdfs:range rdf:resource="http://www.ontotext.com/proton/protonext#Profession"/>
    <rdfs:label xml:lang="en">has Profession</rdfs:label>
    <rdfs:domain rdf:resource="http://www.ontotext.com/proton/protontop#Person"/>
    <rdfs:comment xml:lang="en">A relation between a person and his/her profession.</rdfs:comment>
  </owl:ObjectProperty>
  <owl:ObjectProperty rdf:about="http://www.ontotext.com/proton/protonext#hasOutOfLawsTitle">
    <rdfs:subPropertyOf rdf:resource="http://www.ontotext.com/proton/protonext#hasSocialFunctionTitle"/>
    <rdfs:range rdf:resource="http://www.ontotext.com/proton/protonext#OutOfLawsTitle"/>
    <rdfs:label xml:lang="en">has OutOfLaws Title</rdfs:label>
    <rdfs:domain rdf:resource="http://www.ontotext.com/proton/protonext#OutOfLaws"/>
    <rdfs:comment xml:lang="en">The relation between the status of a criminal, and title, for instance a prisoner.</rdfs:comment>
  </owl:ObjectProperty>
  <owl:ObjectProperty rdf:about="http://www.ontotext.com/proton/protonext#hasSocialPositionCleric">
    <owl:inverseOf>
      <owl:ObjectProperty rdf:about="http://www.ontotext.com/proton/protonext#socialPositionCleric"/>
    </owl:inverseOf>
    <rdfs:subPropertyOf rdf:resource="http://www.ontotext.com/proton/protontop#hasSocialPosition"/>
    <rdfs:range rdf:resource="http://www.ontotext.com/proton/protonext#Cleric"/>
    <rdfs:label xml:lang="en">has Social Position Cleric</rdfs:label>
    <rdfs:domain rdf:resource="http://www.ontotext.com/proton/protontop#Person"/>
    <rdfs:comment xml:lang="en">The relation between a person and the social position of Cleric he has.</rdfs:comment>
  </owl:ObjectProperty>
  <owl:ObjectProperty rdf:about="http://www.ontotext.com/proton/protonext#hasBrother">
    <rdfs:subPropertyOf rdf:resource="http://www.ontotext.com/proton/protontop#hasSibling"/>
    <rdfs:range rdf:resource="http://www.ontotext.com/proton/protonext#Man"/>
    <rdfs:label xml:lang="en">has Brother</rdfs:label>
    <rdfs:comment xml:lang="en">Relates a person and his/her brother.</rdfs:comment>
  </owl:ObjectProperty>
  <owl:ObjectProperty rdf:about="http://www.ontotext.com/proton/protonext#nearby">
    <rdfs:range rdf:resource="http://www.ontotext.com/proton/protontop#Location"/>
    <rdfs:label xml:lang="en">Location Nearby another Location</rdfs:label>
    <rdfs:domain rdf:resource="http://www.ontotext.com/proton/protontop#Location"/>
    <rdfs:comment xml:lang="en">The relation of a location nearby another location</rdfs:comment>
  </owl:ObjectProperty>
  <owl:ObjectProperty rdf:about="http://www.ontotext.com/proton/protonext#subSectorOf">
    <rdfs:subPropertyOf rdf:resource="http://www.ontotext.com/proton/protontop#partOf"/>
    <rdfs:range rdf:resource="http://www.ontotext.com/proton/protonext#IndustrySector"/>
    <rdfs:label xml:lang="en">Subsector of</rdfs:label>
    <rdfs:domain rdf:resource="http://www.ontotext.com/proton/protonext#IndustrySector"/>
    <rdfs:comment xml:lang="en">The general part-of relation that takes place between a whole and each of its parts. It has number of specializations.</rdfs:comment>
    <rdf:type rdf:resource="http://www.w3.org/2002/07/owl#TransitiveProperty"/>
  </owl:ObjectProperty>
  <owl:ObjectProperty rdf:about="http://www.ontotext.com/proton/protonext#hasInternetAddress">
    <rdfs:subPropertyOf rdf:resource="http://www.ontotext.com/proton/protontop#hasContactInfo"/>
    <rdfs:range rdf:resource="http://www.ontotext.com/proton/protonext#InternetAddress"/>
    <rdfs:label xml:lang="en">has Internet Address</rdfs:label>
    <rdfs:comment xml:lang="en">Relates an object to its internet address.</rdfs:comment>
  </owl:ObjectProperty>
  <owl:ObjectProperty rdf:about="http://www.ontotext.com/proton/protonext#hasPublisher">
    <rdfs:range rdf:resource="http://www.ontotext.com/proton/protontop#Agent"/>
    <rdfs:label xml:lang="en">has Publisher</rdfs:label>
    <rdfs:domain rdf:resource="http://www.ontotext.com/proton/protonext#PublishedMaterial"/>
    <rdfs:comment xml:lang="en">An entity responsible for making the resource available. Examples of Publisher include a person, an organization, or a service. (DC2003ISO)</rdfs:comment>
  </owl:ObjectProperty>
  <owl:ObjectProperty rdf:about="http://www.ontotext.com/proton/protonext#acquirer">
    <rdfs:range rdf:resource="http://www.ontotext.com/proton/protontop#Organization"/>
    <rdfs:label xml:lang="en">Acquirer</rdfs:label>
    <rdfs:domain rdf:resource="http://www.ontotext.com/proton/protonext#Acquirement"/>
    <rdfs:comment xml:lang="en">The participant of an acquirement event which became an owner of another participant in this event.</rdfs:comment>
  </owl:ObjectProperty>
  <owl:ObjectProperty rdf:about="http://www.ontotext.com/proton/protonext#positionWithinOrganization">
    <rdfs:range rdf:resource="http://www.ontotext.com/proton/protontop#Organization"/>
    <rdfs:label xml:lang="en">Position within Organization</rdfs:label>
    <rdfs:domain rdf:resource="http://www.ontotext.com/proton/protonext#PositionOrganization"/>
    <rdfs:comment xml:lang="en">The relation between the job position and the organization it is available in. The organization where the job position is available.</rdfs:comment>
  </owl:ObjectProperty>
  <owl:ObjectProperty rdf:about="http://www.ontotext.com/proton/protonext#appointedBy">
    <rdfs:range rdf:resource="http://www.ontotext.com/proton/protontop#Person"/>
    <rdfs:label xml:lang="en">Appointed by</rdfs:label>
    <rdfs:domain rdf:resource="http://www.ontotext.com/proton/protontop#JobPosition"/>
    <rdfs:comment xml:lang="en">A concrete job position appointed by a given person.</rdfs:comment>
  </owl:ObjectProperty>
  <owl:ObjectProperty rdf:about="http://www.ontotext.com/proton/protonext#hasWife">
    <rdfs:subPropertyOf rdf:resource="http://www.ontotext.com/proton/protontop#hasSpouse"/>
    <rdfs:range rdf:resource="http://www.ontotext.com/proton/protonext#Woman"/>
    <rdfs:label xml:lang="en">has Wife</rdfs:label>
    <rdfs:domain rdf:resource="http://www.ontotext.com/proton/protonext#Man"/>
    <rdfs:comment xml:lang="en">Relates a man to his spouse.</rdfs:comment>
  </owl:ObjectProperty>
  <owl:ObjectProperty rdf:about="http://www.ontotext.com/proton/protonext#hasCurrency">
    <rdfs:range rdf:resource="http://www.ontotext.com/proton/protonext#Currency"/>
    <rdfs:label xml:lang="en">has Currency</rdfs:label>
    <rdfs:domain rdf:resource="http://www.ontotext.com/proton/protonext#Country"/>
    <rdfs:comment xml:lang="en">A relation between a country and the currency used within the country</rdfs:comment>
  </owl:ObjectProperty>
  <owl:ObjectProperty rdf:about="http://www.ontotext.com/proton/protonext#hasPoint">
    <rdfs:range rdf:resource="http://www.ontotext.com/proton/protonext#SportGamePoint"/>
    <rdfs:label xml:lang="en">Point Scorred in a Sport Game</rdfs:label>
    <rdfs:domain rdf:resource="http://www.ontotext.com/proton/protonext#SportGame"/>
    <rdfs:comment xml:lang="en">The relation between a given sport game event and a point scored in it.</rdfs:comment>
  </owl:ObjectProperty>
  <owl:ObjectProperty rdf:about="http://www.ontotext.com/proton/protonext#ownerOf">
    <rdfs:range rdf:resource="http://www.ontotext.com/proton/protontop#Agent"/>
    <rdfs:label xml:lang="en">Owner</rdfs:label>
    <rdfs:domain rdf:resource="http://www.ontotext.com/proton/protontop#Object"/>
    <rdfs:comment xml:lang="en">The relationship between an object and an agent who owns it.</rdfs:comment>
  </owl:ObjectProperty>
  <owl:ObjectProperty rdf:about="http://www.ontotext.com/proton/protonext#hasRecurringEventInstance">
    <rdfs:range rdf:resource="http://www.ontotext.com/proton/protontop#Event"/>
    <rdfs:label xml:lang="en">Recurring Event Instance</rdfs:label>
    <rdfs:domain rdf:resource="http://www.ontotext.com/proton/protonext#RecurringEvent"/>
    <rdfs:comment xml:lang="en">The relation between a particular event as an element of a recurring event.</rdfs:comment>
  </owl:ObjectProperty>
  <owl:ObjectProperty rdf:about="http://www.ontotext.com/proton/protonext#socialPositionCleric">
    <owl:inverseOf rdf:resource="http://www.ontotext.com/proton/protonext#hasSocialPositionCleric"/>
    <rdfs:subPropertyOf rdf:resource="http://www.ontotext.com/proton/protontop#socialPositionHolder"/>
    <rdfs:range rdf:resource="http://www.ontotext.com/proton/protontop#Person"/>
    <rdfs:label xml:lang="en">Social Position Cleric</rdfs:label>
    <rdfs:domain rdf:resource="http://www.ontotext.com/proton/protonext#Cleric"/>
    <rdfs:comment xml:lang="en">The relation between a social position of Cleric and the person who has it.</rdfs:comment>
  </owl:ObjectProperty>
  <owl:ObjectProperty rdf:about="http://www.ontotext.com/proton/protonext#containsLocation">
    <owl:inverseOf rdf:resource="http://www.ontotext.com/proton/protontop#subegionOf"/>
    <rdfs:comment xml:lang="en">Relation between two locations where the first contains the other.</rdfs:comment>
    <owl:inverseOf rdf:resource="http://www.ontotext.com/proton/protontop#subRegionOf"/>
    <rdfs:range rdf:resource="http://www.ontotext.com/proton/protontop#Location"/>
    <rdfs:label xml:lang="en">Contains a Location</rdfs:label>
    <rdfs:domain rdf:resource="http://www.ontotext.com/proton/protontop#Location"/>
    <rdfs:comment xml:lang="en">The relation between a location and another location that is contained by the first one.</rdfs:comment>
    <rdf:type rdf:resource="http://www.w3.org/2002/07/owl#TransitiveProperty"/>
  </owl:ObjectProperty>
  <owl:ObjectProperty rdf:about="http://www.ontotext.com/proton/protonext#hasNobeltyTitle">
    <rdfs:subPropertyOf rdf:resource="http://www.ontotext.com/proton/protonext#hasSocialFunctionTitle"/>
    <rdfs:range rdf:resource="http://www.ontotext.com/proton/protonext#NobeltyTitle"/>
    <rdfs:label xml:lang="en">has Nobetlty Title</rdfs:label>
    <rdfs:domain rdf:resource="http://www.ontotext.com/proton/protonext#Nobelty"/>
    <rdfs:comment xml:lang="en">The relation between the social position and the social title of nobelty.</rdfs:comment>
  </owl:ObjectProperty>
  <owl:ObjectProperty rdf:about="http://www.ontotext.com/proton/protonext#isBirthPlaceOf">
    <owl:inverseOf>
      <owl:ObjectProperty rdf:about="http://www.ontotext.com/proton/protonext#birthPlace"/>
    </owl:inverseOf>
    <rdfs:range rdf:resource="http://www.ontotext.com/proton/protontop#Person"/>
    <rdfs:label xml:lang="en">is a Birth Place of</rdfs:label>
    <rdfs:domain rdf:resource="http://www.ontotext.com/proton/protontop#Location"/>
    <rdfs:comment xml:lang="en">A place where a person is born. The relation between a location and a person who is born in this location.</rdfs:comment>
  </owl:ObjectProperty>
  <owl:ObjectProperty rdf:about="http://www.ontotext.com/proton/protonext#neighbour">
    <rdfs:range rdf:resource="http://www.ontotext.com/proton/protontop#Location"/>
    <rdfs:label xml:lang="en">Location Sharing a Common Location with Another Location</rdfs:label>
    <rdfs:domain rdf:resource="http://www.ontotext.com/proton/protontop#Location"/>
    <rdfs:comment xml:lang="en">The relation of a location sharing a common location with another location</rdfs:comment>
  </owl:ObjectProperty>
  <owl:ObjectProperty rdf:about="http://www.ontotext.com/proton/protonext#ofCountry">
    <rdfs:subPropertyOf rdf:resource="http://www.ontotext.com/proton/protontop#locatedIn"/>
    <rdfs:range rdf:resource="http://www.ontotext.com/proton/protonext#Country"/>
    <rdfs:label xml:lang="en">of Country</rdfs:label>
    <rdfs:domain rdf:resource="http://www.ontotext.com/proton/protonext#GovernmentOrganization"/>
    <rdfs:comment xml:lang="en">The relation between a government organization and its country.</rdfs:comment>
  </owl:ObjectProperty>
  <owl:ObjectProperty rdf:about="http://www.ontotext.com/proton/protonext#districtRepresented">
    <rdfs:range rdf:resource="http://www.ontotext.com/proton/protontop#Location"/>
    <rdfs:label xml:lang="en">Represented District</rdfs:label>
    <rdfs:domain rdf:resource="http://www.ontotext.com/proton/protonext#OfficialPosition"/>
    <rdfs:comment xml:lang="en">the relation between an official position, usually political and the location it represents. The district represented by an official position, usually political.</rdfs:comment>
  </owl:ObjectProperty>
  <owl:ObjectProperty rdf:about="http://www.ontotext.com/proton/protonext#hasWebPage">
    <rdfs:subPropertyOf rdf:resource="http://www.ontotext.com/proton/protonext#hasInternetAddress"/>
    <rdfs:range rdf:resource="http://www.ontotext.com/proton/protonext#WebPage"/>
    <rdfs:label xml:lang="en">has Web Page</rdfs:label>
    <rdfs:comment xml:lang="en">Relates an object (usually a person or an organization) to its web page.</rdfs:comment>
  </owl:ObjectProperty>
  <owl:ObjectProperty rdf:about="http://www.ontotext.com/proton/protonext#hasDevice">
    <rdfs:range rdf:resource="http://www.ontotext.com/proton/protonext#Device"/>
    <rdfs:label>hasDevice</rdfs:label>
    <rdfs:domain rdf:resource="http://www.ontotext.com/proton/protonext#UserProfile"/>
  </owl:ObjectProperty>
  <owl:ObjectProperty rdf:about="http://www.ontotext.com/proton/protonext#isInterestedIn">
    <rdfs:range rdf:resource="http://www.ontotext.com/proton/protontop#Topic"/>
    <rdfs:label>isInterestedIn</rdfs:label>
    <rdfs:domain rdf:resource="http://www.ontotext.com/proton/protonext#InformationSpaceProfile"/>
    <rdfs:domain rdf:resource="http://www.ontotext.com/proton/protonext#UserProfile"/>
  </owl:ObjectProperty>
  <owl:ObjectProperty rdf:about="http://www.ontotext.com/proton/protonext#designerOfFacility">
    <rdfs:range rdf:resource="http://www.ontotext.com/proton/protonext#Facility"/>
    <rdfs:label xml:lang="en">Designer</rdfs:label>
    <rdfs:domain rdf:resource="http://www.ontotext.com/proton/protontop#Agent"/>
    <rdfs:comment xml:lang="en">Any author of engineering and architecture designs. The relation between an author and the facility he has designed.</rdfs:comment>
  </owl:ObjectProperty>
  <owl:ObjectProperty rdf:about="http://www.ontotext.com/proton/protonext#socialPositionOutOfLaws">
    <owl:inverseOf rdf:resource="http://www.ontotext.com/proton/protonext#hasSocialPositionOutOfLaws"/>
    <rdfs:subPropertyOf rdf:resource="http://www.ontotext.com/proton/protontop#socialPositionHolder"/>
    <rdfs:range rdf:resource="http://www.ontotext.com/proton/protontop#Person"/>
    <rdfs:label xml:lang="en">Social Position Holder OutOfLaws</rdfs:label>
    <rdfs:domain rdf:resource="http://www.ontotext.com/proton/protonext#OutOfLaws"/>
    <rdfs:comment xml:lang="en">The relation between a social position of OutOfLaws and the person who has it.</rdfs:comment>
  </owl:ObjectProperty>
  <owl:ObjectProperty rdf:about="http://www.ontotext.com/proton/protonext#hasAirport">
    <rdfs:range rdf:resource="http://www.ontotext.com/proton/protonext#Airport"/>
    <rdfs:label xml:lang="en">has Airport</rdfs:label>
    <rdfs:domain rdf:resource="http://www.ontotext.com/proton/protonext#City"/>
    <rdfs:comment xml:lang="en">A relation between a city and an airport near to the city.</rdfs:comment>
  </owl:ObjectProperty>
  <owl:ObjectProperty rdf:about="http://www.ontotext.com/proton/protonext#hasUserProfile">
    <rdfs:range rdf:resource="http://www.ontotext.com/proton/protonext#UserProfile"/>
    <rdfs:label>hasUserProfile</rdfs:label>
    <rdfs:domain rdf:resource="http://www.ontotext.com/proton/protonext#User"/>
    <rdfs:comment>a relation between an User and its Profile</rdfs:comment>
  </owl:ObjectProperty>
  <owl:ObjectProperty rdf:about="http://www.ontotext.com/proton/protonext#appointmentFor">
    <rdfs:range rdf:resource="http://www.ontotext.com/proton/protonext#PositionOrganization"/>
    <rdfs:label xml:lang="en">Posision</rdfs:label>
    <rdfs:domain rdf:resource="http://www.ontotext.com/proton/protontop#JobPosition"/>
    <rdfs:comment xml:lang="en">A concrete job position which is assigned to the position available in a given organization.</rdfs:comment>
  </owl:ObjectProperty>
  <owl:ObjectProperty rdf:about="http://www.ontotext.com/proton/protonext#productOf">
    <rdfs:range rdf:resource="http://www.ontotext.com/proton/protontop#ProductModel"/>
    <rdfs:label xml:lang="en">Product</rdfs:label>
    <rdfs:domain rdf:resource="http://www.ontotext.com/proton/protontop#Organization"/>
    <rdfs:comment xml:lang="en">The relation between a producer and the product produced. The producer is restricted to an organization, like Microsoft, Ford, GM, etc.</rdfs:comment>
  </owl:ObjectProperty>
  <owl:ObjectProperty rdf:about="http://www.ontotext.com/proton/protonext#hasLocation">
    <rdfs:range rdf:resource="http://www.ontotext.com/proton/protontop#Location"/>
    <rdfs:label>hasLocation</rdfs:label>
    <rdfs:domain rdf:resource="http://www.ontotext.com/proton/protonext#UserProfile"/>
  </owl:ObjectProperty>
  <owl:ObjectProperty rdf:about="http://www.ontotext.com/proton/protonext#deathPlace">
    <rdfs:range rdf:resource="http://www.ontotext.com/proton/protontop#Location"/>
    <rdfs:label xml:lang="en">Place of Death</rdfs:label>
    <rdfs:domain rdf:resource="http://www.ontotext.com/proton/protontop#Person"/>
    <rdfs:comment xml:lang="en">The relation between a person and the place he/she died.</rdfs:comment>
  </owl:ObjectProperty>
  <owl:ObjectProperty rdf:about="http://www.ontotext.com/proton/protonext#birthPlace">
    <rdfs:range rdf:resource="http://www.ontotext.com/proton/protontop#Location"/>
    <rdfs:label xml:lang="en">Place of Birth</rdfs:label>
    <rdfs:domain rdf:resource="http://www.ontotext.com/proton/protontop#Person"/>
    <rdfs:comment xml:lang="en">The relation between a person and the place he/she is born.</rdfs:comment>
  </owl:ObjectProperty>
  <owl:ObjectProperty rdf:about="http://www.ontotext.com/proton/protonext#partOfPostalAddress">
    <rdfs:subPropertyOf rdf:resource="http://www.ontotext.com/proton/protontop#partOf"/>
    <rdfs:range rdf:resource="http://www.ontotext.com/proton/protonext#PostalAddress"/>
    <rdfs:label xml:lang="en">a Part of a Postal Address</rdfs:label>
    <rdfs:domain rdf:resource="http://www.ontotext.com/proton/protontop#ContactInformation"/>
    <rdfs:comment xml:lang="en">Relation between the part of postal address and a given postal address.</rdfs:comment>
  </owl:ObjectProperty>
  <owl:ObjectProperty rdf:about="http://www.ontotext.com/proton/protonext#hasFax">
    <rdfs:subPropertyOf rdf:resource="http://www.ontotext.com/proton/protontop#hasContactInfo"/>
    <rdfs:range rdf:resource="http://www.ontotext.com/proton/protonext#FaxNumber"/>
    <rdfs:label xml:lang="en">has Fax</rdfs:label>
    <rdfs:comment xml:lang="en">Relates an object (usually an organization) to its fax number.</rdfs:comment>
  </owl:ObjectProperty>
  <owl:ObjectProperty rdf:about="http://www.ontotext.com/proton/protonext#hasCelebrityTitle">
    <rdfs:subPropertyOf rdf:resource="http://www.ontotext.com/proton/protonext#hasSocialFunctionTitle"/>
    <rdfs:range rdf:resource="http://www.ontotext.com/proton/protonext#CelebrityTitle"/>
    <rdfs:label xml:lang="en">has Celebrity Title</rdfs:label>
    <rdfs:domain rdf:resource="http://www.ontotext.com/proton/protonext#Celebrity"/>
    <rdfs:comment xml:lang="en">The relation between the status of celebrity and its celebrity title of notoriety in the society.</rdfs:comment>
  </owl:ObjectProperty>
  <owl:ObjectProperty rdf:about="http://www.ontotext.com/proton/protonext#authorOf">
    <owl:inverseOf rdf:resource="http://www.ontotext.com/proton/protonext#isAuthorOf"/>
    <rdfs:range rdf:resource="http://www.ontotext.com/proton/protontop#Agent"/>
    <rdfs:label xml:lang="en">Author</rdfs:label>
    <rdfs:domain rdf:resource="http://www.ontotext.com/proton/protontop#Object"/>
    <rdfs:comment xml:lang="en">Any author of a product. Links any object to its author (producer).</rdfs:comment>
  </owl:ObjectProperty>
  <owl:ObjectProperty rdf:about="http://www.ontotext.com/proton/protonext#hasPrimeMinister">
    <rdfs:subPropertyOf rdf:resource="http://www.ontotext.com/proton/protonext#hasMinister"/>
    <rdfs:label xml:lang="en">has Prime Minister</rdfs:label>
    <rdfs:comment xml:lang="en">The relation between a government and its head.</rdfs:comment>
  </owl:ObjectProperty>
  <owl:DatatypeProperty rdf:about="http://www.ontotext.com/proton/protonext#finalOccuranceDate">
    <rdfs:subPropertyOf rdf:resource="http://www.ontotext.com/proton/protontop#endTime"/>
    <rdfs:label xml:lang="en">Date of Last Occurance</rdfs:label>
    <rdfs:domain rdf:resource="http://www.ontotext.com/proton/protonext#RecurringEvent"/>
    <rdfs:comment xml:lang="en">The date of the last occurrence of a recurring event.</rdfs:comment>
  </owl:DatatypeProperty>
  <owl:DatatypeProperty rdf:about="http://www.ontotext.com/proton/protonext#hasTopOffset">
    <rdfs:label>has Top Offset</rdfs:label>
    <rdfs:domain rdf:resource="http://www.ontotext.com/proton/protonext#RegionMention"/>
  </owl:DatatypeProperty>
  <owl:DatatypeProperty rdf:about="http://www.ontotext.com/proton/protonext#ISSN">
    <rdfs:subPropertyOf rdf:resource="http://www.ontotext.com/proton/protontop#informationResourceIdentifier"/>
    <rdfs:label xml:lang="en">ISSN</rdfs:label>
    <rdfs:domain rdf:resource="http://www.ontotext.com/proton/protonext#PeriodicalPublication"/>
    <rdfs:comment xml:lang="en">The ISSN (International Standard Serial Number) is an eight-digit number which identifies periodical publications as such, including electronic serials. More than one million ISSN numbers have so far been assigned.</rdfs:comment>
  </owl:DatatypeProperty>
  <owl:DatatypeProperty rdf:about="http://www.ontotext.com/proton/protonext#locationName">
    <rdfs:subPropertyOf rdf:resource="http://www.ontotext.com/proton/protontop#name"/>
    <rdfs:label xml:lang="en">Location Name</rdfs:label>
    <rdfs:label xml:lang="en">Name</rdfs:label>
    <rdfs:domain rdf:resource="http://www.ontotext.com/proton/protontop#Location"/>
    <rdfs:comment xml:lang="en">The name of a georgaphic region.</rdfs:comment>
  </owl:DatatypeProperty>
  <owl:DatatypeProperty rdf:about="http://www.ontotext.com/proton/protonext#birthDate">
    <rdfs:label xml:lang="en">Birthday</rdfs:label>
    <rdfs:domain rdf:resource="http://www.ontotext.com/proton/protontop#Person"/>
    <rdfs:comment xml:lang="en">The relation between a person and the date he/she is born.</rdfs:comment>
  </owl:DatatypeProperty>
  <owl:DatatypeProperty rdf:about="http://www.ontotext.com/proton/protonext#stockExchangeIndex">
    <rdfs:label xml:lang="en">Stock Exchange Index</rdfs:label>
    <rdfs:domain rdf:resource="http://www.ontotext.com/proton/protonext#PublicCompany"/>
    <rdfs:comment xml:lang="en">Name of the company on the Stock Exchange, where it is traded. At present, if a company is traded on two SEs with different indices, there is no way to encode which of them is applicable where.</rdfs:comment>
  </owl:DatatypeProperty>
  <owl:DatatypeProperty rdf:about="http://www.ontotext.com/proton/protonext#hasLeftOffset">
    <rdfs:subPropertyOf>
      <owl:DatatypeProperty rdf:about="http://www.ontotext.com/proton/protonext#hasStartOffset"/>
    </rdfs:subPropertyOf>
    <rdfs:label>has Left Offset</rdfs:label>
    <rdfs:domain rdf:resource="http://www.ontotext.com/proton/protonext#RegionMention"/>
  </owl:DatatypeProperty>
  <owl:DatatypeProperty rdf:about="http://www.ontotext.com/proton/protonext#hasEndOffset">
    <rdfs:label>hasEndOffset</rdfs:label>
    <rdfs:domain rdf:resource="http://www.ontotext.com/proton/protonext#Mention"/>
  </owl:DatatypeProperty>
  <owl:DatatypeProperty rdf:about="http://www.ontotext.com/proton/protonext#hasCapabilities">
    <rdfs:label>hasCapabilities</rdfs:label>
    <rdfs:domain rdf:resource="http://www.ontotext.com/proton/protonext#Device"/>
  </owl:DatatypeProperty>
  <owl:DatatypeProperty rdf:about="http://www.ontotext.com/proton/protonext#deathDate">
    <rdfs:label xml:lang="en">Deathday</rdfs:label>
    <rdfs:domain rdf:resource="http://www.ontotext.com/proton/protontop#Person"/>
    <rdfs:comment xml:lang="en">The relation between a person and the date he/she died.</rdfs:comment>
  </owl:DatatypeProperty>
  <owl:DatatypeProperty rdf:about="http://www.ontotext.com/proton/protonext#hasStartOffset">
    <rdfs:label>hasStartOffset</rdfs:label>
    <rdfs:domain rdf:resource="http://www.ontotext.com/proton/protonext#Mention"/>
  </owl:DatatypeProperty>
  <owl:DatatypeProperty rdf:about="http://www.ontotext.com/proton/protonext#firstOccuranceDate">
    <rdfs:subPropertyOf rdf:resource="http://www.ontotext.com/proton/protontop#startTime"/>
    <rdfs:label xml:lang="en">Date of First Occurance</rdfs:label>
    <rdfs:domain rdf:resource="http://www.ontotext.com/proton/protonext#RecurringEvent"/>
    <rdfs:comment xml:lang="en">The date of the first occurrence of a recurring event.</rdfs:comment>
  </owl:DatatypeProperty>
  <owl:DatatypeProperty rdf:about="http://www.ontotext.com/proton/protonext#currentFrequency">
    <rdfs:label xml:lang="en">Current Frequency</rdfs:label>
    <rdfs:domain rdf:resource="http://www.ontotext.com/proton/protonext#RecurringEvent"/>
    <rdfs:comment xml:lang="en">The relation between a recurring event and its frequency.</rdfs:comment>
  </owl:DatatypeProperty>
  <owl:DatatypeProperty rdf:about="http://www.ontotext.com/proton/protonext#hasBottomOffset">
    <rdfs:label>has Bottom Offset</rdfs:label>
    <rdfs:domain rdf:resource="http://www.ontotext.com/proton/protonext#RegionMention"/>
  </owl:DatatypeProperty>
  <owl:DatatypeProperty rdf:about="http://www.ontotext.com/proton/protonext#hasString">
    <rdfs:label>hasString</rdfs:label>
    <rdfs:domain rdf:resource="http://www.ontotext.com/proton/protonext#Mention"/>
  </owl:DatatypeProperty>
  <owl:DatatypeProperty rdf:about="http://www.ontotext.com/proton/protonext#ISBN">
    <rdfs:subPropertyOf rdf:resource="http://www.ontotext.com/proton/protontop#informationResourceIdentifier"/>
    <rdfs:label xml:lang="en">ISBN</rdfs:label>
    <rdfs:domain rdf:resource="http://www.ontotext.com/proton/protonext#Book"/>
    <rdfs:comment xml:lang="en">The ISBN (International Standard Book Number) is a unique machine-readable identification number, which marks any book unmistakably.</rdfs:comment>
  </owl:DatatypeProperty>
  <owl:DatatypeProperty rdf:about="http://www.ontotext.com/proton/protonext#fiscalNetIncome">
    <rdfs:label xml:lang="en">fiscal net income</rdfs:label>
    <rdfs:domain rdf:resource="http://www.ontotext.com/proton/protonext#CommercialOrganization"/>
    <rdfs:comment xml:lang="en">Net Income last year.</rdfs:comment>
  </owl:DatatypeProperty>
  <owl:DatatypeProperty rdf:about="http://www.ontotext.com/proton/protonext#hasUnit">
    <rdfs:label xml:lang="en">has Unit</rdfs:label>
    <rdfs:domain rdf:resource="http://www.ontotext.com/proton/protonext#Currency"/>
    <rdfs:comment xml:lang="en">Relates a currency to its unit. Examples: dollar, euro, etc.</rdfs:comment>
  </owl:DatatypeProperty>
  <owl:DatatypeProperty rdf:about="http://www.ontotext.com/proton/protonext#datePublished">
    <rdfs:subPropertyOf rdf:resource="http://www.ontotext.com/proton/protontop#hasDate"/>
    <rdfs:label xml:lang="en">Date Published</rdfs:label>
    <rdfs:domain rdf:resource="http://www.ontotext.com/proton/protonext#PublishedMaterial"/>
    <rdfs:comment xml:lang="en">Typically, associated with the creation or availability of the resource. Recommended best practice for encoding the date value is defined in a profile of ISO 8601 [W3CDTF] and includes (among others) dates of the form YYYY-MM-DD. This date is related to an event of publishing which here is implicit. If necessary for the task it can be made explicit in an extension of the ontology.</rdfs:comment>
  </owl:DatatypeProperty>
  <owl:DatatypeProperty rdf:about="http://www.ontotext.com/proton/protonext#transmission">
    <rdfs:label xml:lang="en">transmission</rdfs:label>
    <rdfs:domain rdf:resource="http://www.ontotext.com/proton/protonext#CarModel"/>
    <rdfs:comment xml:lang="en">Describes the transmission type of a given car model</rdfs:comment>
  </owl:DatatypeProperty>
  <owl:DatatypeProperty rdf:about="http://www.ontotext.com/proton/protonext#hasCode">
    <rdfs:label xml:lang="en">has Code</rdfs:label>
    <rdfs:domain rdf:resource="http://www.ontotext.com/proton/protonext#IndustrySector"/>
    <rdfs:comment xml:lang="en">Denotes that the Sector has the specified SIC code</rdfs:comment>
  </owl:DatatypeProperty>
  <owl:DatatypeProperty rdf:about="http://www.ontotext.com/proton/protonext#hasRightOffset">
    <rdfs:subPropertyOf rdf:resource="http://www.ontotext.com/proton/protonext#hasEndOffset"/>
    <rdfs:label>has Right Offset</rdfs:label>
    <rdfs:domain rdf:resource="http://www.ontotext.com/proton/protonext#RegionMention"/>
  </owl:DatatypeProperty>
  <owl:DatatypeProperty rdf:about="http://www.ontotext.com/proton/protonext#fiscalSales">
    <rdfs:label xml:lang="en">fiscal sales</rdfs:label>
    <rdfs:domain rdf:resource="http://www.ontotext.com/proton/protonext#CommercialOrganization"/>
    <rdfs:comment xml:lang="en">Sales last year.</rdfs:comment>
  </owl:DatatypeProperty>
  <pext:Sportsman rdf:about="http://www.ontotext.com/proton/protonext#BullFighter">
    <rdfs:label xml:lang="en">BullFighter</rdfs:label>
    <rdfs:label xml:lang="en">Bull Fighter</rdfs:label>
    <rdfs:comment xml:lang="en">Professional toreros (also called matadors) who execute various formal moves which can be interpreted and innovated according to the bullfighter's style or school. Wikipedia</rdfs:comment>
  </pext:Sportsman>
  <pext:Profession rdf:about="http://www.ontotext.com/proton/protonext#Priest">
    <rdfs:label xml:lang="en">Priest</rdfs:label>
    <rdfs:comment xml:lang="en">Any priest, a professsion of a person who is authorized to perform the sacred rites of a religion. (Wikipedia)</rdfs:comment>
  </pext:Profession>
  <pext:ClericTitle rdf:about="http://www.ontotext.com/proton/protonext#Pope">
    <rdfs:label xml:lang="en">Pope</rdfs:label>
    <rdfs:comment xml:lang="en">Any Pope. the head of the Roman-Catholic church.</rdfs:comment>
  </pext:ClericTitle>
  <pext:JobTitle rdf:about="http://www.ontotext.com/proton/protonext#Ambassador">
    <rdfs:label xml:lang="en">Ambassador</rdfs:label>
    <rdfs:comment xml:lang="en">Any ambassador, a title of a position of representing a country abroad</rdfs:comment>
  </pext:JobTitle>
  <pext:JobTitle rdf:about="http://www.ontotext.com/proton/protonext#Chancellor">
    <rdfs:label xml:lang="en">Chancellor</rdfs:label>
    <rdfs:comment xml:lang="en">Any Chancellor, a title of various official positions in the governments of many nations. (Wikipedia)</rdfs:comment>
  </pext:JobTitle>
  <pext:ArtProfession rdf:about="http://www.ontotext.com/proton/protonext#Artist">
    <rdfs:label xml:lang="en">Artist</rdfs:label>
    <rdfs:comment xml:lang="en">Any artist a profession engaging in a broad spectrum of activities related to creating art, practicing the arts and/or demonstrating an art. (Wikipedia)</rdfs:comment>
  </pext:ArtProfession>
  <pext:Profession rdf:about="http://www.ontotext.com/proton/protonext#Lawyer">
    <rdfs:label xml:lang="en">Lawyer</rdfs:label>
    <rdfs:comment xml:lang="en">Any lawyer, a profession of according to Black's Law Dictionary, is a person learned in the law; as an attorney, counsel or solicitor; a person who is practicing law. of judges. (Wikipedia)</rdfs:comment>
  </pext:Profession>
  <pext:Sportsman rdf:about="http://www.ontotext.com/proton/protonext#BasketballPlayer">
    <rdfs:label xml:lang="en">Basketball player</rdfs:label>
    <rdfs:comment xml:lang="en">The profession of basketball player</rdfs:comment>
  </pext:Sportsman>
  <pext:Sportsman rdf:about="http://www.ontotext.com/proton/protonext#TennisPlayer">
    <rdfs:label xml:lang="en">Tennis player</rdfs:label>
    <rdfs:comment xml:lang="en">The profession of tennis player</rdfs:comment>
  </pext:Sportsman>
  <pext:JobTitle rdf:about="http://www.ontotext.com/proton/protonext#Governor">
    <rdfs:label xml:lang="en">Governor</rdfs:label>
    <rdfs:comment xml:lang="en">Any Governor, a title of Governor of a district.</rdfs:comment>
  </pext:JobTitle>
  <pext:Sportsman rdf:about="http://www.ontotext.com/proton/protonext#GolfPlayer">
    <rdfs:label xml:lang="en">Golf Player</rdfs:label>
    <rdfs:comment xml:lang="en">Any player of Golf.</rdfs:comment>
  </pext:Sportsman>
  <pext:Sportsman rdf:about="http://www.ontotext.com/proton/protonext#NationalCollegiateAthleticAssociationAthlete">
    <rdfs:label xml:lang="en">National collegiate athletic association athlete</rdfs:label>
    <rdfs:comment xml:lang="en">The profession of national collegiate athletic association athlete</rdfs:comment>
  </pext:Sportsman>
  <pext:Profession rdf:about="http://www.ontotext.com/proton/protonext#Philosopher">
    <rdfs:label xml:lang="en">Philosopher</rdfs:label>
    <rdfs:comment xml:lang="en">Any philosopher, a profession of studying of general and fundamental problems, such as those connected with existence, knowledge, values, reason, mind, and language.</rdfs:comment>
  </pext:Profession>
  <pext:ClericTitle rdf:about="http://www.ontotext.com/proton/protonext#ChristianPatriarch">
    <rdfs:label xml:lang="en">Patriarch</rdfs:label>
    <rdfs:label xml:lang="en">Christian Patriarch</rdfs:label>
    <rdfs:comment xml:lang="en">Any Christian Patriarch.</rdfs:comment>
  </pext:ClericTitle>
  <pext:ArtProfession rdf:about="http://www.ontotext.com/proton/protonext#Musician">
    <rdfs:label xml:lang="en">Musician</rdfs:label>
    <rdfs:comment xml:lang="en">Any musician, a profession of writing, performing, or making music. (Wikipedia)</rdfs:comment>
  </pext:ArtProfession>
  <owl:AnnotationProperty rdf:about="http://www.w3.org/2000/01/rdf-schema#label"/>
  <pext:Sportsman rdf:about="http://www.ontotext.com/proton/protonext#IceHockeyPlayer">
    <rdfs:label xml:lang="en">Hockey player</rdfs:label>
    <rdfs:label xml:lang="en">Ice hockey player</rdfs:label>
    <rdfs:comment xml:lang="en">The profession of ice hockey player</rdfs:comment>
  </pext:Sportsman>
  <pext:Sportsman rdf:about="http://www.ontotext.com/proton/protonext#RugbyPlayer">
    <rdfs:label xml:lang="en">Rugby player</rdfs:label>
    <rdfs:comment xml:lang="en">The profession of rugby player</rdfs:comment>
  </pext:Sportsman>
  <pext:JobTitle rdf:about="http://www.ontotext.com/proton/protonext#Deputy">
    <rdfs:label xml:lang="en">Deputy</rdfs:label>
    <rdfs:comment xml:lang="en">The occupation of deputy</rdfs:comment>
  </pext:JobTitle>
  <pext:Sportsman rdf:about="http://www.ontotext.com/proton/protonext#VolleyballPlayer">
    <rdfs:label xml:lang="en">Snooker player</rdfs:label>
    <rdfs:comment xml:lang="en">A profession of a volleyball player.</rdfs:comment>
  </pext:Sportsman>
  <pext:ArtProfession rdf:about="http://www.ontotext.com/proton/protonext#Actor">
    <rdfs:label xml:lang="en">Actor</rdfs:label>
    <rdfs:comment xml:lang="en">Any actor acts in a dramatic production and who works in film, television, theatre, or radio in that capacity. (Wikipedia)</rdfs:comment>
  </pext:ArtProfession>
  <pext:JobTitle rdf:about="http://www.ontotext.com/proton/protonext#SoccerManager">
    <rdfs:label xml:lang="en">Soccer Manager</rdfs:label>
    <rdfs:comment xml:lang="en">Any soccer manager, the title of a manager of a soccer team.</rdfs:comment>
  </pext:JobTitle>
  <pext:Sportsman rdf:about="http://www.ontotext.com/proton/protonext#AustralianRulesFootballPlayer">
    <rdfs:label xml:lang="en">Australian rules football player</rdfs:label>
    <rdfs:comment xml:lang="en">The profession of an australian rules football player</rdfs:comment>
  </pext:Sportsman>
  <pext:ArtProfession rdf:about="http://www.ontotext.com/proton/protonext#Comedian">
    <rdfs:label xml:lang="en">Comedian</rdfs:label>
    <rdfs:comment xml:lang="en">The profession of a comedian</rdfs:comment>
  </pext:ArtProfession>
  <pext:Sportsman rdf:about="http://www.ontotext.com/proton/protonext#SoccerPlayer">
    <rdfs:label xml:lang="en">Soccer player</rdfs:label>
    <rdfs:comment xml:lang="en">The profession of soccer player</rdfs:comment>
  </pext:Sportsman>
  <pext:ArtProfession rdf:about="http://www.ontotext.com/proton/protonext#ComicsCreator">
    <rdfs:label xml:lang="en">Comics creator </rdfs:label>
    <rdfs:comment xml:lang="en">The profession of comics creator </rdfs:comment>
  </pext:ArtProfession>
  <pext:Profession rdf:about="http://www.ontotext.com/proton/protonext#MilitaryPerson">
    <rdfs:label xml:lang="en">Military Person</rdfs:label>
    <rdfs:comment xml:lang="en">Any occupation involving service in the military.</rdfs:comment>
  </pext:Profession>
  <pext:Sportsman rdf:about="http://www.ontotext.com/proton/protonext#GaelicGamesPlayer">
    <rdfs:label xml:lang="en">Gaelic games player</rdfs:label>
    <rdfs:comment xml:lang="en">The profession of gaelic games player</rdfs:comment>
  </pext:Sportsman>
  <pext:Sportsman rdf:about="http://www.ontotext.com/proton/protonext#AmericanFootballPlayer">
    <rdfs:label xml:lang="en">American Football Player</rdfs:label>
    <rdfs:comment xml:lang="en">Any player of American football.</rdfs:comment>
  </pext:Sportsman>
  <pext:Profession rdf:about="http://www.ontotext.com/proton/protonext#Judge">
    <rdfs:label xml:lang="en">Judge</rdfs:label>
    <rdfs:comment xml:lang="en">Any judge, a profession of presiding over a court of law, either alone or as part of a panel of judges. (Wikipedia)</rdfs:comment>
  </pext:Profession>
  <pext:JobTitle rdf:about="http://www.ontotext.com/proton/protonext#President">
    <rdfs:label xml:lang="en">President</rdfs:label>
    <rdfs:comment xml:lang="en">Any president, a title of a president of a country or an organization.</rdfs:comment>
  </pext:JobTitle>
  <pext:Sportsman rdf:about="http://www.ontotext.com/proton/protonext#Wrestler">
    <rdfs:label xml:lang="en">Wrestler</rdfs:label>
    <rdfs:comment xml:lang="en">The profession of wrestler</rdfs:comment>
  </pext:Sportsman>
  <pext:JobTitle rdf:about="http://www.ontotext.com/proton/protonext#VicePrimeMinister">
    <rdfs:label xml:lang="en">Vice Prime Minister</rdfs:label>
    <rdfs:comment xml:lang="en">Any Vice Prime Minister, the title of a vice prime minister in a country.</rdfs:comment>
  </pext:JobTitle>
  <pext:Sportsman rdf:about="http://www.ontotext.com/proton/protonext#SnookerPlayer">
    <rdfs:label xml:lang="en">Snooker player</rdfs:label>
    <rdfs:comment xml:lang="en">A profession of a sportsman that plays snooker, which is a billiard derivate. From DBPedia</rdfs:comment>
  </pext:Sportsman>
  <pext:ArtProfession rdf:about="http://www.ontotext.com/proton/protonext#Writer">
    <rdfs:label xml:lang="en">Writer</rdfs:label>
    <rdfs:comment xml:lang="en">Any writer, a profession of producing literary content. (Wikipedia)</rdfs:comment>
  </pext:ArtProfession>
  <pext:Sportsman rdf:about="http://www.ontotext.com/proton/protonext#GridironFootballPlayer">
    <rdfs:label xml:lang="en">Gridilon Football Player</rdfs:label>
    <rdfs:comment xml:lang="en">Any player of a gridilon football.</rdfs:comment>
  </pext:Sportsman>
  <pext:ClericTitle rdf:about="http://www.ontotext.com/proton/protonext#Bishop">
    <rdfs:label xml:lang="en">Bishop</rdfs:label>
    <rdfs:comment xml:lang="en">Any bishop, an official in the Roman-Catholic church.</rdfs:comment>
  </pext:ClericTitle>
  <pext:JobTitle rdf:about="http://www.ontotext.com/proton/protonext#Commander">
    <rdfs:label xml:lang="en">Commander</rdfs:label>
    <rdfs:comment xml:lang="en">Any commander, title of being commander or having a leading role in a military unit or other organization.</rdfs:comment>
  </pext:JobTitle>
  <pext:Sportsman rdf:about="http://www.ontotext.com/proton/protonext#ChessPlayer">
    <rdfs:label xml:lang="en">Chess player</rdfs:label>
    <rdfs:comment xml:lang="en">The profession of a chess player</rdfs:comment>
  </pext:Sportsman>
  <pext:Profession rdf:about="http://www.ontotext.com/proton/protonext#Astronaut">
    <rdfs:label xml:lang="en">Astronaut</rdfs:label>
    <rdfs:comment xml:lang="en">Any astronaut, a profession allowing to command, pilot, or serve as a crew member of a spacecraft. (Wikipedia)</rdfs:comment>
  </pext:Profession>
  <pext:NobeltyTitle rdf:about="http://www.ontotext.com/proton/protonext#Monarch">
    <rdfs:label xml:lang="en">Monarch</rdfs:label>
    <rdfs:comment xml:lang="en">Any Monarch, a title of a head of state in a monarchy.</rdfs:comment>
  </pext:NobeltyTitle>
  <pext:Sportsman rdf:about="http://www.ontotext.com/proton/protonext#Athlete">
    <rdfs:label xml:lang="en">Athlete</rdfs:label>
    <rdfs:comment xml:lang="en">Any athlete, a profession involving sport activities.</rdfs:comment>
  </pext:Sportsman>
  <owl:AnnotationProperty rdf:about="http://www.w3.org/2002/07/owl#versionInfo"/>
  <pext:Profession rdf:about="http://www.ontotext.com/proton/protonext#FashionModel">
    <rdfs:label xml:lang="en">Model</rdfs:label>
    <rdfs:comment xml:lang="en">Any model, a profession involving posing to draw attention to a particualr object or cause.</rdfs:comment>
  </pext:Profession>
  <pext:JobTitle rdf:about="http://www.ontotext.com/proton/protonext#Mayor">
    <rdfs:label xml:lang="en">Mayor</rdfs:label>
    <rdfs:comment xml:lang="en">Any Mayor, a title of the head of a municipality.</rdfs:comment>
  </pext:JobTitle>
  <pext:Sportsman rdf:about="http://www.ontotext.com/proton/protonext#Swimmer">
    <rdfs:label xml:lang="en">Swimmer</rdfs:label>
    <rdfs:comment xml:lang="en">The profession of swimmer</rdfs:comment>
  </pext:Sportsman>
  <pext:JobTitle rdf:about="http://www.ontotext.com/proton/protonext#MemberOfParliament">
    <rdfs:label xml:lang="en">Member of Parliament</rdfs:label>
    <rdfs:comment xml:lang="en">Any member of parliament, a title of a member of parliament.</rdfs:comment>
  </pext:JobTitle>
  <pext:Sportsman rdf:about="http://www.ontotext.com/proton/protonext#NascarDriver">
    <rdfs:label xml:lang="en">Nascar driver</rdfs:label>
    <rdfs:comment xml:lang="en">The profession of nascar driver</rdfs:comment>
  </pext:Sportsman>
  <pext:Sportsman rdf:about="http://www.ontotext.com/proton/protonext#MartialArtist">
    <rdfs:label xml:lang="en">Martial artist</rdfs:label>
    <rdfs:comment xml:lang="en">The profession of a martial artist</rdfs:comment>
  </pext:Sportsman>
  <pext:Profession rdf:about="http://www.ontotext.com/proton/protonext#Scientist">
    <rdfs:label xml:lang="en">Scientist</rdfs:label>
    <rdfs:comment xml:lang="en">Any scientist, a profession of studying and making research on a particualr subject.</rdfs:comment>
  </pext:Profession>
  <pext:Profession rdf:about="http://www.ontotext.com/proton/protonext#CanadianFootballPlayer">
    <rdfs:label xml:lang="en">Canadian Football Player</rdfs:label>
    <rdfs:comment xml:lang="en">Any player of Canadian football.</rdfs:comment>
  </pext:Profession>
  <pext:Profession rdf:about="http://www.ontotext.com/proton/protonext#PokerPlayer">
    <rdfs:label xml:lang="en">Poker player</rdfs:label>
    <rdfs:comment xml:lang="en">The profession of a poker player</rdfs:comment>
  </pext:Profession>
  <pext:Sportsman rdf:about="http://www.ontotext.com/proton/protonext#BaseballPlayer">
    <rdfs:label xml:lang="en">Baseball player</rdfs:label>
    <rdfs:comment xml:lang="en">The profession of baseball player</rdfs:comment>
  </pext:Sportsman>
  <pext:Profession rdf:about="http://www.ontotext.com/proton/protonext#Referee">
    <rdfs:label xml:lang="en">Referee</rdfs:label>
    <rdfs:comment xml:lang="en">A referee is the person of authority, in a variety of sports, who is responsible for presiding over the game from a neutral point of view. (Wikipedia)</rdfs:comment>
  </pext:Profession>
  <pext:Profession rdf:about="http://www.ontotext.com/proton/protonext#Journalist">
    <rdfs:label xml:lang="en">Journalist</rdfs:label>
    <rdfs:comment xml:lang="en">Any journalist, a profession of collecting and disseminating information about current events, people, trends, and issues. (Wikipedia)</rdfs:comment>
  </pext:Profession>
  <pext:JobTitle rdf:about="http://www.ontotext.com/proton/protonext#Manager">
    <rdfs:label xml:lang="en">Manager</rdfs:label>
    <rdfs:comment xml:lang="en">Any manager, the title of a management position in an organization.</rdfs:comment>
  </pext:JobTitle>
  <owl:AnnotationProperty rdf:about="http://www.w3.org/2000/01/rdf-schema#comment"/>
  <pext:JobTitle rdf:about="http://www.ontotext.com/proton/protonext#Lieutenant">
    <rdfs:label xml:lang="en">Lieutenant</rdfs:label>
    <rdfs:comment xml:lang="en">Any lieutenant, title in a military unit.</rdfs:comment>
  </pext:JobTitle>
  <pext:JobTitle rdf:about="http://www.ontotext.com/proton/protonext#CEO">
    <rdfs:label xml:lang="en">CEO</rdfs:label>
    <rdfs:comment xml:lang="en">Any CEO, a title of a chief executive officer of an organization.</rdfs:comment>
  </pext:JobTitle>
  <pext:JobTitle rdf:about="http://www.ontotext.com/proton/protonext#PrimeMinister">
    <rdfs:label xml:lang="en">Prime Minister</rdfs:label>
    <rdfs:comment xml:lang="en">Any prime minister, a title Prime minister of a country.</rdfs:comment>
  </pext:JobTitle>
  <pext:ClericTitle rdf:about="http://www.ontotext.com/proton/protonext#Cardinal">
    <rdfs:label xml:lang="en">Cardinal</rdfs:label>
    <rdfs:comment xml:lang="en">Any Cardinal, a high official in the Roman-Catholic church.</rdfs:comment>
  </pext:ClericTitle>
  <pext:JobTitle rdf:about="http://www.ontotext.com/proton/protonext#BoardMember">
    <rdfs:label xml:lang="en">Board Member</rdfs:label>
    <rdfs:comment xml:lang="en">Any board member, a title of the member of the board of any board</rdfs:comment>
  </pext:JobTitle>
  <pext:Profession rdf:about="http://www.ontotext.com/proton/protonext#Cricketer">
    <rdfs:label xml:lang="en">Cricketer </rdfs:label>
    <rdfs:comment xml:lang="en">The profession of cricketer</rdfs:comment>
  </pext:Profession>
  <pext:Sportsman rdf:about="http://www.ontotext.com/proton/protonext#BadmintonPlayer">
    <rdfs:label xml:lang="en">Badminton player</rdfs:label>
    <rdfs:comment xml:lang="en">The profession of badminton player</rdfs:comment>
  </pext:Sportsman>
  <pext:Sportsman rdf:about="http://www.ontotext.com/proton/protonext#FormulaOneRacer">
    <rdfs:label xml:lang="en">Formula one racer</rdfs:label>
    <rdfs:comment xml:lang="en">The profession of formula one racer</rdfs:comment>
  </pext:Sportsman>
  <pext:Sportsman rdf:about="http://www.ontotext.com/proton/protonext#FigureSkater">
    <rdfs:label xml:lang="en">Figure skater</rdfs:label>
    <rdfs:comment xml:lang="en">The profession of figure skater</rdfs:comment>
  </pext:Sportsman>
  <pext:JobTitle rdf:about="http://www.ontotext.com/proton/protonext#PlayboyPlaymate">
    <rdfs:label xml:lang="en">Playboy playmate</rdfs:label>
    <rdfs:comment xml:lang="en">The occupation of playboy playmate</rdfs:comment>
  </pext:JobTitle>
  <pext:NobeltyTitle rdf:about="http://www.ontotext.com/proton/protonext#BritishRoyalty">
    <rdfs:label xml:lang="en">British Royalty</rdfs:label>
    <rdfs:comment xml:lang="en">Any British Royalty, a title of a memebr of the British royal family.</rdfs:comment>
  </pext:NobeltyTitle>
  <pext:JobTitle rdf:about="http://www.ontotext.com/proton/protonext#Congressman">
    <rdfs:label xml:lang="en">Congressman</rdfs:label>
    <rdfs:comment xml:lang="en">Any Congressman, a title of a position in congress.</rdfs:comment>
  </pext:JobTitle>
  <pext:Profession rdf:about="http://www.ontotext.com/proton/protonext#Politician">
    <rdfs:label xml:lang="en">Politician</rdfs:label>
    <rdfs:comment xml:lang="en">Any Politician, a profession of participating in the political life of a given society.</rdfs:comment>
  </pext:Profession>
  <pext:JobTitle rdf:about="http://www.ontotext.com/proton/protonext#VicePresident">
    <rdfs:label xml:lang="en">Vice President</rdfs:label>
    <rdfs:comment xml:lang="en">Any Vice President, the title of a vice president in a country or in an organization.</rdfs:comment>
  </pext:JobTitle>
  <pext:Sportsman rdf:about="http://www.ontotext.com/proton/protonext#Boxer">
    <rdfs:label xml:lang="en">Boxer</rdfs:label>
    <rdfs:comment xml:lang="en">The profession of boxer</rdfs:comment>
  </pext:Sportsman>
  <pext:JobTitle rdf:about="http://www.ontotext.com/proton/protonext#Senator">
    <rdfs:label xml:lang="en">Senator</rdfs:label>
    <rdfs:comment xml:lang="en">Any Senator, a title of the member of the senat.</rdfs:comment>
  </pext:JobTitle>
  <pext:NobeltyTitle rdf:about="http://www.ontotext.com/proton/protonext#PolishKing">
    <rdfs:label xml:lang="en">Polish king</rdfs:label>
    <rdfs:comment xml:lang="en">A title of Polish kings.</rdfs:comment>
  </pext:NobeltyTitle>
</rdf:RDF>
